@prefix dcterms: <http://purl.org/dc/terms/> .
@prefix ifc: <http://www.buildingsmart-tech.org/ifcOWL/IFC4_ADD2#> .
@prefix owl: <http://www.w3.org/2002/07/owl#> .
@prefix p4bldg: <http://w3id.org/lbd/Product4BuildingOntology#> .
@prefix rdf: <http://www.w3.org/1999/02/22-rdf-syntax-ns#> .
@prefix rdfs: <http://www.w3.org/2000/01/rdf-schema#> .
@prefix xml: <http://www.w3.org/XML/1998/namespace> .
@prefix xsd: <http://www.w3.org/2001/XMLSchema#> .

<http://w3id.org/lbd/Product4BuildingOntology> a owl:Ontology ;
    dcterms:contributor "Mads Holten Rasmussen"^^xsd:string ;
    dcterms:creator <https://www.researchgate.net/profile/Georg_Schneider3>,
        "Georg Ferdinand Schneider"^^xsd:string,
        "Pieter Pauwels"^^xsd:string ;
    dcterms:description "This ontology provides a taxonomy for product elements in a building. It has been created from the ifcOWL4Add2 OWL ontology."^^xsd:string ;
    dcterms:license <http://creativecommons.org/licenses/by-sa/4.0> ;
    dcterms:title "The Product 4 building ontology."^^xsd:string ;
    owl:imports <https://w3id.org/product> .

p4bldg:Actuator-ELECTRICACTUATOR a owl:Class ;
    rdfs:label "ELECTRICACTUATOR"^^xsd:string ;
    rdfs:comment "Describe products of class ELECTRICACTUATOR a specialisation of Actuator"^^xsd:string ;
    rdfs:seeAlso ifc:IfcActuatorEnumType ;
    rdfs:subClassOf p4bldg:Actuator .

p4bldg:Actuator-HANDOPERATEDACTUATOR a owl:Class ;
    rdfs:label "HANDOPERATEDACTUATOR"^^xsd:string ;
    rdfs:comment "Describe products of class HANDOPERATEDACTUATOR a specialisation of Actuator"^^xsd:string ;
    rdfs:seeAlso ifc:IfcActuatorEnumType ;
    rdfs:subClassOf p4bldg:Actuator .

p4bldg:Actuator-HYDRAULICACTUATOR a owl:Class ;
    rdfs:label "HYDRAULICACTUATOR"^^xsd:string ;
    rdfs:comment "Describe products of class HYDRAULICACTUATOR a specialisation of Actuator"^^xsd:string ;
    rdfs:seeAlso ifc:IfcActuatorEnumType ;
    rdfs:subClassOf p4bldg:Actuator .

p4bldg:Actuator-NOTDEFINED a owl:Class ;
    rdfs:label "NOTDEFINED"^^xsd:string ;
    rdfs:comment "Describe products of class NOTDEFINED a specialisation of Actuator"^^xsd:string ;
    rdfs:seeAlso ifc:IfcActuatorEnumType ;
    rdfs:subClassOf p4bldg:Actuator .

p4bldg:Actuator-PNEUMATICACTUATOR a owl:Class ;
    rdfs:label "PNEUMATICACTUATOR"^^xsd:string ;
    rdfs:comment "Describe products of class PNEUMATICACTUATOR a specialisation of Actuator"^^xsd:string ;
    rdfs:seeAlso ifc:IfcActuatorEnumType ;
    rdfs:subClassOf p4bldg:Actuator .

p4bldg:Actuator-THERMOSTATICACTUATOR a owl:Class ;
    rdfs:label "THERMOSTATICACTUATOR"^^xsd:string ;
    rdfs:comment "Describe products of class THERMOSTATICACTUATOR a specialisation of Actuator"^^xsd:string ;
    rdfs:seeAlso ifc:IfcActuatorEnumType ;
    rdfs:subClassOf p4bldg:Actuator .

p4bldg:Actuator-USERDEFINED a owl:Class ;
    rdfs:label "USERDEFINED"^^xsd:string ;
    rdfs:comment "Describe products of class USERDEFINED a specialisation of Actuator"^^xsd:string ;
    rdfs:seeAlso ifc:IfcActuatorEnumType ;
    rdfs:subClassOf p4bldg:Actuator .

p4bldg:AirTerminal-DIFFUSER a owl:Class ;
    rdfs:label "DIFFUSER"^^xsd:string ;
    rdfs:comment "Describe products of class DIFFUSER a specialisation of AirTerminal"^^xsd:string ;
    rdfs:seeAlso ifc:IfcAirTerminalEnumType ;
    rdfs:subClassOf p4bldg:AirTerminal .

p4bldg:AirTerminal-GRILLE a owl:Class ;
    rdfs:label "GRILLE"^^xsd:string ;
    rdfs:comment "Describe products of class GRILLE a specialisation of AirTerminal"^^xsd:string ;
    rdfs:seeAlso ifc:IfcAirTerminalEnumType ;
    rdfs:subClassOf p4bldg:AirTerminal .

p4bldg:AirTerminal-LOUVRE a owl:Class ;
    rdfs:label "LOUVRE"^^xsd:string ;
    rdfs:comment "Describe products of class LOUVRE a specialisation of AirTerminal"^^xsd:string ;
    rdfs:seeAlso ifc:IfcAirTerminalEnumType ;
    rdfs:subClassOf p4bldg:AirTerminal .

p4bldg:AirTerminal-NOTDEFINED a owl:Class ;
    rdfs:label "NOTDEFINED"^^xsd:string ;
    rdfs:comment "Describe products of class NOTDEFINED a specialisation of AirTerminal"^^xsd:string ;
    rdfs:seeAlso ifc:IfcAirTerminalEnumType ;
    rdfs:subClassOf p4bldg:AirTerminal .

p4bldg:AirTerminal-REGISTER a owl:Class ;
    rdfs:label "REGISTER"^^xsd:string ;
    rdfs:comment "Describe products of class REGISTER a specialisation of AirTerminal"^^xsd:string ;
    rdfs:seeAlso ifc:IfcAirTerminalEnumType ;
    rdfs:subClassOf p4bldg:AirTerminal .

p4bldg:AirTerminal-USERDEFINED a owl:Class ;
    rdfs:label "USERDEFINED"^^xsd:string ;
    rdfs:comment "Describe products of class USERDEFINED a specialisation of AirTerminal"^^xsd:string ;
    rdfs:seeAlso ifc:IfcAirTerminalEnumType ;
    rdfs:subClassOf p4bldg:AirTerminal .

p4bldg:AirTerminalBox-CONSTANTFLOW a owl:Class ;
    rdfs:label "CONSTANTFLOW"^^xsd:string ;
    rdfs:comment "Describe products of class CONSTANTFLOW a specialisation of AirTerminalBox"^^xsd:string ;
    rdfs:seeAlso ifc:IfcAirTerminalBoxEnumType ;
    rdfs:subClassOf p4bldg:AirTerminalBox .

p4bldg:AirTerminalBox-NOTDEFINED a owl:Class ;
    rdfs:label "NOTDEFINED"^^xsd:string ;
    rdfs:comment "Describe products of class NOTDEFINED a specialisation of AirTerminalBox"^^xsd:string ;
    rdfs:seeAlso ifc:IfcAirTerminalBoxEnumType ;
    rdfs:subClassOf p4bldg:AirTerminalBox .

p4bldg:AirTerminalBox-USERDEFINED a owl:Class ;
    rdfs:label "USERDEFINED"^^xsd:string ;
    rdfs:comment "Describe products of class USERDEFINED a specialisation of AirTerminalBox"^^xsd:string ;
    rdfs:seeAlso ifc:IfcAirTerminalBoxEnumType ;
    rdfs:subClassOf p4bldg:AirTerminalBox .

p4bldg:AirTerminalBox-VARIABLEFLOWPRESSUREDEPENDANT a owl:Class ;
    rdfs:label "VARIABLEFLOWPRESSUREDEPENDANT"^^xsd:string ;
    rdfs:comment "Describe products of class VARIABLEFLOWPRESSUREDEPENDANT a specialisation of AirTerminalBox"^^xsd:string ;
    rdfs:seeAlso ifc:IfcAirTerminalBoxEnumType ;
    rdfs:subClassOf p4bldg:AirTerminalBox .

p4bldg:AirTerminalBox-VARIABLEFLOWPRESSUREINDEPENDANT a owl:Class ;
    rdfs:label "VARIABLEFLOWPRESSUREINDEPENDANT"^^xsd:string ;
    rdfs:comment "Describe products of class VARIABLEFLOWPRESSUREINDEPENDANT a specialisation of AirTerminalBox"^^xsd:string ;
    rdfs:seeAlso ifc:IfcAirTerminalBoxEnumType ;
    rdfs:subClassOf p4bldg:AirTerminalBox .

p4bldg:AirToAirHeatRecovery-FIXEDPLATECOUNTERFLOWEXCHANGER a owl:Class ;
    rdfs:label "FIXEDPLATECOUNTERFLOWEXCHANGER"^^xsd:string ;
    rdfs:comment "Describe products of class FIXEDPLATECOUNTERFLOWEXCHANGER a specialisation of AirToAirHeatRecovery"^^xsd:string ;
    rdfs:seeAlso ifc:IfcAirToAirHeatRecoveryEnumType ;
    rdfs:subClassOf p4bldg:AirToAirHeatRecovery .

p4bldg:AirToAirHeatRecovery-FIXEDPLATECROSSFLOWEXCHANGER a owl:Class ;
    rdfs:label "FIXEDPLATECROSSFLOWEXCHANGER"^^xsd:string ;
    rdfs:comment "Describe products of class FIXEDPLATECROSSFLOWEXCHANGER a specialisation of AirToAirHeatRecovery"^^xsd:string ;
    rdfs:seeAlso ifc:IfcAirToAirHeatRecoveryEnumType ;
    rdfs:subClassOf p4bldg:AirToAirHeatRecovery .

p4bldg:AirToAirHeatRecovery-FIXEDPLATEPARALLELFLOWEXCHANGER a owl:Class ;
    rdfs:label "FIXEDPLATEPARALLELFLOWEXCHANGER"^^xsd:string ;
    rdfs:comment "Describe products of class FIXEDPLATEPARALLELFLOWEXCHANGER a specialisation of AirToAirHeatRecovery"^^xsd:string ;
    rdfs:seeAlso ifc:IfcAirToAirHeatRecoveryEnumType ;
    rdfs:subClassOf p4bldg:AirToAirHeatRecovery .

p4bldg:AirToAirHeatRecovery-HEATPIPE a owl:Class ;
    rdfs:label "HEATPIPE"^^xsd:string ;
    rdfs:comment "Describe products of class HEATPIPE a specialisation of AirToAirHeatRecovery"^^xsd:string ;
    rdfs:seeAlso ifc:IfcAirToAirHeatRecoveryEnumType ;
    rdfs:subClassOf p4bldg:AirToAirHeatRecovery .

p4bldg:AirToAirHeatRecovery-NOTDEFINED a owl:Class ;
    rdfs:label "NOTDEFINED"^^xsd:string ;
    rdfs:comment "Describe products of class NOTDEFINED a specialisation of AirToAirHeatRecovery"^^xsd:string ;
    rdfs:seeAlso ifc:IfcAirToAirHeatRecoveryEnumType ;
    rdfs:subClassOf p4bldg:AirToAirHeatRecovery .

p4bldg:AirToAirHeatRecovery-ROTARYWHEEL a owl:Class ;
    rdfs:label "ROTARYWHEEL"^^xsd:string ;
    rdfs:comment "Describe products of class ROTARYWHEEL a specialisation of AirToAirHeatRecovery"^^xsd:string ;
    rdfs:seeAlso ifc:IfcAirToAirHeatRecoveryEnumType ;
    rdfs:subClassOf p4bldg:AirToAirHeatRecovery .

p4bldg:AirToAirHeatRecovery-RUNAROUNDCOILLOOP a owl:Class ;
    rdfs:label "RUNAROUNDCOILLOOP"^^xsd:string ;
    rdfs:comment "Describe products of class RUNAROUNDCOILLOOP a specialisation of AirToAirHeatRecovery"^^xsd:string ;
    rdfs:seeAlso ifc:IfcAirToAirHeatRecoveryEnumType ;
    rdfs:subClassOf p4bldg:AirToAirHeatRecovery .

p4bldg:AirToAirHeatRecovery-THERMOSIPHONCOILTYPEHEATEXCHANGERS a owl:Class ;
    rdfs:label "THERMOSIPHONCOILTYPEHEATEXCHANGERS"^^xsd:string ;
    rdfs:comment "Describe products of class THERMOSIPHONCOILTYPEHEATEXCHANGERS a specialisation of AirToAirHeatRecovery"^^xsd:string ;
    rdfs:seeAlso ifc:IfcAirToAirHeatRecoveryEnumType ;
    rdfs:subClassOf p4bldg:AirToAirHeatRecovery .

p4bldg:AirToAirHeatRecovery-THERMOSIPHONSEALEDTUBEHEATEXCHANGERS a owl:Class ;
    rdfs:label "THERMOSIPHONSEALEDTUBEHEATEXCHANGERS"^^xsd:string ;
    rdfs:comment "Describe products of class THERMOSIPHONSEALEDTUBEHEATEXCHANGERS a specialisation of AirToAirHeatRecovery"^^xsd:string ;
    rdfs:seeAlso ifc:IfcAirToAirHeatRecoveryEnumType ;
    rdfs:subClassOf p4bldg:AirToAirHeatRecovery .

p4bldg:AirToAirHeatRecovery-TWINTOWERENTHALPYRECOVERYLOOPS a owl:Class ;
    rdfs:label "TWINTOWERENTHALPYRECOVERYLOOPS"^^xsd:string ;
    rdfs:comment "Describe products of class TWINTOWERENTHALPYRECOVERYLOOPS a specialisation of AirToAirHeatRecovery"^^xsd:string ;
    rdfs:seeAlso ifc:IfcAirToAirHeatRecoveryEnumType ;
    rdfs:subClassOf p4bldg:AirToAirHeatRecovery .

p4bldg:AirToAirHeatRecovery-USERDEFINED a owl:Class ;
    rdfs:label "USERDEFINED"^^xsd:string ;
    rdfs:comment "Describe products of class USERDEFINED a specialisation of AirToAirHeatRecovery"^^xsd:string ;
    rdfs:seeAlso ifc:IfcAirToAirHeatRecoveryEnumType ;
    rdfs:subClassOf p4bldg:AirToAirHeatRecovery .

p4bldg:Alarm-BELL a owl:Class ;
    rdfs:label "BELL"^^xsd:string ;
    rdfs:comment "Describe products of class BELL a specialisation of Alarm"^^xsd:string ;
    rdfs:seeAlso ifc:IfcAlarmEnumType ;
    rdfs:subClassOf p4bldg:Alarm .

p4bldg:Alarm-BREAKGLASSBUTTON a owl:Class ;
    rdfs:label "BREAKGLASSBUTTON"^^xsd:string ;
    rdfs:comment "Describe products of class BREAKGLASSBUTTON a specialisation of Alarm"^^xsd:string ;
    rdfs:seeAlso ifc:IfcAlarmEnumType ;
    rdfs:subClassOf p4bldg:Alarm .

p4bldg:Alarm-LIGHT a owl:Class ;
    rdfs:label "LIGHT"^^xsd:string ;
    rdfs:comment "Describe products of class LIGHT a specialisation of Alarm"^^xsd:string ;
    rdfs:seeAlso ifc:IfcAlarmEnumType ;
    rdfs:subClassOf p4bldg:Alarm .

p4bldg:Alarm-MANUALPULLBOX a owl:Class ;
    rdfs:label "MANUALPULLBOX"^^xsd:string ;
    rdfs:comment "Describe products of class MANUALPULLBOX a specialisation of Alarm"^^xsd:string ;
    rdfs:seeAlso ifc:IfcAlarmEnumType ;
    rdfs:subClassOf p4bldg:Alarm .

p4bldg:Alarm-NOTDEFINED a owl:Class ;
    rdfs:label "NOTDEFINED"^^xsd:string ;
    rdfs:comment "Describe products of class NOTDEFINED a specialisation of Alarm"^^xsd:string ;
    rdfs:seeAlso ifc:IfcAlarmEnumType ;
    rdfs:subClassOf p4bldg:Alarm .

p4bldg:Alarm-SIREN a owl:Class ;
    rdfs:label "SIREN"^^xsd:string ;
    rdfs:comment "Describe products of class SIREN a specialisation of Alarm"^^xsd:string ;
    rdfs:seeAlso ifc:IfcAlarmEnumType ;
    rdfs:subClassOf p4bldg:Alarm .

p4bldg:Alarm-USERDEFINED a owl:Class ;
    rdfs:label "USERDEFINED"^^xsd:string ;
    rdfs:comment "Describe products of class USERDEFINED a specialisation of Alarm"^^xsd:string ;
    rdfs:seeAlso ifc:IfcAlarmEnumType ;
    rdfs:subClassOf p4bldg:Alarm .

p4bldg:Alarm-WHISTLE a owl:Class ;
    rdfs:label "WHISTLE"^^xsd:string ;
    rdfs:comment "Describe products of class WHISTLE a specialisation of Alarm"^^xsd:string ;
    rdfs:seeAlso ifc:IfcAlarmEnumType ;
    rdfs:subClassOf p4bldg:Alarm .

p4bldg:AudioVisualAppliance-AMPLIFIER a owl:Class ;
    rdfs:label "AMPLIFIER"^^xsd:string ;
    rdfs:comment "Describe products of class AMPLIFIER a specialisation of AudioVisualAppliance"^^xsd:string ;
    rdfs:seeAlso ifc:IfcAudioVisualApplianceEnumType ;
    rdfs:subClassOf p4bldg:AudioVisualAppliance .

p4bldg:AudioVisualAppliance-CAMERA a owl:Class ;
    rdfs:label "CAMERA"^^xsd:string ;
    rdfs:comment "Describe products of class CAMERA a specialisation of AudioVisualAppliance"^^xsd:string ;
    rdfs:seeAlso ifc:IfcAudioVisualApplianceEnumType ;
    rdfs:subClassOf p4bldg:AudioVisualAppliance .

p4bldg:AudioVisualAppliance-DISPLAY a owl:Class ;
    rdfs:label "DISPLAY"^^xsd:string ;
    rdfs:comment "Describe products of class DISPLAY a specialisation of AudioVisualAppliance"^^xsd:string ;
    rdfs:seeAlso ifc:IfcAudioVisualApplianceEnumType ;
    rdfs:subClassOf p4bldg:AudioVisualAppliance .

p4bldg:AudioVisualAppliance-MICROPHONE a owl:Class ;
    rdfs:label "MICROPHONE"^^xsd:string ;
    rdfs:comment "Describe products of class MICROPHONE a specialisation of AudioVisualAppliance"^^xsd:string ;
    rdfs:seeAlso ifc:IfcAudioVisualApplianceEnumType ;
    rdfs:subClassOf p4bldg:AudioVisualAppliance .

p4bldg:AudioVisualAppliance-NOTDEFINED a owl:Class ;
    rdfs:label "NOTDEFINED"^^xsd:string ;
    rdfs:comment "Describe products of class NOTDEFINED a specialisation of AudioVisualAppliance"^^xsd:string ;
    rdfs:seeAlso ifc:IfcAudioVisualApplianceEnumType ;
    rdfs:subClassOf p4bldg:AudioVisualAppliance .

p4bldg:AudioVisualAppliance-PLAYER a owl:Class ;
    rdfs:label "PLAYER"^^xsd:string ;
    rdfs:comment "Describe products of class PLAYER a specialisation of AudioVisualAppliance"^^xsd:string ;
    rdfs:seeAlso ifc:IfcAudioVisualApplianceEnumType ;
    rdfs:subClassOf p4bldg:AudioVisualAppliance .

p4bldg:AudioVisualAppliance-PROJECTOR a owl:Class ;
    rdfs:label "PROJECTOR"^^xsd:string ;
    rdfs:comment "Describe products of class PROJECTOR a specialisation of AudioVisualAppliance"^^xsd:string ;
    rdfs:seeAlso ifc:IfcAudioVisualApplianceEnumType ;
    rdfs:subClassOf p4bldg:AudioVisualAppliance .

p4bldg:AudioVisualAppliance-RECEIVER a owl:Class ;
    rdfs:label "RECEIVER"^^xsd:string ;
    rdfs:comment "Describe products of class RECEIVER a specialisation of AudioVisualAppliance"^^xsd:string ;
    rdfs:seeAlso ifc:IfcAudioVisualApplianceEnumType ;
    rdfs:subClassOf p4bldg:AudioVisualAppliance .

p4bldg:AudioVisualAppliance-SPEAKER a owl:Class ;
    rdfs:label "SPEAKER"^^xsd:string ;
    rdfs:comment "Describe products of class SPEAKER a specialisation of AudioVisualAppliance"^^xsd:string ;
    rdfs:seeAlso ifc:IfcAudioVisualApplianceEnumType ;
    rdfs:subClassOf p4bldg:AudioVisualAppliance .

p4bldg:AudioVisualAppliance-SWITCHER a owl:Class ;
    rdfs:label "SWITCHER"^^xsd:string ;
    rdfs:comment "Describe products of class SWITCHER a specialisation of AudioVisualAppliance"^^xsd:string ;
    rdfs:seeAlso ifc:IfcAudioVisualApplianceEnumType ;
    rdfs:subClassOf p4bldg:AudioVisualAppliance .

p4bldg:AudioVisualAppliance-TELEPHONE a owl:Class ;
    rdfs:label "TELEPHONE"^^xsd:string ;
    rdfs:comment "Describe products of class TELEPHONE a specialisation of AudioVisualAppliance"^^xsd:string ;
    rdfs:seeAlso ifc:IfcAudioVisualApplianceEnumType ;
    rdfs:subClassOf p4bldg:AudioVisualAppliance .

p4bldg:AudioVisualAppliance-TUNER a owl:Class ;
    rdfs:label "TUNER"^^xsd:string ;
    rdfs:comment "Describe products of class TUNER a specialisation of AudioVisualAppliance"^^xsd:string ;
    rdfs:seeAlso ifc:IfcAudioVisualApplianceEnumType ;
    rdfs:subClassOf p4bldg:AudioVisualAppliance .

p4bldg:AudioVisualAppliance-USERDEFINED a owl:Class ;
    rdfs:label "USERDEFINED"^^xsd:string ;
    rdfs:comment "Describe products of class USERDEFINED a specialisation of AudioVisualAppliance"^^xsd:string ;
    rdfs:seeAlso ifc:IfcAudioVisualApplianceEnumType ;
    rdfs:subClassOf p4bldg:AudioVisualAppliance .

p4bldg:Beam-BEAM a owl:Class ;
    rdfs:label "BEAM"^^xsd:string ;
    rdfs:comment "Describe products of class BEAM a specialisation of Beam"^^xsd:string ;
    rdfs:seeAlso ifc:IfcBeamEnumType ;
    rdfs:subClassOf p4bldg:Beam .

p4bldg:Beam-HOLLOWCORE a owl:Class ;
    rdfs:label "HOLLOWCORE"^^xsd:string ;
    rdfs:comment "Describe products of class HOLLOWCORE a specialisation of Beam"^^xsd:string ;
    rdfs:seeAlso ifc:IfcBeamEnumType ;
    rdfs:subClassOf p4bldg:Beam .

p4bldg:Beam-JOIST a owl:Class ;
    rdfs:label "JOIST"^^xsd:string ;
    rdfs:comment "Describe products of class JOIST a specialisation of Beam"^^xsd:string ;
    rdfs:seeAlso ifc:IfcBeamEnumType ;
    rdfs:subClassOf p4bldg:Beam .

p4bldg:Beam-LINTEL a owl:Class ;
    rdfs:label "LINTEL"^^xsd:string ;
    rdfs:comment "Describe products of class LINTEL a specialisation of Beam"^^xsd:string ;
    rdfs:seeAlso ifc:IfcBeamEnumType ;
    rdfs:subClassOf p4bldg:Beam .

p4bldg:Beam-NOTDEFINED a owl:Class ;
    rdfs:label "NOTDEFINED"^^xsd:string ;
    rdfs:comment "Describe products of class NOTDEFINED a specialisation of Beam"^^xsd:string ;
    rdfs:seeAlso ifc:IfcBeamEnumType ;
    rdfs:subClassOf p4bldg:Beam .

p4bldg:Beam-SPANDREL a owl:Class ;
    rdfs:label "SPANDREL"^^xsd:string ;
    rdfs:comment "Describe products of class SPANDREL a specialisation of Beam"^^xsd:string ;
    rdfs:seeAlso ifc:IfcBeamEnumType ;
    rdfs:subClassOf p4bldg:Beam .

p4bldg:Beam-T_BEAM a owl:Class ;
    rdfs:label "T_BEAM"^^xsd:string ;
    rdfs:comment "Describe products of class T_BEAM a specialisation of Beam"^^xsd:string ;
    rdfs:seeAlso ifc:IfcBeamEnumType ;
    rdfs:subClassOf p4bldg:Beam .

p4bldg:Beam-USERDEFINED a owl:Class ;
    rdfs:label "USERDEFINED"^^xsd:string ;
    rdfs:comment "Describe products of class USERDEFINED a specialisation of Beam"^^xsd:string ;
    rdfs:seeAlso ifc:IfcBeamEnumType ;
    rdfs:subClassOf p4bldg:Beam .

p4bldg:BeamStandardCase a owl:Class ;
    rdfs:label "BeamStandardCase"^^xsd:string ;
    rdfs:comment "Describe products of class BeamStandardCase"^^xsd:string ;
    rdfs:seeAlso ifc:IfcBeamStandardCase ;
    rdfs:subClassOf p4bldg:Beam .

p4bldg:Boiler-NOTDEFINED a owl:Class ;
    rdfs:label "NOTDEFINED"^^xsd:string ;
    rdfs:comment "Describe products of class NOTDEFINED a specialisation of Boiler"^^xsd:string ;
    rdfs:seeAlso ifc:IfcBoilerEnumType ;
    rdfs:subClassOf p4bldg:Boiler .

p4bldg:Boiler-STEAM a owl:Class ;
    rdfs:label "STEAM"^^xsd:string ;
    rdfs:comment "Describe products of class STEAM a specialisation of Boiler"^^xsd:string ;
    rdfs:seeAlso ifc:IfcBoilerEnumType ;
    rdfs:subClassOf p4bldg:Boiler .

p4bldg:Boiler-USERDEFINED a owl:Class ;
    rdfs:label "USERDEFINED"^^xsd:string ;
    rdfs:comment "Describe products of class USERDEFINED a specialisation of Boiler"^^xsd:string ;
    rdfs:seeAlso ifc:IfcBoilerEnumType ;
    rdfs:subClassOf p4bldg:Boiler .

p4bldg:Boiler-WATER a owl:Class ;
    rdfs:label "WATER"^^xsd:string ;
    rdfs:comment "Describe products of class WATER a specialisation of Boiler"^^xsd:string ;
    rdfs:seeAlso ifc:IfcBoilerEnumType ;
    rdfs:subClassOf p4bldg:Boiler .

p4bldg:BuildingElementPart-INSULATION a owl:Class ;
    rdfs:label "INSULATION"^^xsd:string ;
    rdfs:comment "Describe products of class INSULATION a specialisation of BuildingElementPart"^^xsd:string ;
    rdfs:seeAlso ifc:IfcBuildingElementPartEnumType ;
    rdfs:subClassOf p4bldg:BuildingElementPart .

p4bldg:BuildingElementPart-NOTDEFINED a owl:Class ;
    rdfs:label "NOTDEFINED"^^xsd:string ;
    rdfs:comment "Describe products of class NOTDEFINED a specialisation of BuildingElementPart"^^xsd:string ;
    rdfs:seeAlso ifc:IfcBuildingElementPartEnumType ;
    rdfs:subClassOf p4bldg:BuildingElementPart .

p4bldg:BuildingElementPart-PRECASTPANEL a owl:Class ;
    rdfs:label "PRECASTPANEL"^^xsd:string ;
    rdfs:comment "Describe products of class PRECASTPANEL a specialisation of BuildingElementPart"^^xsd:string ;
    rdfs:seeAlso ifc:IfcBuildingElementPartEnumType ;
    rdfs:subClassOf p4bldg:BuildingElementPart .

p4bldg:BuildingElementPart-USERDEFINED a owl:Class ;
    rdfs:label "USERDEFINED"^^xsd:string ;
    rdfs:comment "Describe products of class USERDEFINED a specialisation of BuildingElementPart"^^xsd:string ;
    rdfs:seeAlso ifc:IfcBuildingElementPartEnumType ;
    rdfs:subClassOf p4bldg:BuildingElementPart .

p4bldg:BuildingElementProxy-COMPLEX a owl:Class ;
    rdfs:label "COMPLEX"^^xsd:string ;
    rdfs:comment "Describe products of class COMPLEX a specialisation of BuildingElementProxy"^^xsd:string ;
    rdfs:seeAlso ifc:IfcBuildingElementProxyEnumType ;
    rdfs:subClassOf p4bldg:BuildingElementProxy .

p4bldg:BuildingElementProxy-ELEMENT a owl:Class ;
    rdfs:label "ELEMENT"^^xsd:string ;
    rdfs:comment "Describe products of class ELEMENT a specialisation of BuildingElementProxy"^^xsd:string ;
    rdfs:seeAlso ifc:IfcBuildingElementProxyEnumType ;
    rdfs:subClassOf p4bldg:BuildingElementProxy .

p4bldg:BuildingElementProxy-NOTDEFINED a owl:Class ;
    rdfs:label "NOTDEFINED"^^xsd:string ;
    rdfs:comment "Describe products of class NOTDEFINED a specialisation of BuildingElementProxy"^^xsd:string ;
    rdfs:seeAlso ifc:IfcBuildingElementProxyEnumType ;
    rdfs:subClassOf p4bldg:BuildingElementProxy .

p4bldg:BuildingElementProxy-PARTIAL a owl:Class ;
    rdfs:label "PARTIAL"^^xsd:string ;
    rdfs:comment "Describe products of class PARTIAL a specialisation of BuildingElementProxy"^^xsd:string ;
    rdfs:seeAlso ifc:IfcBuildingElementProxyEnumType ;
    rdfs:subClassOf p4bldg:BuildingElementProxy .

p4bldg:BuildingElementProxy-PROVISIONFORSPACE a owl:Class ;
    rdfs:label "PROVISIONFORSPACE"^^xsd:string ;
    rdfs:comment "Describe products of class PROVISIONFORSPACE a specialisation of BuildingElementProxy"^^xsd:string ;
    rdfs:seeAlso ifc:IfcBuildingElementProxyEnumType ;
    rdfs:subClassOf p4bldg:BuildingElementProxy .

p4bldg:BuildingElementProxy-PROVISIONFORVOID a owl:Class ;
    rdfs:label "PROVISIONFORVOID"^^xsd:string ;
    rdfs:comment "Describe products of class PROVISIONFORVOID a specialisation of BuildingElementProxy"^^xsd:string ;
    rdfs:seeAlso ifc:IfcBuildingElementProxyEnumType ;
    rdfs:subClassOf p4bldg:BuildingElementProxy .

p4bldg:BuildingElementProxy-USERDEFINED a owl:Class ;
    rdfs:label "USERDEFINED"^^xsd:string ;
    rdfs:comment "Describe products of class USERDEFINED a specialisation of BuildingElementProxy"^^xsd:string ;
    rdfs:seeAlso ifc:IfcBuildingElementProxyEnumType ;
    rdfs:subClassOf p4bldg:BuildingElementProxy .

p4bldg:Burner-NOTDEFINED a owl:Class ;
    rdfs:label "NOTDEFINED"^^xsd:string ;
    rdfs:comment "Describe products of class NOTDEFINED a specialisation of Burner"^^xsd:string ;
    rdfs:seeAlso ifc:IfcBurnerEnumType ;
    rdfs:subClassOf p4bldg:Burner .

p4bldg:Burner-USERDEFINED a owl:Class ;
    rdfs:label "USERDEFINED"^^xsd:string ;
    rdfs:comment "Describe products of class USERDEFINED a specialisation of Burner"^^xsd:string ;
    rdfs:seeAlso ifc:IfcBurnerEnumType ;
    rdfs:subClassOf p4bldg:Burner .

p4bldg:CableCarrierFitting-BEND a owl:Class ;
    rdfs:label "BEND"^^xsd:string ;
    rdfs:comment "Describe products of class BEND a specialisation of CableCarrierFitting"^^xsd:string ;
    rdfs:seeAlso ifc:IfcCableCarrierFittingEnumType ;
    rdfs:subClassOf p4bldg:CableCarrierFitting .

p4bldg:CableCarrierFitting-CROSS a owl:Class ;
    rdfs:label "CROSS"^^xsd:string ;
    rdfs:comment "Describe products of class CROSS a specialisation of CableCarrierFitting"^^xsd:string ;
    rdfs:seeAlso ifc:IfcCableCarrierFittingEnumType ;
    rdfs:subClassOf p4bldg:CableCarrierFitting .

p4bldg:CableCarrierFitting-NOTDEFINED a owl:Class ;
    rdfs:label "NOTDEFINED"^^xsd:string ;
    rdfs:comment "Describe products of class NOTDEFINED a specialisation of CableCarrierFitting"^^xsd:string ;
    rdfs:seeAlso ifc:IfcCableCarrierFittingEnumType ;
    rdfs:subClassOf p4bldg:CableCarrierFitting .

p4bldg:CableCarrierFitting-REDUCER a owl:Class ;
    rdfs:label "REDUCER"^^xsd:string ;
    rdfs:comment "Describe products of class REDUCER a specialisation of CableCarrierFitting"^^xsd:string ;
    rdfs:seeAlso ifc:IfcCableCarrierFittingEnumType ;
    rdfs:subClassOf p4bldg:CableCarrierFitting .

p4bldg:CableCarrierFitting-TEE a owl:Class ;
    rdfs:label "TEE"^^xsd:string ;
    rdfs:comment "Describe products of class TEE a specialisation of CableCarrierFitting"^^xsd:string ;
    rdfs:seeAlso ifc:IfcCableCarrierFittingEnumType ;
    rdfs:subClassOf p4bldg:CableCarrierFitting .

p4bldg:CableCarrierFitting-USERDEFINED a owl:Class ;
    rdfs:label "USERDEFINED"^^xsd:string ;
    rdfs:comment "Describe products of class USERDEFINED a specialisation of CableCarrierFitting"^^xsd:string ;
    rdfs:seeAlso ifc:IfcCableCarrierFittingEnumType ;
    rdfs:subClassOf p4bldg:CableCarrierFitting .

p4bldg:CableCarrierSegment-CABLELADDERSEGMENT a owl:Class ;
    rdfs:label "CABLELADDERSEGMENT"^^xsd:string ;
    rdfs:comment "Describe products of class CABLELADDERSEGMENT a specialisation of CableCarrierSegment"^^xsd:string ;
    rdfs:seeAlso ifc:IfcCableCarrierSegmentEnumType ;
    rdfs:subClassOf p4bldg:CableCarrierSegment .

p4bldg:CableCarrierSegment-CABLETRAYSEGMENT a owl:Class ;
    rdfs:label "CABLETRAYSEGMENT"^^xsd:string ;
    rdfs:comment "Describe products of class CABLETRAYSEGMENT a specialisation of CableCarrierSegment"^^xsd:string ;
    rdfs:seeAlso ifc:IfcCableCarrierSegmentEnumType ;
    rdfs:subClassOf p4bldg:CableCarrierSegment .

p4bldg:CableCarrierSegment-CABLETRUNKINGSEGMENT a owl:Class ;
    rdfs:label "CABLETRUNKINGSEGMENT"^^xsd:string ;
    rdfs:comment "Describe products of class CABLETRUNKINGSEGMENT a specialisation of CableCarrierSegment"^^xsd:string ;
    rdfs:seeAlso ifc:IfcCableCarrierSegmentEnumType ;
    rdfs:subClassOf p4bldg:CableCarrierSegment .

p4bldg:CableCarrierSegment-CONDUITSEGMENT a owl:Class ;
    rdfs:label "CONDUITSEGMENT"^^xsd:string ;
    rdfs:comment "Describe products of class CONDUITSEGMENT a specialisation of CableCarrierSegment"^^xsd:string ;
    rdfs:seeAlso ifc:IfcCableCarrierSegmentEnumType ;
    rdfs:subClassOf p4bldg:CableCarrierSegment .

p4bldg:CableCarrierSegment-NOTDEFINED a owl:Class ;
    rdfs:label "NOTDEFINED"^^xsd:string ;
    rdfs:comment "Describe products of class NOTDEFINED a specialisation of CableCarrierSegment"^^xsd:string ;
    rdfs:seeAlso ifc:IfcCableCarrierSegmentEnumType ;
    rdfs:subClassOf p4bldg:CableCarrierSegment .

p4bldg:CableCarrierSegment-USERDEFINED a owl:Class ;
    rdfs:label "USERDEFINED"^^xsd:string ;
    rdfs:comment "Describe products of class USERDEFINED a specialisation of CableCarrierSegment"^^xsd:string ;
    rdfs:seeAlso ifc:IfcCableCarrierSegmentEnumType ;
    rdfs:subClassOf p4bldg:CableCarrierSegment .

p4bldg:CableFitting-CONNECTOR a owl:Class ;
    rdfs:label "CONNECTOR"^^xsd:string ;
    rdfs:comment "Describe products of class CONNECTOR a specialisation of CableFitting"^^xsd:string ;
    rdfs:seeAlso ifc:IfcCableFittingEnumType ;
    rdfs:subClassOf p4bldg:CableFitting .

p4bldg:CableFitting-ENTRY a owl:Class ;
    rdfs:label "ENTRY"^^xsd:string ;
    rdfs:comment "Describe products of class ENTRY a specialisation of CableFitting"^^xsd:string ;
    rdfs:seeAlso ifc:IfcCableFittingEnumType ;
    rdfs:subClassOf p4bldg:CableFitting .

p4bldg:CableFitting-EXIT a owl:Class ;
    rdfs:label "EXIT"^^xsd:string ;
    rdfs:comment "Describe products of class EXIT a specialisation of CableFitting"^^xsd:string ;
    rdfs:seeAlso ifc:IfcCableFittingEnumType ;
    rdfs:subClassOf p4bldg:CableFitting .

p4bldg:CableFitting-JUNCTION a owl:Class ;
    rdfs:label "JUNCTION"^^xsd:string ;
    rdfs:comment "Describe products of class JUNCTION a specialisation of CableFitting"^^xsd:string ;
    rdfs:seeAlso ifc:IfcCableFittingEnumType ;
    rdfs:subClassOf p4bldg:CableFitting .

p4bldg:CableFitting-NOTDEFINED a owl:Class ;
    rdfs:label "NOTDEFINED"^^xsd:string ;
    rdfs:comment "Describe products of class NOTDEFINED a specialisation of CableFitting"^^xsd:string ;
    rdfs:seeAlso ifc:IfcCableFittingEnumType ;
    rdfs:subClassOf p4bldg:CableFitting .

p4bldg:CableFitting-TRANSITION a owl:Class ;
    rdfs:label "TRANSITION"^^xsd:string ;
    rdfs:comment "Describe products of class TRANSITION a specialisation of CableFitting"^^xsd:string ;
    rdfs:seeAlso ifc:IfcCableFittingEnumType ;
    rdfs:subClassOf p4bldg:CableFitting .

p4bldg:CableFitting-USERDEFINED a owl:Class ;
    rdfs:label "USERDEFINED"^^xsd:string ;
    rdfs:comment "Describe products of class USERDEFINED a specialisation of CableFitting"^^xsd:string ;
    rdfs:seeAlso ifc:IfcCableFittingEnumType ;
    rdfs:subClassOf p4bldg:CableFitting .

p4bldg:CableSegment-BUSBARSEGMENT a owl:Class ;
    rdfs:label "BUSBARSEGMENT"^^xsd:string ;
    rdfs:comment "Describe products of class BUSBARSEGMENT a specialisation of CableSegment"^^xsd:string ;
    rdfs:seeAlso ifc:IfcCableSegmentEnumType ;
    rdfs:subClassOf p4bldg:CableSegment .

p4bldg:CableSegment-CABLESEGMENT a owl:Class ;
    rdfs:label "CABLESEGMENT"^^xsd:string ;
    rdfs:comment "Describe products of class CABLESEGMENT a specialisation of CableSegment"^^xsd:string ;
    rdfs:seeAlso ifc:IfcCableSegmentEnumType ;
    rdfs:subClassOf p4bldg:CableSegment .

p4bldg:CableSegment-CONDUCTORSEGMENT a owl:Class ;
    rdfs:label "CONDUCTORSEGMENT"^^xsd:string ;
    rdfs:comment "Describe products of class CONDUCTORSEGMENT a specialisation of CableSegment"^^xsd:string ;
    rdfs:seeAlso ifc:IfcCableSegmentEnumType ;
    rdfs:subClassOf p4bldg:CableSegment .

p4bldg:CableSegment-CORESEGMENT a owl:Class ;
    rdfs:label "CORESEGMENT"^^xsd:string ;
    rdfs:comment "Describe products of class CORESEGMENT a specialisation of CableSegment"^^xsd:string ;
    rdfs:seeAlso ifc:IfcCableSegmentEnumType ;
    rdfs:subClassOf p4bldg:CableSegment .

p4bldg:CableSegment-NOTDEFINED a owl:Class ;
    rdfs:label "NOTDEFINED"^^xsd:string ;
    rdfs:comment "Describe products of class NOTDEFINED a specialisation of CableSegment"^^xsd:string ;
    rdfs:seeAlso ifc:IfcCableSegmentEnumType ;
    rdfs:subClassOf p4bldg:CableSegment .

p4bldg:CableSegment-USERDEFINED a owl:Class ;
    rdfs:label "USERDEFINED"^^xsd:string ;
    rdfs:comment "Describe products of class USERDEFINED a specialisation of CableSegment"^^xsd:string ;
    rdfs:seeAlso ifc:IfcCableSegmentEnumType ;
    rdfs:subClassOf p4bldg:CableSegment .

p4bldg:Chiller-AIRCOOLED a owl:Class ;
    rdfs:label "AIRCOOLED"^^xsd:string ;
    rdfs:comment "Describe products of class AIRCOOLED a specialisation of Chiller"^^xsd:string ;
    rdfs:seeAlso ifc:IfcChillerEnumType ;
    rdfs:subClassOf p4bldg:Chiller .

p4bldg:Chiller-HEATRECOVERY a owl:Class ;
    rdfs:label "HEATRECOVERY"^^xsd:string ;
    rdfs:comment "Describe products of class HEATRECOVERY a specialisation of Chiller"^^xsd:string ;
    rdfs:seeAlso ifc:IfcChillerEnumType ;
    rdfs:subClassOf p4bldg:Chiller .

p4bldg:Chiller-NOTDEFINED a owl:Class ;
    rdfs:label "NOTDEFINED"^^xsd:string ;
    rdfs:comment "Describe products of class NOTDEFINED a specialisation of Chiller"^^xsd:string ;
    rdfs:seeAlso ifc:IfcChillerEnumType ;
    rdfs:subClassOf p4bldg:Chiller .

p4bldg:Chiller-USERDEFINED a owl:Class ;
    rdfs:label "USERDEFINED"^^xsd:string ;
    rdfs:comment "Describe products of class USERDEFINED a specialisation of Chiller"^^xsd:string ;
    rdfs:seeAlso ifc:IfcChillerEnumType ;
    rdfs:subClassOf p4bldg:Chiller .

p4bldg:Chiller-WATERCOOLED a owl:Class ;
    rdfs:label "WATERCOOLED"^^xsd:string ;
    rdfs:comment "Describe products of class WATERCOOLED a specialisation of Chiller"^^xsd:string ;
    rdfs:seeAlso ifc:IfcChillerEnumType ;
    rdfs:subClassOf p4bldg:Chiller .

p4bldg:Chimney-NOTDEFINED a owl:Class ;
    rdfs:label "NOTDEFINED"^^xsd:string ;
    rdfs:comment "Describe products of class NOTDEFINED a specialisation of Chimney"^^xsd:string ;
    rdfs:seeAlso ifc:IfcChimneyEnumType ;
    rdfs:subClassOf p4bldg:Chimney .

p4bldg:Chimney-USERDEFINED a owl:Class ;
    rdfs:label "USERDEFINED"^^xsd:string ;
    rdfs:comment "Describe products of class USERDEFINED a specialisation of Chimney"^^xsd:string ;
    rdfs:seeAlso ifc:IfcChimneyEnumType ;
    rdfs:subClassOf p4bldg:Chimney .

p4bldg:CivilElement a owl:Class ;
    rdfs:label "CivilElement"^^xsd:string ;
    rdfs:comment "Describe products of class CivilElement"^^xsd:string ;
    rdfs:seeAlso ifc:IfcCivilElement ;
    rdfs:subClassOf p4bldg:Element .

p4bldg:Coil-DXCOOLINGCOIL a owl:Class ;
    rdfs:label "DXCOOLINGCOIL"^^xsd:string ;
    rdfs:comment "Describe products of class DXCOOLINGCOIL a specialisation of Coil"^^xsd:string ;
    rdfs:seeAlso ifc:IfcCoilEnumType ;
    rdfs:subClassOf p4bldg:Coil .

p4bldg:Coil-ELECTRICHEATINGCOIL a owl:Class ;
    rdfs:label "ELECTRICHEATINGCOIL"^^xsd:string ;
    rdfs:comment "Describe products of class ELECTRICHEATINGCOIL a specialisation of Coil"^^xsd:string ;
    rdfs:seeAlso ifc:IfcCoilEnumType ;
    rdfs:subClassOf p4bldg:Coil .

p4bldg:Coil-GASHEATINGCOIL a owl:Class ;
    rdfs:label "GASHEATINGCOIL"^^xsd:string ;
    rdfs:comment "Describe products of class GASHEATINGCOIL a specialisation of Coil"^^xsd:string ;
    rdfs:seeAlso ifc:IfcCoilEnumType ;
    rdfs:subClassOf p4bldg:Coil .

p4bldg:Coil-HYDRONICCOIL a owl:Class ;
    rdfs:label "HYDRONICCOIL"^^xsd:string ;
    rdfs:comment "Describe products of class HYDRONICCOIL a specialisation of Coil"^^xsd:string ;
    rdfs:seeAlso ifc:IfcCoilEnumType ;
    rdfs:subClassOf p4bldg:Coil .

p4bldg:Coil-NOTDEFINED a owl:Class ;
    rdfs:label "NOTDEFINED"^^xsd:string ;
    rdfs:comment "Describe products of class NOTDEFINED a specialisation of Coil"^^xsd:string ;
    rdfs:seeAlso ifc:IfcCoilEnumType ;
    rdfs:subClassOf p4bldg:Coil .

p4bldg:Coil-STEAMHEATINGCOIL a owl:Class ;
    rdfs:label "STEAMHEATINGCOIL"^^xsd:string ;
    rdfs:comment "Describe products of class STEAMHEATINGCOIL a specialisation of Coil"^^xsd:string ;
    rdfs:seeAlso ifc:IfcCoilEnumType ;
    rdfs:subClassOf p4bldg:Coil .

p4bldg:Coil-USERDEFINED a owl:Class ;
    rdfs:label "USERDEFINED"^^xsd:string ;
    rdfs:comment "Describe products of class USERDEFINED a specialisation of Coil"^^xsd:string ;
    rdfs:seeAlso ifc:IfcCoilEnumType ;
    rdfs:subClassOf p4bldg:Coil .

p4bldg:Coil-WATERCOOLINGCOIL a owl:Class ;
    rdfs:label "WATERCOOLINGCOIL"^^xsd:string ;
    rdfs:comment "Describe products of class WATERCOOLINGCOIL a specialisation of Coil"^^xsd:string ;
    rdfs:seeAlso ifc:IfcCoilEnumType ;
    rdfs:subClassOf p4bldg:Coil .

p4bldg:Coil-WATERHEATINGCOIL a owl:Class ;
    rdfs:label "WATERHEATINGCOIL"^^xsd:string ;
    rdfs:comment "Describe products of class WATERHEATINGCOIL a specialisation of Coil"^^xsd:string ;
    rdfs:seeAlso ifc:IfcCoilEnumType ;
    rdfs:subClassOf p4bldg:Coil .

p4bldg:Column-COLUMN a owl:Class ;
    rdfs:label "COLUMN"^^xsd:string ;
    rdfs:comment "Describe products of class COLUMN a specialisation of Column"^^xsd:string ;
    rdfs:seeAlso ifc:IfcColumnEnumType ;
    rdfs:subClassOf p4bldg:Column .

p4bldg:Column-NOTDEFINED a owl:Class ;
    rdfs:label "NOTDEFINED"^^xsd:string ;
    rdfs:comment "Describe products of class NOTDEFINED a specialisation of Column"^^xsd:string ;
    rdfs:seeAlso ifc:IfcColumnEnumType ;
    rdfs:subClassOf p4bldg:Column .

p4bldg:Column-PILASTER a owl:Class ;
    rdfs:label "PILASTER"^^xsd:string ;
    rdfs:comment "Describe products of class PILASTER a specialisation of Column"^^xsd:string ;
    rdfs:seeAlso ifc:IfcColumnEnumType ;
    rdfs:subClassOf p4bldg:Column .

p4bldg:Column-USERDEFINED a owl:Class ;
    rdfs:label "USERDEFINED"^^xsd:string ;
    rdfs:comment "Describe products of class USERDEFINED a specialisation of Column"^^xsd:string ;
    rdfs:seeAlso ifc:IfcColumnEnumType ;
    rdfs:subClassOf p4bldg:Column .

p4bldg:ColumnStandardCase a owl:Class ;
    rdfs:label "ColumnStandardCase"^^xsd:string ;
    rdfs:comment "Describe products of class ColumnStandardCase"^^xsd:string ;
    rdfs:seeAlso ifc:IfcColumnStandardCase ;
    rdfs:subClassOf p4bldg:Column .

p4bldg:CommunicationsAppliance-ANTENNA a owl:Class ;
    rdfs:label "ANTENNA"^^xsd:string ;
    rdfs:comment "Describe products of class ANTENNA a specialisation of CommunicationsAppliance"^^xsd:string ;
    rdfs:seeAlso ifc:IfcCommunicationsApplianceEnumType ;
    rdfs:subClassOf p4bldg:CommunicationsAppliance .

p4bldg:CommunicationsAppliance-COMPUTER a owl:Class ;
    rdfs:label "COMPUTER"^^xsd:string ;
    rdfs:comment "Describe products of class COMPUTER a specialisation of CommunicationsAppliance"^^xsd:string ;
    rdfs:seeAlso ifc:IfcCommunicationsApplianceEnumType ;
    rdfs:subClassOf p4bldg:CommunicationsAppliance .

p4bldg:CommunicationsAppliance-FAX a owl:Class ;
    rdfs:label "FAX"^^xsd:string ;
    rdfs:comment "Describe products of class FAX a specialisation of CommunicationsAppliance"^^xsd:string ;
    rdfs:seeAlso ifc:IfcCommunicationsApplianceEnumType ;
    rdfs:subClassOf p4bldg:CommunicationsAppliance .

p4bldg:CommunicationsAppliance-GATEWAY a owl:Class ;
    rdfs:label "GATEWAY"^^xsd:string ;
    rdfs:comment "Describe products of class GATEWAY a specialisation of CommunicationsAppliance"^^xsd:string ;
    rdfs:seeAlso ifc:IfcCommunicationsApplianceEnumType ;
    rdfs:subClassOf p4bldg:CommunicationsAppliance .

p4bldg:CommunicationsAppliance-MODEM a owl:Class ;
    rdfs:label "MODEM"^^xsd:string ;
    rdfs:comment "Describe products of class MODEM a specialisation of CommunicationsAppliance"^^xsd:string ;
    rdfs:seeAlso ifc:IfcCommunicationsApplianceEnumType ;
    rdfs:subClassOf p4bldg:CommunicationsAppliance .

p4bldg:CommunicationsAppliance-NETWORKAPPLIANCE a owl:Class ;
    rdfs:label "NETWORKAPPLIANCE"^^xsd:string ;
    rdfs:comment "Describe products of class NETWORKAPPLIANCE a specialisation of CommunicationsAppliance"^^xsd:string ;
    rdfs:seeAlso ifc:IfcCommunicationsApplianceEnumType ;
    rdfs:subClassOf p4bldg:CommunicationsAppliance .

p4bldg:CommunicationsAppliance-NETWORKBRIDGE a owl:Class ;
    rdfs:label "NETWORKBRIDGE"^^xsd:string ;
    rdfs:comment "Describe products of class NETWORKBRIDGE a specialisation of CommunicationsAppliance"^^xsd:string ;
    rdfs:seeAlso ifc:IfcCommunicationsApplianceEnumType ;
    rdfs:subClassOf p4bldg:CommunicationsAppliance .

p4bldg:CommunicationsAppliance-NETWORKHUB a owl:Class ;
    rdfs:label "NETWORKHUB"^^xsd:string ;
    rdfs:comment "Describe products of class NETWORKHUB a specialisation of CommunicationsAppliance"^^xsd:string ;
    rdfs:seeAlso ifc:IfcCommunicationsApplianceEnumType ;
    rdfs:subClassOf p4bldg:CommunicationsAppliance .

p4bldg:CommunicationsAppliance-NOTDEFINED a owl:Class ;
    rdfs:label "NOTDEFINED"^^xsd:string ;
    rdfs:comment "Describe products of class NOTDEFINED a specialisation of CommunicationsAppliance"^^xsd:string ;
    rdfs:seeAlso ifc:IfcCommunicationsApplianceEnumType ;
    rdfs:subClassOf p4bldg:CommunicationsAppliance .

p4bldg:CommunicationsAppliance-PRINTER a owl:Class ;
    rdfs:label "PRINTER"^^xsd:string ;
    rdfs:comment "Describe products of class PRINTER a specialisation of CommunicationsAppliance"^^xsd:string ;
    rdfs:seeAlso ifc:IfcCommunicationsApplianceEnumType ;
    rdfs:subClassOf p4bldg:CommunicationsAppliance .

p4bldg:CommunicationsAppliance-REPEATER a owl:Class ;
    rdfs:label "REPEATER"^^xsd:string ;
    rdfs:comment "Describe products of class REPEATER a specialisation of CommunicationsAppliance"^^xsd:string ;
    rdfs:seeAlso ifc:IfcCommunicationsApplianceEnumType ;
    rdfs:subClassOf p4bldg:CommunicationsAppliance .

p4bldg:CommunicationsAppliance-ROUTER a owl:Class ;
    rdfs:label "ROUTER"^^xsd:string ;
    rdfs:comment "Describe products of class ROUTER a specialisation of CommunicationsAppliance"^^xsd:string ;
    rdfs:seeAlso ifc:IfcCommunicationsApplianceEnumType ;
    rdfs:subClassOf p4bldg:CommunicationsAppliance .

p4bldg:CommunicationsAppliance-SCANNER a owl:Class ;
    rdfs:label "SCANNER"^^xsd:string ;
    rdfs:comment "Describe products of class SCANNER a specialisation of CommunicationsAppliance"^^xsd:string ;
    rdfs:seeAlso ifc:IfcCommunicationsApplianceEnumType ;
    rdfs:subClassOf p4bldg:CommunicationsAppliance .

p4bldg:CommunicationsAppliance-USERDEFINED a owl:Class ;
    rdfs:label "USERDEFINED"^^xsd:string ;
    rdfs:comment "Describe products of class USERDEFINED a specialisation of CommunicationsAppliance"^^xsd:string ;
    rdfs:seeAlso ifc:IfcCommunicationsApplianceEnumType ;
    rdfs:subClassOf p4bldg:CommunicationsAppliance .

p4bldg:Compressor-BOOSTER a owl:Class ;
    rdfs:label "BOOSTER"^^xsd:string ;
    rdfs:comment "Describe products of class BOOSTER a specialisation of Compressor"^^xsd:string ;
    rdfs:seeAlso ifc:IfcCompressorEnumType ;
    rdfs:subClassOf p4bldg:Compressor .

p4bldg:Compressor-DYNAMIC a owl:Class ;
    rdfs:label "DYNAMIC"^^xsd:string ;
    rdfs:comment "Describe products of class DYNAMIC a specialisation of Compressor"^^xsd:string ;
    rdfs:seeAlso ifc:IfcCompressorEnumType ;
    rdfs:subClassOf p4bldg:Compressor .

p4bldg:Compressor-HERMETIC a owl:Class ;
    rdfs:label "HERMETIC"^^xsd:string ;
    rdfs:comment "Describe products of class HERMETIC a specialisation of Compressor"^^xsd:string ;
    rdfs:seeAlso ifc:IfcCompressorEnumType ;
    rdfs:subClassOf p4bldg:Compressor .

p4bldg:Compressor-NOTDEFINED a owl:Class ;
    rdfs:label "NOTDEFINED"^^xsd:string ;
    rdfs:comment "Describe products of class NOTDEFINED a specialisation of Compressor"^^xsd:string ;
    rdfs:seeAlso ifc:IfcCompressorEnumType ;
    rdfs:subClassOf p4bldg:Compressor .

p4bldg:Compressor-OPENTYPE a owl:Class ;
    rdfs:label "OPENTYPE"^^xsd:string ;
    rdfs:comment "Describe products of class OPENTYPE a specialisation of Compressor"^^xsd:string ;
    rdfs:seeAlso ifc:IfcCompressorEnumType ;
    rdfs:subClassOf p4bldg:Compressor .

p4bldg:Compressor-RECIPROCATING a owl:Class ;
    rdfs:label "RECIPROCATING"^^xsd:string ;
    rdfs:comment "Describe products of class RECIPROCATING a specialisation of Compressor"^^xsd:string ;
    rdfs:seeAlso ifc:IfcCompressorEnumType ;
    rdfs:subClassOf p4bldg:Compressor .

p4bldg:Compressor-ROLLINGPISTON a owl:Class ;
    rdfs:label "ROLLINGPISTON"^^xsd:string ;
    rdfs:comment "Describe products of class ROLLINGPISTON a specialisation of Compressor"^^xsd:string ;
    rdfs:seeAlso ifc:IfcCompressorEnumType ;
    rdfs:subClassOf p4bldg:Compressor .

p4bldg:Compressor-ROTARY a owl:Class ;
    rdfs:label "ROTARY"^^xsd:string ;
    rdfs:comment "Describe products of class ROTARY a specialisation of Compressor"^^xsd:string ;
    rdfs:seeAlso ifc:IfcCompressorEnumType ;
    rdfs:subClassOf p4bldg:Compressor .

p4bldg:Compressor-ROTARYVANE a owl:Class ;
    rdfs:label "ROTARYVANE"^^xsd:string ;
    rdfs:comment "Describe products of class ROTARYVANE a specialisation of Compressor"^^xsd:string ;
    rdfs:seeAlso ifc:IfcCompressorEnumType ;
    rdfs:subClassOf p4bldg:Compressor .

p4bldg:Compressor-SCROLL a owl:Class ;
    rdfs:label "SCROLL"^^xsd:string ;
    rdfs:comment "Describe products of class SCROLL a specialisation of Compressor"^^xsd:string ;
    rdfs:seeAlso ifc:IfcCompressorEnumType ;
    rdfs:subClassOf p4bldg:Compressor .

p4bldg:Compressor-SEMIHERMETIC a owl:Class ;
    rdfs:label "SEMIHERMETIC"^^xsd:string ;
    rdfs:comment "Describe products of class SEMIHERMETIC a specialisation of Compressor"^^xsd:string ;
    rdfs:seeAlso ifc:IfcCompressorEnumType ;
    rdfs:subClassOf p4bldg:Compressor .

p4bldg:Compressor-SINGLESCREW a owl:Class ;
    rdfs:label "SINGLESCREW"^^xsd:string ;
    rdfs:comment "Describe products of class SINGLESCREW a specialisation of Compressor"^^xsd:string ;
    rdfs:seeAlso ifc:IfcCompressorEnumType ;
    rdfs:subClassOf p4bldg:Compressor .

p4bldg:Compressor-SINGLESTAGE a owl:Class ;
    rdfs:label "SINGLESTAGE"^^xsd:string ;
    rdfs:comment "Describe products of class SINGLESTAGE a specialisation of Compressor"^^xsd:string ;
    rdfs:seeAlso ifc:IfcCompressorEnumType ;
    rdfs:subClassOf p4bldg:Compressor .

p4bldg:Compressor-TROCHOIDAL a owl:Class ;
    rdfs:label "TROCHOIDAL"^^xsd:string ;
    rdfs:comment "Describe products of class TROCHOIDAL a specialisation of Compressor"^^xsd:string ;
    rdfs:seeAlso ifc:IfcCompressorEnumType ;
    rdfs:subClassOf p4bldg:Compressor .

p4bldg:Compressor-TWINSCREW a owl:Class ;
    rdfs:label "TWINSCREW"^^xsd:string ;
    rdfs:comment "Describe products of class TWINSCREW a specialisation of Compressor"^^xsd:string ;
    rdfs:seeAlso ifc:IfcCompressorEnumType ;
    rdfs:subClassOf p4bldg:Compressor .

p4bldg:Compressor-USERDEFINED a owl:Class ;
    rdfs:label "USERDEFINED"^^xsd:string ;
    rdfs:comment "Describe products of class USERDEFINED a specialisation of Compressor"^^xsd:string ;
    rdfs:seeAlso ifc:IfcCompressorEnumType ;
    rdfs:subClassOf p4bldg:Compressor .

p4bldg:Compressor-WELDEDSHELLHERMETIC a owl:Class ;
    rdfs:label "WELDEDSHELLHERMETIC"^^xsd:string ;
    rdfs:comment "Describe products of class WELDEDSHELLHERMETIC a specialisation of Compressor"^^xsd:string ;
    rdfs:seeAlso ifc:IfcCompressorEnumType ;
    rdfs:subClassOf p4bldg:Compressor .

p4bldg:Condenser-AIRCOOLED a owl:Class ;
    rdfs:label "AIRCOOLED"^^xsd:string ;
    rdfs:comment "Describe products of class AIRCOOLED a specialisation of Condenser"^^xsd:string ;
    rdfs:seeAlso ifc:IfcCondenserEnumType ;
    rdfs:subClassOf p4bldg:Condenser .

p4bldg:Condenser-EVAPORATIVECOOLED a owl:Class ;
    rdfs:label "EVAPORATIVECOOLED"^^xsd:string ;
    rdfs:comment "Describe products of class EVAPORATIVECOOLED a specialisation of Condenser"^^xsd:string ;
    rdfs:seeAlso ifc:IfcCondenserEnumType ;
    rdfs:subClassOf p4bldg:Condenser .

p4bldg:Condenser-NOTDEFINED a owl:Class ;
    rdfs:label "NOTDEFINED"^^xsd:string ;
    rdfs:comment "Describe products of class NOTDEFINED a specialisation of Condenser"^^xsd:string ;
    rdfs:seeAlso ifc:IfcCondenserEnumType ;
    rdfs:subClassOf p4bldg:Condenser .

p4bldg:Condenser-USERDEFINED a owl:Class ;
    rdfs:label "USERDEFINED"^^xsd:string ;
    rdfs:comment "Describe products of class USERDEFINED a specialisation of Condenser"^^xsd:string ;
    rdfs:seeAlso ifc:IfcCondenserEnumType ;
    rdfs:subClassOf p4bldg:Condenser .

p4bldg:Condenser-WATERCOOLED a owl:Class ;
    rdfs:label "WATERCOOLED"^^xsd:string ;
    rdfs:comment "Describe products of class WATERCOOLED a specialisation of Condenser"^^xsd:string ;
    rdfs:seeAlso ifc:IfcCondenserEnumType ;
    rdfs:subClassOf p4bldg:Condenser .

p4bldg:Condenser-WATERCOOLEDBRAZEDPLATE a owl:Class ;
    rdfs:label "WATERCOOLEDBRAZEDPLATE"^^xsd:string ;
    rdfs:comment "Describe products of class WATERCOOLEDBRAZEDPLATE a specialisation of Condenser"^^xsd:string ;
    rdfs:seeAlso ifc:IfcCondenserEnumType ;
    rdfs:subClassOf p4bldg:Condenser .

p4bldg:Condenser-WATERCOOLEDSHELLCOIL a owl:Class ;
    rdfs:label "WATERCOOLEDSHELLCOIL"^^xsd:string ;
    rdfs:comment "Describe products of class WATERCOOLEDSHELLCOIL a specialisation of Condenser"^^xsd:string ;
    rdfs:seeAlso ifc:IfcCondenserEnumType ;
    rdfs:subClassOf p4bldg:Condenser .

p4bldg:Condenser-WATERCOOLEDSHELLTUBE a owl:Class ;
    rdfs:label "WATERCOOLEDSHELLTUBE"^^xsd:string ;
    rdfs:comment "Describe products of class WATERCOOLEDSHELLTUBE a specialisation of Condenser"^^xsd:string ;
    rdfs:seeAlso ifc:IfcCondenserEnumType ;
    rdfs:subClassOf p4bldg:Condenser .

p4bldg:Condenser-WATERCOOLEDTUBEINTUBE a owl:Class ;
    rdfs:label "WATERCOOLEDTUBEINTUBE"^^xsd:string ;
    rdfs:comment "Describe products of class WATERCOOLEDTUBEINTUBE a specialisation of Condenser"^^xsd:string ;
    rdfs:seeAlso ifc:IfcCondenserEnumType ;
    rdfs:subClassOf p4bldg:Condenser .

p4bldg:Controller-FLOATING a owl:Class ;
    rdfs:label "FLOATING"^^xsd:string ;
    rdfs:comment "Describe products of class FLOATING a specialisation of Controller"^^xsd:string ;
    rdfs:seeAlso ifc:IfcControllerEnumType ;
    rdfs:subClassOf p4bldg:Controller .

p4bldg:Controller-MULTIPOSITION a owl:Class ;
    rdfs:label "MULTIPOSITION"^^xsd:string ;
    rdfs:comment "Describe products of class MULTIPOSITION a specialisation of Controller"^^xsd:string ;
    rdfs:seeAlso ifc:IfcControllerEnumType ;
    rdfs:subClassOf p4bldg:Controller .

p4bldg:Controller-NOTDEFINED a owl:Class ;
    rdfs:label "NOTDEFINED"^^xsd:string ;
    rdfs:comment "Describe products of class NOTDEFINED a specialisation of Controller"^^xsd:string ;
    rdfs:seeAlso ifc:IfcControllerEnumType ;
    rdfs:subClassOf p4bldg:Controller .

p4bldg:Controller-PROGRAMMABLE a owl:Class ;
    rdfs:label "PROGRAMMABLE"^^xsd:string ;
    rdfs:comment "Describe products of class PROGRAMMABLE a specialisation of Controller"^^xsd:string ;
    rdfs:seeAlso ifc:IfcControllerEnumType ;
    rdfs:subClassOf p4bldg:Controller .

p4bldg:Controller-PROPORTIONAL a owl:Class ;
    rdfs:label "PROPORTIONAL"^^xsd:string ;
    rdfs:comment "Describe products of class PROPORTIONAL a specialisation of Controller"^^xsd:string ;
    rdfs:seeAlso ifc:IfcControllerEnumType ;
    rdfs:subClassOf p4bldg:Controller .

p4bldg:Controller-TWOPOSITION a owl:Class ;
    rdfs:label "TWOPOSITION"^^xsd:string ;
    rdfs:comment "Describe products of class TWOPOSITION a specialisation of Controller"^^xsd:string ;
    rdfs:seeAlso ifc:IfcControllerEnumType ;
    rdfs:subClassOf p4bldg:Controller .

p4bldg:Controller-USERDEFINED a owl:Class ;
    rdfs:label "USERDEFINED"^^xsd:string ;
    rdfs:comment "Describe products of class USERDEFINED a specialisation of Controller"^^xsd:string ;
    rdfs:seeAlso ifc:IfcControllerEnumType ;
    rdfs:subClassOf p4bldg:Controller .

p4bldg:CooledBeam-ACTIVE a owl:Class ;
    rdfs:label "ACTIVE"^^xsd:string ;
    rdfs:comment "Describe products of class ACTIVE a specialisation of CooledBeam"^^xsd:string ;
    rdfs:seeAlso ifc:IfcCooledBeamEnumType ;
    rdfs:subClassOf p4bldg:CooledBeam .

p4bldg:CooledBeam-NOTDEFINED a owl:Class ;
    rdfs:label "NOTDEFINED"^^xsd:string ;
    rdfs:comment "Describe products of class NOTDEFINED a specialisation of CooledBeam"^^xsd:string ;
    rdfs:seeAlso ifc:IfcCooledBeamEnumType ;
    rdfs:subClassOf p4bldg:CooledBeam .

p4bldg:CooledBeam-PASSIVE a owl:Class ;
    rdfs:label "PASSIVE"^^xsd:string ;
    rdfs:comment "Describe products of class PASSIVE a specialisation of CooledBeam"^^xsd:string ;
    rdfs:seeAlso ifc:IfcCooledBeamEnumType ;
    rdfs:subClassOf p4bldg:CooledBeam .

p4bldg:CooledBeam-USERDEFINED a owl:Class ;
    rdfs:label "USERDEFINED"^^xsd:string ;
    rdfs:comment "Describe products of class USERDEFINED a specialisation of CooledBeam"^^xsd:string ;
    rdfs:seeAlso ifc:IfcCooledBeamEnumType ;
    rdfs:subClassOf p4bldg:CooledBeam .

p4bldg:CoolingTower-MECHANICALFORCEDDRAFT a owl:Class ;
    rdfs:label "MECHANICALFORCEDDRAFT"^^xsd:string ;
    rdfs:comment "Describe products of class MECHANICALFORCEDDRAFT a specialisation of CoolingTower"^^xsd:string ;
    rdfs:seeAlso ifc:IfcCoolingTowerEnumType ;
    rdfs:subClassOf p4bldg:CoolingTower .

p4bldg:CoolingTower-MECHANICALINDUCEDDRAFT a owl:Class ;
    rdfs:label "MECHANICALINDUCEDDRAFT"^^xsd:string ;
    rdfs:comment "Describe products of class MECHANICALINDUCEDDRAFT a specialisation of CoolingTower"^^xsd:string ;
    rdfs:seeAlso ifc:IfcCoolingTowerEnumType ;
    rdfs:subClassOf p4bldg:CoolingTower .

p4bldg:CoolingTower-NATURALDRAFT a owl:Class ;
    rdfs:label "NATURALDRAFT"^^xsd:string ;
    rdfs:comment "Describe products of class NATURALDRAFT a specialisation of CoolingTower"^^xsd:string ;
    rdfs:seeAlso ifc:IfcCoolingTowerEnumType ;
    rdfs:subClassOf p4bldg:CoolingTower .

p4bldg:CoolingTower-NOTDEFINED a owl:Class ;
    rdfs:label "NOTDEFINED"^^xsd:string ;
    rdfs:comment "Describe products of class NOTDEFINED a specialisation of CoolingTower"^^xsd:string ;
    rdfs:seeAlso ifc:IfcCoolingTowerEnumType ;
    rdfs:subClassOf p4bldg:CoolingTower .

p4bldg:CoolingTower-USERDEFINED a owl:Class ;
    rdfs:label "USERDEFINED"^^xsd:string ;
    rdfs:comment "Describe products of class USERDEFINED a specialisation of CoolingTower"^^xsd:string ;
    rdfs:seeAlso ifc:IfcCoolingTowerEnumType ;
    rdfs:subClassOf p4bldg:CoolingTower .

p4bldg:Covering-CEILING a owl:Class ;
    rdfs:label "CEILING"^^xsd:string ;
    rdfs:comment "Describe products of class CEILING a specialisation of Covering"^^xsd:string ;
    rdfs:seeAlso ifc:IfcCoveringEnumType ;
    rdfs:subClassOf p4bldg:Covering .

p4bldg:Covering-CLADDING a owl:Class ;
    rdfs:label "CLADDING"^^xsd:string ;
    rdfs:comment "Describe products of class CLADDING a specialisation of Covering"^^xsd:string ;
    rdfs:seeAlso ifc:IfcCoveringEnumType ;
    rdfs:subClassOf p4bldg:Covering .

p4bldg:Covering-FLOORING a owl:Class ;
    rdfs:label "FLOORING"^^xsd:string ;
    rdfs:comment "Describe products of class FLOORING a specialisation of Covering"^^xsd:string ;
    rdfs:seeAlso ifc:IfcCoveringEnumType ;
    rdfs:subClassOf p4bldg:Covering .

p4bldg:Covering-INSULATION a owl:Class ;
    rdfs:label "INSULATION"^^xsd:string ;
    rdfs:comment "Describe products of class INSULATION a specialisation of Covering"^^xsd:string ;
    rdfs:seeAlso ifc:IfcCoveringEnumType ;
    rdfs:subClassOf p4bldg:Covering .

p4bldg:Covering-MEMBRANE a owl:Class ;
    rdfs:label "MEMBRANE"^^xsd:string ;
    rdfs:comment "Describe products of class MEMBRANE a specialisation of Covering"^^xsd:string ;
    rdfs:seeAlso ifc:IfcCoveringEnumType ;
    rdfs:subClassOf p4bldg:Covering .

p4bldg:Covering-MOLDING a owl:Class ;
    rdfs:label "MOLDING"^^xsd:string ;
    rdfs:comment "Describe products of class MOLDING a specialisation of Covering"^^xsd:string ;
    rdfs:seeAlso ifc:IfcCoveringEnumType ;
    rdfs:subClassOf p4bldg:Covering .

p4bldg:Covering-NOTDEFINED a owl:Class ;
    rdfs:label "NOTDEFINED"^^xsd:string ;
    rdfs:comment "Describe products of class NOTDEFINED a specialisation of Covering"^^xsd:string ;
    rdfs:seeAlso ifc:IfcCoveringEnumType ;
    rdfs:subClassOf p4bldg:Covering .

p4bldg:Covering-ROOFING a owl:Class ;
    rdfs:label "ROOFING"^^xsd:string ;
    rdfs:comment "Describe products of class ROOFING a specialisation of Covering"^^xsd:string ;
    rdfs:seeAlso ifc:IfcCoveringEnumType ;
    rdfs:subClassOf p4bldg:Covering .

p4bldg:Covering-SKIRTINGBOARD a owl:Class ;
    rdfs:label "SKIRTINGBOARD"^^xsd:string ;
    rdfs:comment "Describe products of class SKIRTINGBOARD a specialisation of Covering"^^xsd:string ;
    rdfs:seeAlso ifc:IfcCoveringEnumType ;
    rdfs:subClassOf p4bldg:Covering .

p4bldg:Covering-SLEEVING a owl:Class ;
    rdfs:label "SLEEVING"^^xsd:string ;
    rdfs:comment "Describe products of class SLEEVING a specialisation of Covering"^^xsd:string ;
    rdfs:seeAlso ifc:IfcCoveringEnumType ;
    rdfs:subClassOf p4bldg:Covering .

p4bldg:Covering-USERDEFINED a owl:Class ;
    rdfs:label "USERDEFINED"^^xsd:string ;
    rdfs:comment "Describe products of class USERDEFINED a specialisation of Covering"^^xsd:string ;
    rdfs:seeAlso ifc:IfcCoveringEnumType ;
    rdfs:subClassOf p4bldg:Covering .

p4bldg:Covering-WRAPPING a owl:Class ;
    rdfs:label "WRAPPING"^^xsd:string ;
    rdfs:comment "Describe products of class WRAPPING a specialisation of Covering"^^xsd:string ;
    rdfs:seeAlso ifc:IfcCoveringEnumType ;
    rdfs:subClassOf p4bldg:Covering .

p4bldg:CurtainWall-NOTDEFINED a owl:Class ;
    rdfs:label "NOTDEFINED"^^xsd:string ;
    rdfs:comment "Describe products of class NOTDEFINED a specialisation of CurtainWall"^^xsd:string ;
    rdfs:seeAlso ifc:IfcCurtainWallEnumType ;
    rdfs:subClassOf p4bldg:CurtainWall .

p4bldg:CurtainWall-USERDEFINED a owl:Class ;
    rdfs:label "USERDEFINED"^^xsd:string ;
    rdfs:comment "Describe products of class USERDEFINED a specialisation of CurtainWall"^^xsd:string ;
    rdfs:seeAlso ifc:IfcCurtainWallEnumType ;
    rdfs:subClassOf p4bldg:CurtainWall .

p4bldg:Damper-BACKDRAFTDAMPER a owl:Class ;
    rdfs:label "BACKDRAFTDAMPER"^^xsd:string ;
    rdfs:comment "Describe products of class BACKDRAFTDAMPER a specialisation of Damper"^^xsd:string ;
    rdfs:seeAlso ifc:IfcDamperEnumType ;
    rdfs:subClassOf p4bldg:Damper .

p4bldg:Damper-BALANCINGDAMPER a owl:Class ;
    rdfs:label "BALANCINGDAMPER"^^xsd:string ;
    rdfs:comment "Describe products of class BALANCINGDAMPER a specialisation of Damper"^^xsd:string ;
    rdfs:seeAlso ifc:IfcDamperEnumType ;
    rdfs:subClassOf p4bldg:Damper .

p4bldg:Damper-BLASTDAMPER a owl:Class ;
    rdfs:label "BLASTDAMPER"^^xsd:string ;
    rdfs:comment "Describe products of class BLASTDAMPER a specialisation of Damper"^^xsd:string ;
    rdfs:seeAlso ifc:IfcDamperEnumType ;
    rdfs:subClassOf p4bldg:Damper .

p4bldg:Damper-CONTROLDAMPER a owl:Class ;
    rdfs:label "CONTROLDAMPER"^^xsd:string ;
    rdfs:comment "Describe products of class CONTROLDAMPER a specialisation of Damper"^^xsd:string ;
    rdfs:seeAlso ifc:IfcDamperEnumType ;
    rdfs:subClassOf p4bldg:Damper .

p4bldg:Damper-FIREDAMPER a owl:Class ;
    rdfs:label "FIREDAMPER"^^xsd:string ;
    rdfs:comment "Describe products of class FIREDAMPER a specialisation of Damper"^^xsd:string ;
    rdfs:seeAlso ifc:IfcDamperEnumType ;
    rdfs:subClassOf p4bldg:Damper .

p4bldg:Damper-FIRESMOKEDAMPER a owl:Class ;
    rdfs:label "FIRESMOKEDAMPER"^^xsd:string ;
    rdfs:comment "Describe products of class FIRESMOKEDAMPER a specialisation of Damper"^^xsd:string ;
    rdfs:seeAlso ifc:IfcDamperEnumType ;
    rdfs:subClassOf p4bldg:Damper .

p4bldg:Damper-FUMEHOODEXHAUST a owl:Class ;
    rdfs:label "FUMEHOODEXHAUST"^^xsd:string ;
    rdfs:comment "Describe products of class FUMEHOODEXHAUST a specialisation of Damper"^^xsd:string ;
    rdfs:seeAlso ifc:IfcDamperEnumType ;
    rdfs:subClassOf p4bldg:Damper .

p4bldg:Damper-GRAVITYDAMPER a owl:Class ;
    rdfs:label "GRAVITYDAMPER"^^xsd:string ;
    rdfs:comment "Describe products of class GRAVITYDAMPER a specialisation of Damper"^^xsd:string ;
    rdfs:seeAlso ifc:IfcDamperEnumType ;
    rdfs:subClassOf p4bldg:Damper .

p4bldg:Damper-GRAVITYRELIEFDAMPER a owl:Class ;
    rdfs:label "GRAVITYRELIEFDAMPER"^^xsd:string ;
    rdfs:comment "Describe products of class GRAVITYRELIEFDAMPER a specialisation of Damper"^^xsd:string ;
    rdfs:seeAlso ifc:IfcDamperEnumType ;
    rdfs:subClassOf p4bldg:Damper .

p4bldg:Damper-NOTDEFINED a owl:Class ;
    rdfs:label "NOTDEFINED"^^xsd:string ;
    rdfs:comment "Describe products of class NOTDEFINED a specialisation of Damper"^^xsd:string ;
    rdfs:seeAlso ifc:IfcDamperEnumType ;
    rdfs:subClassOf p4bldg:Damper .

p4bldg:Damper-RELIEFDAMPER a owl:Class ;
    rdfs:label "RELIEFDAMPER"^^xsd:string ;
    rdfs:comment "Describe products of class RELIEFDAMPER a specialisation of Damper"^^xsd:string ;
    rdfs:seeAlso ifc:IfcDamperEnumType ;
    rdfs:subClassOf p4bldg:Damper .

p4bldg:Damper-SMOKEDAMPER a owl:Class ;
    rdfs:label "SMOKEDAMPER"^^xsd:string ;
    rdfs:comment "Describe products of class SMOKEDAMPER a specialisation of Damper"^^xsd:string ;
    rdfs:seeAlso ifc:IfcDamperEnumType ;
    rdfs:subClassOf p4bldg:Damper .

p4bldg:Damper-USERDEFINED a owl:Class ;
    rdfs:label "USERDEFINED"^^xsd:string ;
    rdfs:comment "Describe products of class USERDEFINED a specialisation of Damper"^^xsd:string ;
    rdfs:seeAlso ifc:IfcDamperEnumType ;
    rdfs:subClassOf p4bldg:Damper .

p4bldg:DiscreteAccessory-ANCHORPLATE a owl:Class ;
    rdfs:label "ANCHORPLATE"^^xsd:string ;
    rdfs:comment "Describe products of class ANCHORPLATE a specialisation of DiscreteAccessory"^^xsd:string ;
    rdfs:seeAlso ifc:IfcDiscreteAccessoryEnumType ;
    rdfs:subClassOf p4bldg:DiscreteAccessory .

p4bldg:DiscreteAccessory-BRACKET a owl:Class ;
    rdfs:label "BRACKET"^^xsd:string ;
    rdfs:comment "Describe products of class BRACKET a specialisation of DiscreteAccessory"^^xsd:string ;
    rdfs:seeAlso ifc:IfcDiscreteAccessoryEnumType ;
    rdfs:subClassOf p4bldg:DiscreteAccessory .

p4bldg:DiscreteAccessory-NOTDEFINED a owl:Class ;
    rdfs:label "NOTDEFINED"^^xsd:string ;
    rdfs:comment "Describe products of class NOTDEFINED a specialisation of DiscreteAccessory"^^xsd:string ;
    rdfs:seeAlso ifc:IfcDiscreteAccessoryEnumType ;
    rdfs:subClassOf p4bldg:DiscreteAccessory .

p4bldg:DiscreteAccessory-SHOE a owl:Class ;
    rdfs:label "SHOE"^^xsd:string ;
    rdfs:comment "Describe products of class SHOE a specialisation of DiscreteAccessory"^^xsd:string ;
    rdfs:seeAlso ifc:IfcDiscreteAccessoryEnumType ;
    rdfs:subClassOf p4bldg:DiscreteAccessory .

p4bldg:DiscreteAccessory-USERDEFINED a owl:Class ;
    rdfs:label "USERDEFINED"^^xsd:string ;
    rdfs:comment "Describe products of class USERDEFINED a specialisation of DiscreteAccessory"^^xsd:string ;
    rdfs:seeAlso ifc:IfcDiscreteAccessoryEnumType ;
    rdfs:subClassOf p4bldg:DiscreteAccessory .

p4bldg:DistributionChamberElement-FORMEDDUCT a owl:Class ;
    rdfs:label "FORMEDDUCT"^^xsd:string ;
    rdfs:comment "Describe products of class FORMEDDUCT a specialisation of DistributionChamberElement"^^xsd:string ;
    rdfs:seeAlso ifc:IfcDistributionChamberElementEnumType ;
    rdfs:subClassOf p4bldg:DistributionChamberElement .

p4bldg:DistributionChamberElement-INSPECTIONCHAMBER a owl:Class ;
    rdfs:label "INSPECTIONCHAMBER"^^xsd:string ;
    rdfs:comment "Describe products of class INSPECTIONCHAMBER a specialisation of DistributionChamberElement"^^xsd:string ;
    rdfs:seeAlso ifc:IfcDistributionChamberElementEnumType ;
    rdfs:subClassOf p4bldg:DistributionChamberElement .

p4bldg:DistributionChamberElement-INSPECTIONPIT a owl:Class ;
    rdfs:label "INSPECTIONPIT"^^xsd:string ;
    rdfs:comment "Describe products of class INSPECTIONPIT a specialisation of DistributionChamberElement"^^xsd:string ;
    rdfs:seeAlso ifc:IfcDistributionChamberElementEnumType ;
    rdfs:subClassOf p4bldg:DistributionChamberElement .

p4bldg:DistributionChamberElement-MANHOLE a owl:Class ;
    rdfs:label "MANHOLE"^^xsd:string ;
    rdfs:comment "Describe products of class MANHOLE a specialisation of DistributionChamberElement"^^xsd:string ;
    rdfs:seeAlso ifc:IfcDistributionChamberElementEnumType ;
    rdfs:subClassOf p4bldg:DistributionChamberElement .

p4bldg:DistributionChamberElement-METERCHAMBER a owl:Class ;
    rdfs:label "METERCHAMBER"^^xsd:string ;
    rdfs:comment "Describe products of class METERCHAMBER a specialisation of DistributionChamberElement"^^xsd:string ;
    rdfs:seeAlso ifc:IfcDistributionChamberElementEnumType ;
    rdfs:subClassOf p4bldg:DistributionChamberElement .

p4bldg:DistributionChamberElement-NOTDEFINED a owl:Class ;
    rdfs:label "NOTDEFINED"^^xsd:string ;
    rdfs:comment "Describe products of class NOTDEFINED a specialisation of DistributionChamberElement"^^xsd:string ;
    rdfs:seeAlso ifc:IfcDistributionChamberElementEnumType ;
    rdfs:subClassOf p4bldg:DistributionChamberElement .

p4bldg:DistributionChamberElement-SUMP a owl:Class ;
    rdfs:label "SUMP"^^xsd:string ;
    rdfs:comment "Describe products of class SUMP a specialisation of DistributionChamberElement"^^xsd:string ;
    rdfs:seeAlso ifc:IfcDistributionChamberElementEnumType ;
    rdfs:subClassOf p4bldg:DistributionChamberElement .

p4bldg:DistributionChamberElement-TRENCH a owl:Class ;
    rdfs:label "TRENCH"^^xsd:string ;
    rdfs:comment "Describe products of class TRENCH a specialisation of DistributionChamberElement"^^xsd:string ;
    rdfs:seeAlso ifc:IfcDistributionChamberElementEnumType ;
    rdfs:subClassOf p4bldg:DistributionChamberElement .

p4bldg:DistributionChamberElement-USERDEFINED a owl:Class ;
    rdfs:label "USERDEFINED"^^xsd:string ;
    rdfs:comment "Describe products of class USERDEFINED a specialisation of DistributionChamberElement"^^xsd:string ;
    rdfs:seeAlso ifc:IfcDistributionChamberElementEnumType ;
    rdfs:subClassOf p4bldg:DistributionChamberElement .

p4bldg:DistributionChamberElement-VALVECHAMBER a owl:Class ;
    rdfs:label "VALVECHAMBER"^^xsd:string ;
    rdfs:comment "Describe products of class VALVECHAMBER a specialisation of DistributionChamberElement"^^xsd:string ;
    rdfs:seeAlso ifc:IfcDistributionChamberElementEnumType ;
    rdfs:subClassOf p4bldg:DistributionChamberElement .

p4bldg:Door-DOOR a owl:Class ;
    rdfs:label "DOOR"^^xsd:string ;
    rdfs:comment "Describe products of class DOOR a specialisation of Door"^^xsd:string ;
    rdfs:seeAlso ifc:IfcDoorEnumType ;
    rdfs:subClassOf p4bldg:Door .

p4bldg:Door-GATE a owl:Class ;
    rdfs:label "GATE"^^xsd:string ;
    rdfs:comment "Describe products of class GATE a specialisation of Door"^^xsd:string ;
    rdfs:seeAlso ifc:IfcDoorEnumType ;
    rdfs:subClassOf p4bldg:Door .

p4bldg:Door-NOTDEFINED a owl:Class ;
    rdfs:label "NOTDEFINED"^^xsd:string ;
    rdfs:comment "Describe products of class NOTDEFINED a specialisation of Door"^^xsd:string ;
    rdfs:seeAlso ifc:IfcDoorEnumType ;
    rdfs:subClassOf p4bldg:Door .

p4bldg:Door-TRAPDOOR a owl:Class ;
    rdfs:label "TRAPDOOR"^^xsd:string ;
    rdfs:comment "Describe products of class TRAPDOOR a specialisation of Door"^^xsd:string ;
    rdfs:seeAlso ifc:IfcDoorEnumType ;
    rdfs:subClassOf p4bldg:Door .

p4bldg:Door-USERDEFINED a owl:Class ;
    rdfs:label "USERDEFINED"^^xsd:string ;
    rdfs:comment "Describe products of class USERDEFINED a specialisation of Door"^^xsd:string ;
    rdfs:seeAlso ifc:IfcDoorEnumType ;
    rdfs:subClassOf p4bldg:Door .

p4bldg:DoorStandardCase a owl:Class ;
    rdfs:label "DoorStandardCase"^^xsd:string ;
    rdfs:comment "Describe products of class DoorStandardCase"^^xsd:string ;
    rdfs:seeAlso ifc:IfcDoorStandardCase ;
    rdfs:subClassOf p4bldg:Door .

p4bldg:DuctFitting-BEND a owl:Class ;
    rdfs:label "BEND"^^xsd:string ;
    rdfs:comment "Describe products of class BEND a specialisation of DuctFitting"^^xsd:string ;
    rdfs:seeAlso ifc:IfcDuctFittingEnumType ;
    rdfs:subClassOf p4bldg:DuctFitting .

p4bldg:DuctFitting-CONNECTOR a owl:Class ;
    rdfs:label "CONNECTOR"^^xsd:string ;
    rdfs:comment "Describe products of class CONNECTOR a specialisation of DuctFitting"^^xsd:string ;
    rdfs:seeAlso ifc:IfcDuctFittingEnumType ;
    rdfs:subClassOf p4bldg:DuctFitting .

p4bldg:DuctFitting-ENTRY a owl:Class ;
    rdfs:label "ENTRY"^^xsd:string ;
    rdfs:comment "Describe products of class ENTRY a specialisation of DuctFitting"^^xsd:string ;
    rdfs:seeAlso ifc:IfcDuctFittingEnumType ;
    rdfs:subClassOf p4bldg:DuctFitting .

p4bldg:DuctFitting-EXIT a owl:Class ;
    rdfs:label "EXIT"^^xsd:string ;
    rdfs:comment "Describe products of class EXIT a specialisation of DuctFitting"^^xsd:string ;
    rdfs:seeAlso ifc:IfcDuctFittingEnumType ;
    rdfs:subClassOf p4bldg:DuctFitting .

p4bldg:DuctFitting-JUNCTION a owl:Class ;
    rdfs:label "JUNCTION"^^xsd:string ;
    rdfs:comment "Describe products of class JUNCTION a specialisation of DuctFitting"^^xsd:string ;
    rdfs:seeAlso ifc:IfcDuctFittingEnumType ;
    rdfs:subClassOf p4bldg:DuctFitting .

p4bldg:DuctFitting-NOTDEFINED a owl:Class ;
    rdfs:label "NOTDEFINED"^^xsd:string ;
    rdfs:comment "Describe products of class NOTDEFINED a specialisation of DuctFitting"^^xsd:string ;
    rdfs:seeAlso ifc:IfcDuctFittingEnumType ;
    rdfs:subClassOf p4bldg:DuctFitting .

p4bldg:DuctFitting-OBSTRUCTION a owl:Class ;
    rdfs:label "OBSTRUCTION"^^xsd:string ;
    rdfs:comment "Describe products of class OBSTRUCTION a specialisation of DuctFitting"^^xsd:string ;
    rdfs:seeAlso ifc:IfcDuctFittingEnumType ;
    rdfs:subClassOf p4bldg:DuctFitting .

p4bldg:DuctFitting-TRANSITION a owl:Class ;
    rdfs:label "TRANSITION"^^xsd:string ;
    rdfs:comment "Describe products of class TRANSITION a specialisation of DuctFitting"^^xsd:string ;
    rdfs:seeAlso ifc:IfcDuctFittingEnumType ;
    rdfs:subClassOf p4bldg:DuctFitting .

p4bldg:DuctFitting-USERDEFINED a owl:Class ;
    rdfs:label "USERDEFINED"^^xsd:string ;
    rdfs:comment "Describe products of class USERDEFINED a specialisation of DuctFitting"^^xsd:string ;
    rdfs:seeAlso ifc:IfcDuctFittingEnumType ;
    rdfs:subClassOf p4bldg:DuctFitting .

p4bldg:DuctSegment-FLEXIBLESEGMENT a owl:Class ;
    rdfs:label "FLEXIBLESEGMENT"^^xsd:string ;
    rdfs:comment "Describe products of class FLEXIBLESEGMENT a specialisation of DuctSegment"^^xsd:string ;
    rdfs:seeAlso ifc:IfcDuctSegmentEnumType ;
    rdfs:subClassOf p4bldg:DuctSegment .

p4bldg:DuctSegment-NOTDEFINED a owl:Class ;
    rdfs:label "NOTDEFINED"^^xsd:string ;
    rdfs:comment "Describe products of class NOTDEFINED a specialisation of DuctSegment"^^xsd:string ;
    rdfs:seeAlso ifc:IfcDuctSegmentEnumType ;
    rdfs:subClassOf p4bldg:DuctSegment .

p4bldg:DuctSegment-RIGIDSEGMENT a owl:Class ;
    rdfs:label "RIGIDSEGMENT"^^xsd:string ;
    rdfs:comment "Describe products of class RIGIDSEGMENT a specialisation of DuctSegment"^^xsd:string ;
    rdfs:seeAlso ifc:IfcDuctSegmentEnumType ;
    rdfs:subClassOf p4bldg:DuctSegment .

p4bldg:DuctSegment-USERDEFINED a owl:Class ;
    rdfs:label "USERDEFINED"^^xsd:string ;
    rdfs:comment "Describe products of class USERDEFINED a specialisation of DuctSegment"^^xsd:string ;
    rdfs:seeAlso ifc:IfcDuctSegmentEnumType ;
    rdfs:subClassOf p4bldg:DuctSegment .

p4bldg:DuctSilencer-FLATOVAL a owl:Class ;
    rdfs:label "FLATOVAL"^^xsd:string ;
    rdfs:comment "Describe products of class FLATOVAL a specialisation of DuctSilencer"^^xsd:string ;
    rdfs:seeAlso ifc:IfcDuctSilencerEnumType ;
    rdfs:subClassOf p4bldg:DuctSilencer .

p4bldg:DuctSilencer-NOTDEFINED a owl:Class ;
    rdfs:label "NOTDEFINED"^^xsd:string ;
    rdfs:comment "Describe products of class NOTDEFINED a specialisation of DuctSilencer"^^xsd:string ;
    rdfs:seeAlso ifc:IfcDuctSilencerEnumType ;
    rdfs:subClassOf p4bldg:DuctSilencer .

p4bldg:DuctSilencer-RECTANGULAR a owl:Class ;
    rdfs:label "RECTANGULAR"^^xsd:string ;
    rdfs:comment "Describe products of class RECTANGULAR a specialisation of DuctSilencer"^^xsd:string ;
    rdfs:seeAlso ifc:IfcDuctSilencerEnumType ;
    rdfs:subClassOf p4bldg:DuctSilencer .

p4bldg:DuctSilencer-ROUND a owl:Class ;
    rdfs:label "ROUND"^^xsd:string ;
    rdfs:comment "Describe products of class ROUND a specialisation of DuctSilencer"^^xsd:string ;
    rdfs:seeAlso ifc:IfcDuctSilencerEnumType ;
    rdfs:subClassOf p4bldg:DuctSilencer .

p4bldg:DuctSilencer-USERDEFINED a owl:Class ;
    rdfs:label "USERDEFINED"^^xsd:string ;
    rdfs:comment "Describe products of class USERDEFINED a specialisation of DuctSilencer"^^xsd:string ;
    rdfs:seeAlso ifc:IfcDuctSilencerEnumType ;
    rdfs:subClassOf p4bldg:DuctSilencer .

p4bldg:ElectricAppliance-DISHWASHER a owl:Class ;
    rdfs:label "DISHWASHER"^^xsd:string ;
    rdfs:comment "Describe products of class DISHWASHER a specialisation of ElectricAppliance"^^xsd:string ;
    rdfs:seeAlso ifc:IfcElectricApplianceEnumType ;
    rdfs:subClassOf p4bldg:ElectricAppliance .

p4bldg:ElectricAppliance-ELECTRICCOOKER a owl:Class ;
    rdfs:label "ELECTRICCOOKER"^^xsd:string ;
    rdfs:comment "Describe products of class ELECTRICCOOKER a specialisation of ElectricAppliance"^^xsd:string ;
    rdfs:seeAlso ifc:IfcElectricApplianceEnumType ;
    rdfs:subClassOf p4bldg:ElectricAppliance .

p4bldg:ElectricAppliance-FREESTANDINGELECTRICHEATER a owl:Class ;
    rdfs:label "FREESTANDINGELECTRICHEATER"^^xsd:string ;
    rdfs:comment "Describe products of class FREESTANDINGELECTRICHEATER a specialisation of ElectricAppliance"^^xsd:string ;
    rdfs:seeAlso ifc:IfcElectricApplianceEnumType ;
    rdfs:subClassOf p4bldg:ElectricAppliance .

p4bldg:ElectricAppliance-FREESTANDINGFAN a owl:Class ;
    rdfs:label "FREESTANDINGFAN"^^xsd:string ;
    rdfs:comment "Describe products of class FREESTANDINGFAN a specialisation of ElectricAppliance"^^xsd:string ;
    rdfs:seeAlso ifc:IfcElectricApplianceEnumType ;
    rdfs:subClassOf p4bldg:ElectricAppliance .

p4bldg:ElectricAppliance-FREESTANDINGWATERCOOLER a owl:Class ;
    rdfs:label "FREESTANDINGWATERCOOLER"^^xsd:string ;
    rdfs:comment "Describe products of class FREESTANDINGWATERCOOLER a specialisation of ElectricAppliance"^^xsd:string ;
    rdfs:seeAlso ifc:IfcElectricApplianceEnumType ;
    rdfs:subClassOf p4bldg:ElectricAppliance .

p4bldg:ElectricAppliance-FREESTANDINGWATERHEATER a owl:Class ;
    rdfs:label "FREESTANDINGWATERHEATER"^^xsd:string ;
    rdfs:comment "Describe products of class FREESTANDINGWATERHEATER a specialisation of ElectricAppliance"^^xsd:string ;
    rdfs:seeAlso ifc:IfcElectricApplianceEnumType ;
    rdfs:subClassOf p4bldg:ElectricAppliance .

p4bldg:ElectricAppliance-FREEZER a owl:Class ;
    rdfs:label "FREEZER"^^xsd:string ;
    rdfs:comment "Describe products of class FREEZER a specialisation of ElectricAppliance"^^xsd:string ;
    rdfs:seeAlso ifc:IfcElectricApplianceEnumType ;
    rdfs:subClassOf p4bldg:ElectricAppliance .

p4bldg:ElectricAppliance-FRIDGE_FREEZER a owl:Class ;
    rdfs:label "FRIDGE_FREEZER"^^xsd:string ;
    rdfs:comment "Describe products of class FRIDGE_FREEZER a specialisation of ElectricAppliance"^^xsd:string ;
    rdfs:seeAlso ifc:IfcElectricApplianceEnumType ;
    rdfs:subClassOf p4bldg:ElectricAppliance .

p4bldg:ElectricAppliance-HANDDRYER a owl:Class ;
    rdfs:label "HANDDRYER"^^xsd:string ;
    rdfs:comment "Describe products of class HANDDRYER a specialisation of ElectricAppliance"^^xsd:string ;
    rdfs:seeAlso ifc:IfcElectricApplianceEnumType ;
    rdfs:subClassOf p4bldg:ElectricAppliance .

p4bldg:ElectricAppliance-KITCHENMACHINE a owl:Class ;
    rdfs:label "KITCHENMACHINE"^^xsd:string ;
    rdfs:comment "Describe products of class KITCHENMACHINE a specialisation of ElectricAppliance"^^xsd:string ;
    rdfs:seeAlso ifc:IfcElectricApplianceEnumType ;
    rdfs:subClassOf p4bldg:ElectricAppliance .

p4bldg:ElectricAppliance-MICROWAVE a owl:Class ;
    rdfs:label "MICROWAVE"^^xsd:string ;
    rdfs:comment "Describe products of class MICROWAVE a specialisation of ElectricAppliance"^^xsd:string ;
    rdfs:seeAlso ifc:IfcElectricApplianceEnumType ;
    rdfs:subClassOf p4bldg:ElectricAppliance .

p4bldg:ElectricAppliance-NOTDEFINED a owl:Class ;
    rdfs:label "NOTDEFINED"^^xsd:string ;
    rdfs:comment "Describe products of class NOTDEFINED a specialisation of ElectricAppliance"^^xsd:string ;
    rdfs:seeAlso ifc:IfcElectricApplianceEnumType ;
    rdfs:subClassOf p4bldg:ElectricAppliance .

p4bldg:ElectricAppliance-PHOTOCOPIER a owl:Class ;
    rdfs:label "PHOTOCOPIER"^^xsd:string ;
    rdfs:comment "Describe products of class PHOTOCOPIER a specialisation of ElectricAppliance"^^xsd:string ;
    rdfs:seeAlso ifc:IfcElectricApplianceEnumType ;
    rdfs:subClassOf p4bldg:ElectricAppliance .

p4bldg:ElectricAppliance-REFRIGERATOR a owl:Class ;
    rdfs:label "REFRIGERATOR"^^xsd:string ;
    rdfs:comment "Describe products of class REFRIGERATOR a specialisation of ElectricAppliance"^^xsd:string ;
    rdfs:seeAlso ifc:IfcElectricApplianceEnumType ;
    rdfs:subClassOf p4bldg:ElectricAppliance .

p4bldg:ElectricAppliance-TUMBLEDRYER a owl:Class ;
    rdfs:label "TUMBLEDRYER"^^xsd:string ;
    rdfs:comment "Describe products of class TUMBLEDRYER a specialisation of ElectricAppliance"^^xsd:string ;
    rdfs:seeAlso ifc:IfcElectricApplianceEnumType ;
    rdfs:subClassOf p4bldg:ElectricAppliance .

p4bldg:ElectricAppliance-USERDEFINED a owl:Class ;
    rdfs:label "USERDEFINED"^^xsd:string ;
    rdfs:comment "Describe products of class USERDEFINED a specialisation of ElectricAppliance"^^xsd:string ;
    rdfs:seeAlso ifc:IfcElectricApplianceEnumType ;
    rdfs:subClassOf p4bldg:ElectricAppliance .

p4bldg:ElectricAppliance-VENDINGMACHINE a owl:Class ;
    rdfs:label "VENDINGMACHINE"^^xsd:string ;
    rdfs:comment "Describe products of class VENDINGMACHINE a specialisation of ElectricAppliance"^^xsd:string ;
    rdfs:seeAlso ifc:IfcElectricApplianceEnumType ;
    rdfs:subClassOf p4bldg:ElectricAppliance .

p4bldg:ElectricAppliance-WASHINGMACHINE a owl:Class ;
    rdfs:label "WASHINGMACHINE"^^xsd:string ;
    rdfs:comment "Describe products of class WASHINGMACHINE a specialisation of ElectricAppliance"^^xsd:string ;
    rdfs:seeAlso ifc:IfcElectricApplianceEnumType ;
    rdfs:subClassOf p4bldg:ElectricAppliance .

p4bldg:ElectricDistributionBoard-CONSUMERUNIT a owl:Class ;
    rdfs:label "CONSUMERUNIT"^^xsd:string ;
    rdfs:comment "Describe products of class CONSUMERUNIT a specialisation of ElectricDistributionBoard"^^xsd:string ;
    rdfs:seeAlso ifc:IfcElectricDistributionBoardEnumType ;
    rdfs:subClassOf p4bldg:ElectricDistributionBoard .

p4bldg:ElectricDistributionBoard-DISTRIBUTIONBOARD a owl:Class ;
    rdfs:label "DISTRIBUTIONBOARD"^^xsd:string ;
    rdfs:comment "Describe products of class DISTRIBUTIONBOARD a specialisation of ElectricDistributionBoard"^^xsd:string ;
    rdfs:seeAlso ifc:IfcElectricDistributionBoardEnumType ;
    rdfs:subClassOf p4bldg:ElectricDistributionBoard .

p4bldg:ElectricDistributionBoard-MOTORCONTROLCENTRE a owl:Class ;
    rdfs:label "MOTORCONTROLCENTRE"^^xsd:string ;
    rdfs:comment "Describe products of class MOTORCONTROLCENTRE a specialisation of ElectricDistributionBoard"^^xsd:string ;
    rdfs:seeAlso ifc:IfcElectricDistributionBoardEnumType ;
    rdfs:subClassOf p4bldg:ElectricDistributionBoard .

p4bldg:ElectricDistributionBoard-NOTDEFINED a owl:Class ;
    rdfs:label "NOTDEFINED"^^xsd:string ;
    rdfs:comment "Describe products of class NOTDEFINED a specialisation of ElectricDistributionBoard"^^xsd:string ;
    rdfs:seeAlso ifc:IfcElectricDistributionBoardEnumType ;
    rdfs:subClassOf p4bldg:ElectricDistributionBoard .

p4bldg:ElectricDistributionBoard-SWITCHBOARD a owl:Class ;
    rdfs:label "SWITCHBOARD"^^xsd:string ;
    rdfs:comment "Describe products of class SWITCHBOARD a specialisation of ElectricDistributionBoard"^^xsd:string ;
    rdfs:seeAlso ifc:IfcElectricDistributionBoardEnumType ;
    rdfs:subClassOf p4bldg:ElectricDistributionBoard .

p4bldg:ElectricDistributionBoard-USERDEFINED a owl:Class ;
    rdfs:label "USERDEFINED"^^xsd:string ;
    rdfs:comment "Describe products of class USERDEFINED a specialisation of ElectricDistributionBoard"^^xsd:string ;
    rdfs:seeAlso ifc:IfcElectricDistributionBoardEnumType ;
    rdfs:subClassOf p4bldg:ElectricDistributionBoard .

p4bldg:ElectricFlowStorageDevice-BATTERY a owl:Class ;
    rdfs:label "BATTERY"^^xsd:string ;
    rdfs:comment "Describe products of class BATTERY a specialisation of ElectricFlowStorageDevice"^^xsd:string ;
    rdfs:seeAlso ifc:IfcElectricFlowStorageDeviceEnumType ;
    rdfs:subClassOf p4bldg:ElectricFlowStorageDevice .

p4bldg:ElectricFlowStorageDevice-CAPACITORBANK a owl:Class ;
    rdfs:label "CAPACITORBANK"^^xsd:string ;
    rdfs:comment "Describe products of class CAPACITORBANK a specialisation of ElectricFlowStorageDevice"^^xsd:string ;
    rdfs:seeAlso ifc:IfcElectricFlowStorageDeviceEnumType ;
    rdfs:subClassOf p4bldg:ElectricFlowStorageDevice .

p4bldg:ElectricFlowStorageDevice-HARMONICFILTER a owl:Class ;
    rdfs:label "HARMONICFILTER"^^xsd:string ;
    rdfs:comment "Describe products of class HARMONICFILTER a specialisation of ElectricFlowStorageDevice"^^xsd:string ;
    rdfs:seeAlso ifc:IfcElectricFlowStorageDeviceEnumType ;
    rdfs:subClassOf p4bldg:ElectricFlowStorageDevice .

p4bldg:ElectricFlowStorageDevice-INDUCTORBANK a owl:Class ;
    rdfs:label "INDUCTORBANK"^^xsd:string ;
    rdfs:comment "Describe products of class INDUCTORBANK a specialisation of ElectricFlowStorageDevice"^^xsd:string ;
    rdfs:seeAlso ifc:IfcElectricFlowStorageDeviceEnumType ;
    rdfs:subClassOf p4bldg:ElectricFlowStorageDevice .

p4bldg:ElectricFlowStorageDevice-NOTDEFINED a owl:Class ;
    rdfs:label "NOTDEFINED"^^xsd:string ;
    rdfs:comment "Describe products of class NOTDEFINED a specialisation of ElectricFlowStorageDevice"^^xsd:string ;
    rdfs:seeAlso ifc:IfcElectricFlowStorageDeviceEnumType ;
    rdfs:subClassOf p4bldg:ElectricFlowStorageDevice .

p4bldg:ElectricFlowStorageDevice-UPS a owl:Class ;
    rdfs:label "UPS"^^xsd:string ;
    rdfs:comment "Describe products of class UPS a specialisation of ElectricFlowStorageDevice"^^xsd:string ;
    rdfs:seeAlso ifc:IfcElectricFlowStorageDeviceEnumType ;
    rdfs:subClassOf p4bldg:ElectricFlowStorageDevice .

p4bldg:ElectricFlowStorageDevice-USERDEFINED a owl:Class ;
    rdfs:label "USERDEFINED"^^xsd:string ;
    rdfs:comment "Describe products of class USERDEFINED a specialisation of ElectricFlowStorageDevice"^^xsd:string ;
    rdfs:seeAlso ifc:IfcElectricFlowStorageDeviceEnumType ;
    rdfs:subClassOf p4bldg:ElectricFlowStorageDevice .

p4bldg:ElectricGenerator-CHP a owl:Class ;
    rdfs:label "CHP"^^xsd:string ;
    rdfs:comment "Describe products of class CHP a specialisation of ElectricGenerator"^^xsd:string ;
    rdfs:seeAlso ifc:IfcElectricGeneratorEnumType ;
    rdfs:subClassOf p4bldg:ElectricGenerator .

p4bldg:ElectricGenerator-ENGINEGENERATOR a owl:Class ;
    rdfs:label "ENGINEGENERATOR"^^xsd:string ;
    rdfs:comment "Describe products of class ENGINEGENERATOR a specialisation of ElectricGenerator"^^xsd:string ;
    rdfs:seeAlso ifc:IfcElectricGeneratorEnumType ;
    rdfs:subClassOf p4bldg:ElectricGenerator .

p4bldg:ElectricGenerator-NOTDEFINED a owl:Class ;
    rdfs:label "NOTDEFINED"^^xsd:string ;
    rdfs:comment "Describe products of class NOTDEFINED a specialisation of ElectricGenerator"^^xsd:string ;
    rdfs:seeAlso ifc:IfcElectricGeneratorEnumType ;
    rdfs:subClassOf p4bldg:ElectricGenerator .

p4bldg:ElectricGenerator-STANDALONE a owl:Class ;
    rdfs:label "STANDALONE"^^xsd:string ;
    rdfs:comment "Describe products of class STANDALONE a specialisation of ElectricGenerator"^^xsd:string ;
    rdfs:seeAlso ifc:IfcElectricGeneratorEnumType ;
    rdfs:subClassOf p4bldg:ElectricGenerator .

p4bldg:ElectricGenerator-USERDEFINED a owl:Class ;
    rdfs:label "USERDEFINED"^^xsd:string ;
    rdfs:comment "Describe products of class USERDEFINED a specialisation of ElectricGenerator"^^xsd:string ;
    rdfs:seeAlso ifc:IfcElectricGeneratorEnumType ;
    rdfs:subClassOf p4bldg:ElectricGenerator .

p4bldg:ElectricMotor-DC a owl:Class ;
    rdfs:label "DC"^^xsd:string ;
    rdfs:comment "Describe products of class DC a specialisation of ElectricMotor"^^xsd:string ;
    rdfs:seeAlso ifc:IfcElectricMotorEnumType ;
    rdfs:subClassOf p4bldg:ElectricMotor .

p4bldg:ElectricMotor-INDUCTION a owl:Class ;
    rdfs:label "INDUCTION"^^xsd:string ;
    rdfs:comment "Describe products of class INDUCTION a specialisation of ElectricMotor"^^xsd:string ;
    rdfs:seeAlso ifc:IfcElectricMotorEnumType ;
    rdfs:subClassOf p4bldg:ElectricMotor .

p4bldg:ElectricMotor-NOTDEFINED a owl:Class ;
    rdfs:label "NOTDEFINED"^^xsd:string ;
    rdfs:comment "Describe products of class NOTDEFINED a specialisation of ElectricMotor"^^xsd:string ;
    rdfs:seeAlso ifc:IfcElectricMotorEnumType ;
    rdfs:subClassOf p4bldg:ElectricMotor .

p4bldg:ElectricMotor-POLYPHASE a owl:Class ;
    rdfs:label "POLYPHASE"^^xsd:string ;
    rdfs:comment "Describe products of class POLYPHASE a specialisation of ElectricMotor"^^xsd:string ;
    rdfs:seeAlso ifc:IfcElectricMotorEnumType ;
    rdfs:subClassOf p4bldg:ElectricMotor .

p4bldg:ElectricMotor-RELUCTANCESYNCHRONOUS a owl:Class ;
    rdfs:label "RELUCTANCESYNCHRONOUS"^^xsd:string ;
    rdfs:comment "Describe products of class RELUCTANCESYNCHRONOUS a specialisation of ElectricMotor"^^xsd:string ;
    rdfs:seeAlso ifc:IfcElectricMotorEnumType ;
    rdfs:subClassOf p4bldg:ElectricMotor .

p4bldg:ElectricMotor-SYNCHRONOUS a owl:Class ;
    rdfs:label "SYNCHRONOUS"^^xsd:string ;
    rdfs:comment "Describe products of class SYNCHRONOUS a specialisation of ElectricMotor"^^xsd:string ;
    rdfs:seeAlso ifc:IfcElectricMotorEnumType ;
    rdfs:subClassOf p4bldg:ElectricMotor .

p4bldg:ElectricMotor-USERDEFINED a owl:Class ;
    rdfs:label "USERDEFINED"^^xsd:string ;
    rdfs:comment "Describe products of class USERDEFINED a specialisation of ElectricMotor"^^xsd:string ;
    rdfs:seeAlso ifc:IfcElectricMotorEnumType ;
    rdfs:subClassOf p4bldg:ElectricMotor .

p4bldg:ElectricTimeControl-NOTDEFINED a owl:Class ;
    rdfs:label "NOTDEFINED"^^xsd:string ;
    rdfs:comment "Describe products of class NOTDEFINED a specialisation of ElectricTimeControl"^^xsd:string ;
    rdfs:seeAlso ifc:IfcElectricTimeControlEnumType ;
    rdfs:subClassOf p4bldg:ElectricTimeControl .

p4bldg:ElectricTimeControl-RELAY a owl:Class ;
    rdfs:label "RELAY"^^xsd:string ;
    rdfs:comment "Describe products of class RELAY a specialisation of ElectricTimeControl"^^xsd:string ;
    rdfs:seeAlso ifc:IfcElectricTimeControlEnumType ;
    rdfs:subClassOf p4bldg:ElectricTimeControl .

p4bldg:ElectricTimeControl-TIMECLOCK a owl:Class ;
    rdfs:label "TIMECLOCK"^^xsd:string ;
    rdfs:comment "Describe products of class TIMECLOCK a specialisation of ElectricTimeControl"^^xsd:string ;
    rdfs:seeAlso ifc:IfcElectricTimeControlEnumType ;
    rdfs:subClassOf p4bldg:ElectricTimeControl .

p4bldg:ElectricTimeControl-TIMEDELAY a owl:Class ;
    rdfs:label "TIMEDELAY"^^xsd:string ;
    rdfs:comment "Describe products of class TIMEDELAY a specialisation of ElectricTimeControl"^^xsd:string ;
    rdfs:seeAlso ifc:IfcElectricTimeControlEnumType ;
    rdfs:subClassOf p4bldg:ElectricTimeControl .

p4bldg:ElectricTimeControl-USERDEFINED a owl:Class ;
    rdfs:label "USERDEFINED"^^xsd:string ;
    rdfs:comment "Describe products of class USERDEFINED a specialisation of ElectricTimeControl"^^xsd:string ;
    rdfs:seeAlso ifc:IfcElectricTimeControlEnumType ;
    rdfs:subClassOf p4bldg:ElectricTimeControl .

p4bldg:ElementAssembly-ACCESSORY_ASSEMBLY a owl:Class ;
    rdfs:label "ACCESSORY_ASSEMBLY"^^xsd:string ;
    rdfs:comment "Describe products of class ACCESSORY_ASSEMBLY a specialisation of ElementAssembly"^^xsd:string ;
    rdfs:seeAlso ifc:IfcElementAssemblyEnumType ;
    rdfs:subClassOf p4bldg:ElementAssembly .

p4bldg:ElementAssembly-ARCH a owl:Class ;
    rdfs:label "ARCH"^^xsd:string ;
    rdfs:comment "Describe products of class ARCH a specialisation of ElementAssembly"^^xsd:string ;
    rdfs:seeAlso ifc:IfcElementAssemblyEnumType ;
    rdfs:subClassOf p4bldg:ElementAssembly .

p4bldg:ElementAssembly-BEAM_GRID a owl:Class ;
    rdfs:label "BEAM_GRID"^^xsd:string ;
    rdfs:comment "Describe products of class BEAM_GRID a specialisation of ElementAssembly"^^xsd:string ;
    rdfs:seeAlso ifc:IfcElementAssemblyEnumType ;
    rdfs:subClassOf p4bldg:ElementAssembly .

p4bldg:ElementAssembly-BRACED_FRAME a owl:Class ;
    rdfs:label "BRACED_FRAME"^^xsd:string ;
    rdfs:comment "Describe products of class BRACED_FRAME a specialisation of ElementAssembly"^^xsd:string ;
    rdfs:seeAlso ifc:IfcElementAssemblyEnumType ;
    rdfs:subClassOf p4bldg:ElementAssembly .

p4bldg:ElementAssembly-GIRDER a owl:Class ;
    rdfs:label "GIRDER"^^xsd:string ;
    rdfs:comment "Describe products of class GIRDER a specialisation of ElementAssembly"^^xsd:string ;
    rdfs:seeAlso ifc:IfcElementAssemblyEnumType ;
    rdfs:subClassOf p4bldg:ElementAssembly .

p4bldg:ElementAssembly-NOTDEFINED a owl:Class ;
    rdfs:label "NOTDEFINED"^^xsd:string ;
    rdfs:comment "Describe products of class NOTDEFINED a specialisation of ElementAssembly"^^xsd:string ;
    rdfs:seeAlso ifc:IfcElementAssemblyEnumType ;
    rdfs:subClassOf p4bldg:ElementAssembly .

p4bldg:ElementAssembly-REINFORCEMENT_UNIT a owl:Class ;
    rdfs:label "REINFORCEMENT_UNIT"^^xsd:string ;
    rdfs:comment "Describe products of class REINFORCEMENT_UNIT a specialisation of ElementAssembly"^^xsd:string ;
    rdfs:seeAlso ifc:IfcElementAssemblyEnumType ;
    rdfs:subClassOf p4bldg:ElementAssembly .

p4bldg:ElementAssembly-RIGID_FRAME a owl:Class ;
    rdfs:label "RIGID_FRAME"^^xsd:string ;
    rdfs:comment "Describe products of class RIGID_FRAME a specialisation of ElementAssembly"^^xsd:string ;
    rdfs:seeAlso ifc:IfcElementAssemblyEnumType ;
    rdfs:subClassOf p4bldg:ElementAssembly .

p4bldg:ElementAssembly-SLAB_FIELD a owl:Class ;
    rdfs:label "SLAB_FIELD"^^xsd:string ;
    rdfs:comment "Describe products of class SLAB_FIELD a specialisation of ElementAssembly"^^xsd:string ;
    rdfs:seeAlso ifc:IfcElementAssemblyEnumType ;
    rdfs:subClassOf p4bldg:ElementAssembly .

p4bldg:ElementAssembly-TRUSS a owl:Class ;
    rdfs:label "TRUSS"^^xsd:string ;
    rdfs:comment "Describe products of class TRUSS a specialisation of ElementAssembly"^^xsd:string ;
    rdfs:seeAlso ifc:IfcElementAssemblyEnumType ;
    rdfs:subClassOf p4bldg:ElementAssembly .

p4bldg:ElementAssembly-USERDEFINED a owl:Class ;
    rdfs:label "USERDEFINED"^^xsd:string ;
    rdfs:comment "Describe products of class USERDEFINED a specialisation of ElementAssembly"^^xsd:string ;
    rdfs:seeAlso ifc:IfcElementAssemblyEnumType ;
    rdfs:subClassOf p4bldg:ElementAssembly .

p4bldg:Engine-EXTERNALCOMBUSTION a owl:Class ;
    rdfs:label "EXTERNALCOMBUSTION"^^xsd:string ;
    rdfs:comment "Describe products of class EXTERNALCOMBUSTION a specialisation of Engine"^^xsd:string ;
    rdfs:seeAlso ifc:IfcEngineEnumType ;
    rdfs:subClassOf p4bldg:Engine .

p4bldg:Engine-INTERNALCOMBUSTION a owl:Class ;
    rdfs:label "INTERNALCOMBUSTION"^^xsd:string ;
    rdfs:comment "Describe products of class INTERNALCOMBUSTION a specialisation of Engine"^^xsd:string ;
    rdfs:seeAlso ifc:IfcEngineEnumType ;
    rdfs:subClassOf p4bldg:Engine .

p4bldg:Engine-NOTDEFINED a owl:Class ;
    rdfs:label "NOTDEFINED"^^xsd:string ;
    rdfs:comment "Describe products of class NOTDEFINED a specialisation of Engine"^^xsd:string ;
    rdfs:seeAlso ifc:IfcEngineEnumType ;
    rdfs:subClassOf p4bldg:Engine .

p4bldg:Engine-USERDEFINED a owl:Class ;
    rdfs:label "USERDEFINED"^^xsd:string ;
    rdfs:comment "Describe products of class USERDEFINED a specialisation of Engine"^^xsd:string ;
    rdfs:seeAlso ifc:IfcEngineEnumType ;
    rdfs:subClassOf p4bldg:Engine .

p4bldg:EvaporativeCooler-DIRECTEVAPORATIVEAIRWASHER a owl:Class ;
    rdfs:label "DIRECTEVAPORATIVEAIRWASHER"^^xsd:string ;
    rdfs:comment "Describe products of class DIRECTEVAPORATIVEAIRWASHER a specialisation of EvaporativeCooler"^^xsd:string ;
    rdfs:seeAlso ifc:IfcEvaporativeCoolerEnumType ;
    rdfs:subClassOf p4bldg:EvaporativeCooler .

p4bldg:EvaporativeCooler-DIRECTEVAPORATIVEPACKAGEDROTARYAIRCOOLER a owl:Class ;
    rdfs:label "DIRECTEVAPORATIVEPACKAGEDROTARYAIRCOOLER"^^xsd:string ;
    rdfs:comment "Describe products of class DIRECTEVAPORATIVEPACKAGEDROTARYAIRCOOLER a specialisation of EvaporativeCooler"^^xsd:string ;
    rdfs:seeAlso ifc:IfcEvaporativeCoolerEnumType ;
    rdfs:subClassOf p4bldg:EvaporativeCooler .

p4bldg:EvaporativeCooler-DIRECTEVAPORATIVERANDOMMEDIAAIRCOOLER a owl:Class ;
    rdfs:label "DIRECTEVAPORATIVERANDOMMEDIAAIRCOOLER"^^xsd:string ;
    rdfs:comment "Describe products of class DIRECTEVAPORATIVERANDOMMEDIAAIRCOOLER a specialisation of EvaporativeCooler"^^xsd:string ;
    rdfs:seeAlso ifc:IfcEvaporativeCoolerEnumType ;
    rdfs:subClassOf p4bldg:EvaporativeCooler .

p4bldg:EvaporativeCooler-DIRECTEVAPORATIVERIGIDMEDIAAIRCOOLER a owl:Class ;
    rdfs:label "DIRECTEVAPORATIVERIGIDMEDIAAIRCOOLER"^^xsd:string ;
    rdfs:comment "Describe products of class DIRECTEVAPORATIVERIGIDMEDIAAIRCOOLER a specialisation of EvaporativeCooler"^^xsd:string ;
    rdfs:seeAlso ifc:IfcEvaporativeCoolerEnumType ;
    rdfs:subClassOf p4bldg:EvaporativeCooler .

p4bldg:EvaporativeCooler-DIRECTEVAPORATIVESLINGERSPACKAGEDAIRCOOLER a owl:Class ;
    rdfs:label "DIRECTEVAPORATIVESLINGERSPACKAGEDAIRCOOLER"^^xsd:string ;
    rdfs:comment "Describe products of class DIRECTEVAPORATIVESLINGERSPACKAGEDAIRCOOLER a specialisation of EvaporativeCooler"^^xsd:string ;
    rdfs:seeAlso ifc:IfcEvaporativeCoolerEnumType ;
    rdfs:subClassOf p4bldg:EvaporativeCooler .

p4bldg:EvaporativeCooler-INDIRECTDIRECTCOMBINATION a owl:Class ;
    rdfs:label "INDIRECTDIRECTCOMBINATION"^^xsd:string ;
    rdfs:comment "Describe products of class INDIRECTDIRECTCOMBINATION a specialisation of EvaporativeCooler"^^xsd:string ;
    rdfs:seeAlso ifc:IfcEvaporativeCoolerEnumType ;
    rdfs:subClassOf p4bldg:EvaporativeCooler .

p4bldg:EvaporativeCooler-INDIRECTEVAPORATIVECOOLINGTOWERORCOILCOOLER a owl:Class ;
    rdfs:label "INDIRECTEVAPORATIVECOOLINGTOWERORCOILCOOLER"^^xsd:string ;
    rdfs:comment "Describe products of class INDIRECTEVAPORATIVECOOLINGTOWERORCOILCOOLER a specialisation of EvaporativeCooler"^^xsd:string ;
    rdfs:seeAlso ifc:IfcEvaporativeCoolerEnumType ;
    rdfs:subClassOf p4bldg:EvaporativeCooler .

p4bldg:EvaporativeCooler-INDIRECTEVAPORATIVEPACKAGEAIRCOOLER a owl:Class ;
    rdfs:label "INDIRECTEVAPORATIVEPACKAGEAIRCOOLER"^^xsd:string ;
    rdfs:comment "Describe products of class INDIRECTEVAPORATIVEPACKAGEAIRCOOLER a specialisation of EvaporativeCooler"^^xsd:string ;
    rdfs:seeAlso ifc:IfcEvaporativeCoolerEnumType ;
    rdfs:subClassOf p4bldg:EvaporativeCooler .

p4bldg:EvaporativeCooler-INDIRECTEVAPORATIVEWETCOIL a owl:Class ;
    rdfs:label "INDIRECTEVAPORATIVEWETCOIL"^^xsd:string ;
    rdfs:comment "Describe products of class INDIRECTEVAPORATIVEWETCOIL a specialisation of EvaporativeCooler"^^xsd:string ;
    rdfs:seeAlso ifc:IfcEvaporativeCoolerEnumType ;
    rdfs:subClassOf p4bldg:EvaporativeCooler .

p4bldg:EvaporativeCooler-NOTDEFINED a owl:Class ;
    rdfs:label "NOTDEFINED"^^xsd:string ;
    rdfs:comment "Describe products of class NOTDEFINED a specialisation of EvaporativeCooler"^^xsd:string ;
    rdfs:seeAlso ifc:IfcEvaporativeCoolerEnumType ;
    rdfs:subClassOf p4bldg:EvaporativeCooler .

p4bldg:EvaporativeCooler-USERDEFINED a owl:Class ;
    rdfs:label "USERDEFINED"^^xsd:string ;
    rdfs:comment "Describe products of class USERDEFINED a specialisation of EvaporativeCooler"^^xsd:string ;
    rdfs:seeAlso ifc:IfcEvaporativeCoolerEnumType ;
    rdfs:subClassOf p4bldg:EvaporativeCooler .

p4bldg:Evaporator-DIRECTEXPANSION a owl:Class ;
    rdfs:label "DIRECTEXPANSION"^^xsd:string ;
    rdfs:comment "Describe products of class DIRECTEXPANSION a specialisation of Evaporator"^^xsd:string ;
    rdfs:seeAlso ifc:IfcEvaporatorEnumType ;
    rdfs:subClassOf p4bldg:Evaporator .

p4bldg:Evaporator-DIRECTEXPANSIONBRAZEDPLATE a owl:Class ;
    rdfs:label "DIRECTEXPANSIONBRAZEDPLATE"^^xsd:string ;
    rdfs:comment "Describe products of class DIRECTEXPANSIONBRAZEDPLATE a specialisation of Evaporator"^^xsd:string ;
    rdfs:seeAlso ifc:IfcEvaporatorEnumType ;
    rdfs:subClassOf p4bldg:Evaporator .

p4bldg:Evaporator-DIRECTEXPANSIONSHELLANDTUBE a owl:Class ;
    rdfs:label "DIRECTEXPANSIONSHELLANDTUBE"^^xsd:string ;
    rdfs:comment "Describe products of class DIRECTEXPANSIONSHELLANDTUBE a specialisation of Evaporator"^^xsd:string ;
    rdfs:seeAlso ifc:IfcEvaporatorEnumType ;
    rdfs:subClassOf p4bldg:Evaporator .

p4bldg:Evaporator-DIRECTEXPANSIONTUBEINTUBE a owl:Class ;
    rdfs:label "DIRECTEXPANSIONTUBEINTUBE"^^xsd:string ;
    rdfs:comment "Describe products of class DIRECTEXPANSIONTUBEINTUBE a specialisation of Evaporator"^^xsd:string ;
    rdfs:seeAlso ifc:IfcEvaporatorEnumType ;
    rdfs:subClassOf p4bldg:Evaporator .

p4bldg:Evaporator-FLOODEDSHELLANDTUBE a owl:Class ;
    rdfs:label "FLOODEDSHELLANDTUBE"^^xsd:string ;
    rdfs:comment "Describe products of class FLOODEDSHELLANDTUBE a specialisation of Evaporator"^^xsd:string ;
    rdfs:seeAlso ifc:IfcEvaporatorEnumType ;
    rdfs:subClassOf p4bldg:Evaporator .

p4bldg:Evaporator-NOTDEFINED a owl:Class ;
    rdfs:label "NOTDEFINED"^^xsd:string ;
    rdfs:comment "Describe products of class NOTDEFINED a specialisation of Evaporator"^^xsd:string ;
    rdfs:seeAlso ifc:IfcEvaporatorEnumType ;
    rdfs:subClassOf p4bldg:Evaporator .

p4bldg:Evaporator-SHELLANDCOIL a owl:Class ;
    rdfs:label "SHELLANDCOIL"^^xsd:string ;
    rdfs:comment "Describe products of class SHELLANDCOIL a specialisation of Evaporator"^^xsd:string ;
    rdfs:seeAlso ifc:IfcEvaporatorEnumType ;
    rdfs:subClassOf p4bldg:Evaporator .

p4bldg:Evaporator-USERDEFINED a owl:Class ;
    rdfs:label "USERDEFINED"^^xsd:string ;
    rdfs:comment "Describe products of class USERDEFINED a specialisation of Evaporator"^^xsd:string ;
    rdfs:seeAlso ifc:IfcEvaporatorEnumType ;
    rdfs:subClassOf p4bldg:Evaporator .

p4bldg:Fan-CENTRIFUGALAIRFOIL a owl:Class ;
    rdfs:label "CENTRIFUGALAIRFOIL"^^xsd:string ;
    rdfs:comment "Describe products of class CENTRIFUGALAIRFOIL a specialisation of Fan"^^xsd:string ;
    rdfs:seeAlso ifc:IfcFanEnumType ;
    rdfs:subClassOf p4bldg:Fan .

p4bldg:Fan-CENTRIFUGALBACKWARDINCLINEDCURVED a owl:Class ;
    rdfs:label "CENTRIFUGALBACKWARDINCLINEDCURVED"^^xsd:string ;
    rdfs:comment "Describe products of class CENTRIFUGALBACKWARDINCLINEDCURVED a specialisation of Fan"^^xsd:string ;
    rdfs:seeAlso ifc:IfcFanEnumType ;
    rdfs:subClassOf p4bldg:Fan .

p4bldg:Fan-CENTRIFUGALFORWARDCURVED a owl:Class ;
    rdfs:label "CENTRIFUGALFORWARDCURVED"^^xsd:string ;
    rdfs:comment "Describe products of class CENTRIFUGALFORWARDCURVED a specialisation of Fan"^^xsd:string ;
    rdfs:seeAlso ifc:IfcFanEnumType ;
    rdfs:subClassOf p4bldg:Fan .

p4bldg:Fan-CENTRIFUGALRADIAL a owl:Class ;
    rdfs:label "CENTRIFUGALRADIAL"^^xsd:string ;
    rdfs:comment "Describe products of class CENTRIFUGALRADIAL a specialisation of Fan"^^xsd:string ;
    rdfs:seeAlso ifc:IfcFanEnumType ;
    rdfs:subClassOf p4bldg:Fan .

p4bldg:Fan-NOTDEFINED a owl:Class ;
    rdfs:label "NOTDEFINED"^^xsd:string ;
    rdfs:comment "Describe products of class NOTDEFINED a specialisation of Fan"^^xsd:string ;
    rdfs:seeAlso ifc:IfcFanEnumType ;
    rdfs:subClassOf p4bldg:Fan .

p4bldg:Fan-PROPELLORAXIAL a owl:Class ;
    rdfs:label "PROPELLORAXIAL"^^xsd:string ;
    rdfs:comment "Describe products of class PROPELLORAXIAL a specialisation of Fan"^^xsd:string ;
    rdfs:seeAlso ifc:IfcFanEnumType ;
    rdfs:subClassOf p4bldg:Fan .

p4bldg:Fan-TUBEAXIAL a owl:Class ;
    rdfs:label "TUBEAXIAL"^^xsd:string ;
    rdfs:comment "Describe products of class TUBEAXIAL a specialisation of Fan"^^xsd:string ;
    rdfs:seeAlso ifc:IfcFanEnumType ;
    rdfs:subClassOf p4bldg:Fan .

p4bldg:Fan-USERDEFINED a owl:Class ;
    rdfs:label "USERDEFINED"^^xsd:string ;
    rdfs:comment "Describe products of class USERDEFINED a specialisation of Fan"^^xsd:string ;
    rdfs:seeAlso ifc:IfcFanEnumType ;
    rdfs:subClassOf p4bldg:Fan .

p4bldg:Fan-VANEAXIAL a owl:Class ;
    rdfs:label "VANEAXIAL"^^xsd:string ;
    rdfs:comment "Describe products of class VANEAXIAL a specialisation of Fan"^^xsd:string ;
    rdfs:seeAlso ifc:IfcFanEnumType ;
    rdfs:subClassOf p4bldg:Fan .

p4bldg:Fastener-GLUE a owl:Class ;
    rdfs:label "GLUE"^^xsd:string ;
    rdfs:comment "Describe products of class GLUE a specialisation of Fastener"^^xsd:string ;
    rdfs:seeAlso ifc:IfcFastenerEnumType ;
    rdfs:subClassOf p4bldg:Fastener .

p4bldg:Fastener-MORTAR a owl:Class ;
    rdfs:label "MORTAR"^^xsd:string ;
    rdfs:comment "Describe products of class MORTAR a specialisation of Fastener"^^xsd:string ;
    rdfs:seeAlso ifc:IfcFastenerEnumType ;
    rdfs:subClassOf p4bldg:Fastener .

p4bldg:Fastener-NOTDEFINED a owl:Class ;
    rdfs:label "NOTDEFINED"^^xsd:string ;
    rdfs:comment "Describe products of class NOTDEFINED a specialisation of Fastener"^^xsd:string ;
    rdfs:seeAlso ifc:IfcFastenerEnumType ;
    rdfs:subClassOf p4bldg:Fastener .

p4bldg:Fastener-USERDEFINED a owl:Class ;
    rdfs:label "USERDEFINED"^^xsd:string ;
    rdfs:comment "Describe products of class USERDEFINED a specialisation of Fastener"^^xsd:string ;
    rdfs:seeAlso ifc:IfcFastenerEnumType ;
    rdfs:subClassOf p4bldg:Fastener .

p4bldg:Fastener-WELD a owl:Class ;
    rdfs:label "WELD"^^xsd:string ;
    rdfs:comment "Describe products of class WELD a specialisation of Fastener"^^xsd:string ;
    rdfs:seeAlso ifc:IfcFastenerEnumType ;
    rdfs:subClassOf p4bldg:Fastener .

p4bldg:Filter-AIRPARTICLEFILTER a owl:Class ;
    rdfs:label "AIRPARTICLEFILTER"^^xsd:string ;
    rdfs:comment "Describe products of class AIRPARTICLEFILTER a specialisation of Filter"^^xsd:string ;
    rdfs:seeAlso ifc:IfcFilterEnumType ;
    rdfs:subClassOf p4bldg:Filter .

p4bldg:Filter-COMPRESSEDAIRFILTER a owl:Class ;
    rdfs:label "COMPRESSEDAIRFILTER"^^xsd:string ;
    rdfs:comment "Describe products of class COMPRESSEDAIRFILTER a specialisation of Filter"^^xsd:string ;
    rdfs:seeAlso ifc:IfcFilterEnumType ;
    rdfs:subClassOf p4bldg:Filter .

p4bldg:Filter-NOTDEFINED a owl:Class ;
    rdfs:label "NOTDEFINED"^^xsd:string ;
    rdfs:comment "Describe products of class NOTDEFINED a specialisation of Filter"^^xsd:string ;
    rdfs:seeAlso ifc:IfcFilterEnumType ;
    rdfs:subClassOf p4bldg:Filter .

p4bldg:Filter-ODORFILTER a owl:Class ;
    rdfs:label "ODORFILTER"^^xsd:string ;
    rdfs:comment "Describe products of class ODORFILTER a specialisation of Filter"^^xsd:string ;
    rdfs:seeAlso ifc:IfcFilterEnumType ;
    rdfs:subClassOf p4bldg:Filter .

p4bldg:Filter-OILFILTER a owl:Class ;
    rdfs:label "OILFILTER"^^xsd:string ;
    rdfs:comment "Describe products of class OILFILTER a specialisation of Filter"^^xsd:string ;
    rdfs:seeAlso ifc:IfcFilterEnumType ;
    rdfs:subClassOf p4bldg:Filter .

p4bldg:Filter-STRAINER a owl:Class ;
    rdfs:label "STRAINER"^^xsd:string ;
    rdfs:comment "Describe products of class STRAINER a specialisation of Filter"^^xsd:string ;
    rdfs:seeAlso ifc:IfcFilterEnumType ;
    rdfs:subClassOf p4bldg:Filter .

p4bldg:Filter-USERDEFINED a owl:Class ;
    rdfs:label "USERDEFINED"^^xsd:string ;
    rdfs:comment "Describe products of class USERDEFINED a specialisation of Filter"^^xsd:string ;
    rdfs:seeAlso ifc:IfcFilterEnumType ;
    rdfs:subClassOf p4bldg:Filter .

p4bldg:Filter-WATERFILTER a owl:Class ;
    rdfs:label "WATERFILTER"^^xsd:string ;
    rdfs:comment "Describe products of class WATERFILTER a specialisation of Filter"^^xsd:string ;
    rdfs:seeAlso ifc:IfcFilterEnumType ;
    rdfs:subClassOf p4bldg:Filter .

p4bldg:FireSuppressionTerminal-BREECHINGINLET a owl:Class ;
    rdfs:label "BREECHINGINLET"^^xsd:string ;
    rdfs:comment "Describe products of class BREECHINGINLET a specialisation of FireSuppressionTerminal"^^xsd:string ;
    rdfs:seeAlso ifc:IfcFireSuppressionTerminalEnumType ;
    rdfs:subClassOf p4bldg:FireSuppressionTerminal .

p4bldg:FireSuppressionTerminal-FIREHYDRANT a owl:Class ;
    rdfs:label "FIREHYDRANT"^^xsd:string ;
    rdfs:comment "Describe products of class FIREHYDRANT a specialisation of FireSuppressionTerminal"^^xsd:string ;
    rdfs:seeAlso ifc:IfcFireSuppressionTerminalEnumType ;
    rdfs:subClassOf p4bldg:FireSuppressionTerminal .

p4bldg:FireSuppressionTerminal-HOSEREEL a owl:Class ;
    rdfs:label "HOSEREEL"^^xsd:string ;
    rdfs:comment "Describe products of class HOSEREEL a specialisation of FireSuppressionTerminal"^^xsd:string ;
    rdfs:seeAlso ifc:IfcFireSuppressionTerminalEnumType ;
    rdfs:subClassOf p4bldg:FireSuppressionTerminal .

p4bldg:FireSuppressionTerminal-NOTDEFINED a owl:Class ;
    rdfs:label "NOTDEFINED"^^xsd:string ;
    rdfs:comment "Describe products of class NOTDEFINED a specialisation of FireSuppressionTerminal"^^xsd:string ;
    rdfs:seeAlso ifc:IfcFireSuppressionTerminalEnumType ;
    rdfs:subClassOf p4bldg:FireSuppressionTerminal .

p4bldg:FireSuppressionTerminal-SPRINKLER a owl:Class ;
    rdfs:label "SPRINKLER"^^xsd:string ;
    rdfs:comment "Describe products of class SPRINKLER a specialisation of FireSuppressionTerminal"^^xsd:string ;
    rdfs:seeAlso ifc:IfcFireSuppressionTerminalEnumType ;
    rdfs:subClassOf p4bldg:FireSuppressionTerminal .

p4bldg:FireSuppressionTerminal-SPRINKLERDEFLECTOR a owl:Class ;
    rdfs:label "SPRINKLERDEFLECTOR"^^xsd:string ;
    rdfs:comment "Describe products of class SPRINKLERDEFLECTOR a specialisation of FireSuppressionTerminal"^^xsd:string ;
    rdfs:seeAlso ifc:IfcFireSuppressionTerminalEnumType ;
    rdfs:subClassOf p4bldg:FireSuppressionTerminal .

p4bldg:FireSuppressionTerminal-USERDEFINED a owl:Class ;
    rdfs:label "USERDEFINED"^^xsd:string ;
    rdfs:comment "Describe products of class USERDEFINED a specialisation of FireSuppressionTerminal"^^xsd:string ;
    rdfs:seeAlso ifc:IfcFireSuppressionTerminalEnumType ;
    rdfs:subClassOf p4bldg:FireSuppressionTerminal .

p4bldg:FlowInstrument-AMMETER a owl:Class ;
    rdfs:label "AMMETER"^^xsd:string ;
    rdfs:comment "Describe products of class AMMETER a specialisation of FlowInstrument"^^xsd:string ;
    rdfs:seeAlso ifc:IfcFlowInstrumentEnumType ;
    rdfs:subClassOf p4bldg:FlowInstrument .

p4bldg:FlowInstrument-FREQUENCYMETER a owl:Class ;
    rdfs:label "FREQUENCYMETER"^^xsd:string ;
    rdfs:comment "Describe products of class FREQUENCYMETER a specialisation of FlowInstrument"^^xsd:string ;
    rdfs:seeAlso ifc:IfcFlowInstrumentEnumType ;
    rdfs:subClassOf p4bldg:FlowInstrument .

p4bldg:FlowInstrument-NOTDEFINED a owl:Class ;
    rdfs:label "NOTDEFINED"^^xsd:string ;
    rdfs:comment "Describe products of class NOTDEFINED a specialisation of FlowInstrument"^^xsd:string ;
    rdfs:seeAlso ifc:IfcFlowInstrumentEnumType ;
    rdfs:subClassOf p4bldg:FlowInstrument .

p4bldg:FlowInstrument-PHASEANGLEMETER a owl:Class ;
    rdfs:label "PHASEANGLEMETER"^^xsd:string ;
    rdfs:comment "Describe products of class PHASEANGLEMETER a specialisation of FlowInstrument"^^xsd:string ;
    rdfs:seeAlso ifc:IfcFlowInstrumentEnumType ;
    rdfs:subClassOf p4bldg:FlowInstrument .

p4bldg:FlowInstrument-POWERFACTORMETER a owl:Class ;
    rdfs:label "POWERFACTORMETER"^^xsd:string ;
    rdfs:comment "Describe products of class POWERFACTORMETER a specialisation of FlowInstrument"^^xsd:string ;
    rdfs:seeAlso ifc:IfcFlowInstrumentEnumType ;
    rdfs:subClassOf p4bldg:FlowInstrument .

p4bldg:FlowInstrument-PRESSUREGAUGE a owl:Class ;
    rdfs:label "PRESSUREGAUGE"^^xsd:string ;
    rdfs:comment "Describe products of class PRESSUREGAUGE a specialisation of FlowInstrument"^^xsd:string ;
    rdfs:seeAlso ifc:IfcFlowInstrumentEnumType ;
    rdfs:subClassOf p4bldg:FlowInstrument .

p4bldg:FlowInstrument-THERMOMETER a owl:Class ;
    rdfs:label "THERMOMETER"^^xsd:string ;
    rdfs:comment "Describe products of class THERMOMETER a specialisation of FlowInstrument"^^xsd:string ;
    rdfs:seeAlso ifc:IfcFlowInstrumentEnumType ;
    rdfs:subClassOf p4bldg:FlowInstrument .

p4bldg:FlowInstrument-USERDEFINED a owl:Class ;
    rdfs:label "USERDEFINED"^^xsd:string ;
    rdfs:comment "Describe products of class USERDEFINED a specialisation of FlowInstrument"^^xsd:string ;
    rdfs:seeAlso ifc:IfcFlowInstrumentEnumType ;
    rdfs:subClassOf p4bldg:FlowInstrument .

p4bldg:FlowInstrument-VOLTMETER_PEAK a owl:Class ;
    rdfs:label "VOLTMETER_PEAK"^^xsd:string ;
    rdfs:comment "Describe products of class VOLTMETER_PEAK a specialisation of FlowInstrument"^^xsd:string ;
    rdfs:seeAlso ifc:IfcFlowInstrumentEnumType ;
    rdfs:subClassOf p4bldg:FlowInstrument .

p4bldg:FlowInstrument-VOLTMETER_RMS a owl:Class ;
    rdfs:label "VOLTMETER_RMS"^^xsd:string ;
    rdfs:comment "Describe products of class VOLTMETER_RMS a specialisation of FlowInstrument"^^xsd:string ;
    rdfs:seeAlso ifc:IfcFlowInstrumentEnumType ;
    rdfs:subClassOf p4bldg:FlowInstrument .

p4bldg:FlowMeter-ENERGYMETER a owl:Class ;
    rdfs:label "ENERGYMETER"^^xsd:string ;
    rdfs:comment "Describe products of class ENERGYMETER a specialisation of FlowMeter"^^xsd:string ;
    rdfs:seeAlso ifc:IfcFlowMeterEnumType ;
    rdfs:subClassOf p4bldg:FlowMeter .

p4bldg:FlowMeter-GASMETER a owl:Class ;
    rdfs:label "GASMETER"^^xsd:string ;
    rdfs:comment "Describe products of class GASMETER a specialisation of FlowMeter"^^xsd:string ;
    rdfs:seeAlso ifc:IfcFlowMeterEnumType ;
    rdfs:subClassOf p4bldg:FlowMeter .

p4bldg:FlowMeter-NOTDEFINED a owl:Class ;
    rdfs:label "NOTDEFINED"^^xsd:string ;
    rdfs:comment "Describe products of class NOTDEFINED a specialisation of FlowMeter"^^xsd:string ;
    rdfs:seeAlso ifc:IfcFlowMeterEnumType ;
    rdfs:subClassOf p4bldg:FlowMeter .

p4bldg:FlowMeter-OILMETER a owl:Class ;
    rdfs:label "OILMETER"^^xsd:string ;
    rdfs:comment "Describe products of class OILMETER a specialisation of FlowMeter"^^xsd:string ;
    rdfs:seeAlso ifc:IfcFlowMeterEnumType ;
    rdfs:subClassOf p4bldg:FlowMeter .

p4bldg:FlowMeter-USERDEFINED a owl:Class ;
    rdfs:label "USERDEFINED"^^xsd:string ;
    rdfs:comment "Describe products of class USERDEFINED a specialisation of FlowMeter"^^xsd:string ;
    rdfs:seeAlso ifc:IfcFlowMeterEnumType ;
    rdfs:subClassOf p4bldg:FlowMeter .

p4bldg:FlowMeter-WATERMETER a owl:Class ;
    rdfs:label "WATERMETER"^^xsd:string ;
    rdfs:comment "Describe products of class WATERMETER a specialisation of FlowMeter"^^xsd:string ;
    rdfs:seeAlso ifc:IfcFlowMeterEnumType ;
    rdfs:subClassOf p4bldg:FlowMeter .

p4bldg:Footing-CAISSON_FOUNDATION a owl:Class ;
    rdfs:label "CAISSON_FOUNDATION"^^xsd:string ;
    rdfs:comment "Describe products of class CAISSON_FOUNDATION a specialisation of Footing"^^xsd:string ;
    rdfs:seeAlso ifc:IfcFootingEnumType ;
    rdfs:subClassOf p4bldg:Footing .

p4bldg:Footing-FOOTING_BEAM a owl:Class ;
    rdfs:label "FOOTING_BEAM"^^xsd:string ;
    rdfs:comment "Describe products of class FOOTING_BEAM a specialisation of Footing"^^xsd:string ;
    rdfs:seeAlso ifc:IfcFootingEnumType ;
    rdfs:subClassOf p4bldg:Footing .

p4bldg:Footing-NOTDEFINED a owl:Class ;
    rdfs:label "NOTDEFINED"^^xsd:string ;
    rdfs:comment "Describe products of class NOTDEFINED a specialisation of Footing"^^xsd:string ;
    rdfs:seeAlso ifc:IfcFootingEnumType ;
    rdfs:subClassOf p4bldg:Footing .

p4bldg:Footing-PAD_FOOTING a owl:Class ;
    rdfs:label "PAD_FOOTING"^^xsd:string ;
    rdfs:comment "Describe products of class PAD_FOOTING a specialisation of Footing"^^xsd:string ;
    rdfs:seeAlso ifc:IfcFootingEnumType ;
    rdfs:subClassOf p4bldg:Footing .

p4bldg:Footing-PILE_CAP a owl:Class ;
    rdfs:label "PILE_CAP"^^xsd:string ;
    rdfs:comment "Describe products of class PILE_CAP a specialisation of Footing"^^xsd:string ;
    rdfs:seeAlso ifc:IfcFootingEnumType ;
    rdfs:subClassOf p4bldg:Footing .

p4bldg:Footing-STRIP_FOOTING a owl:Class ;
    rdfs:label "STRIP_FOOTING"^^xsd:string ;
    rdfs:comment "Describe products of class STRIP_FOOTING a specialisation of Footing"^^xsd:string ;
    rdfs:seeAlso ifc:IfcFootingEnumType ;
    rdfs:subClassOf p4bldg:Footing .

p4bldg:Footing-USERDEFINED a owl:Class ;
    rdfs:label "USERDEFINED"^^xsd:string ;
    rdfs:comment "Describe products of class USERDEFINED a specialisation of Footing"^^xsd:string ;
    rdfs:seeAlso ifc:IfcFootingEnumType ;
    rdfs:subClassOf p4bldg:Footing .

p4bldg:Furniture-BED a owl:Class ;
    rdfs:label "BED"^^xsd:string ;
    rdfs:comment "Describe products of class BED a specialisation of Furniture"^^xsd:string ;
    rdfs:seeAlso ifc:IfcFurnitureEnumType ;
    rdfs:subClassOf p4bldg:Furniture .

p4bldg:Furniture-CHAIR a owl:Class ;
    rdfs:label "CHAIR"^^xsd:string ;
    rdfs:comment "Describe products of class CHAIR a specialisation of Furniture"^^xsd:string ;
    rdfs:seeAlso ifc:IfcFurnitureEnumType ;
    rdfs:subClassOf p4bldg:Furniture .

p4bldg:Furniture-DESK a owl:Class ;
    rdfs:label "DESK"^^xsd:string ;
    rdfs:comment "Describe products of class DESK a specialisation of Furniture"^^xsd:string ;
    rdfs:seeAlso ifc:IfcFurnitureEnumType ;
    rdfs:subClassOf p4bldg:Furniture .

p4bldg:Furniture-FILECABINET a owl:Class ;
    rdfs:label "FILECABINET"^^xsd:string ;
    rdfs:comment "Describe products of class FILECABINET a specialisation of Furniture"^^xsd:string ;
    rdfs:seeAlso ifc:IfcFurnitureEnumType ;
    rdfs:subClassOf p4bldg:Furniture .

p4bldg:Furniture-NOTDEFINED a owl:Class ;
    rdfs:label "NOTDEFINED"^^xsd:string ;
    rdfs:comment "Describe products of class NOTDEFINED a specialisation of Furniture"^^xsd:string ;
    rdfs:seeAlso ifc:IfcFurnitureEnumType ;
    rdfs:subClassOf p4bldg:Furniture .

p4bldg:Furniture-SHELF a owl:Class ;
    rdfs:label "SHELF"^^xsd:string ;
    rdfs:comment "Describe products of class SHELF a specialisation of Furniture"^^xsd:string ;
    rdfs:seeAlso ifc:IfcFurnitureEnumType ;
    rdfs:subClassOf p4bldg:Furniture .

p4bldg:Furniture-SOFA a owl:Class ;
    rdfs:label "SOFA"^^xsd:string ;
    rdfs:comment "Describe products of class SOFA a specialisation of Furniture"^^xsd:string ;
    rdfs:seeAlso ifc:IfcFurnitureEnumType ;
    rdfs:subClassOf p4bldg:Furniture .

p4bldg:Furniture-TABLE a owl:Class ;
    rdfs:label "TABLE"^^xsd:string ;
    rdfs:comment "Describe products of class TABLE a specialisation of Furniture"^^xsd:string ;
    rdfs:seeAlso ifc:IfcFurnitureEnumType ;
    rdfs:subClassOf p4bldg:Furniture .

p4bldg:Furniture-USERDEFINED a owl:Class ;
    rdfs:label "USERDEFINED"^^xsd:string ;
    rdfs:comment "Describe products of class USERDEFINED a specialisation of Furniture"^^xsd:string ;
    rdfs:seeAlso ifc:IfcFurnitureEnumType ;
    rdfs:subClassOf p4bldg:Furniture .

p4bldg:GeographicElement-NOTDEFINED a owl:Class ;
    rdfs:label "NOTDEFINED"^^xsd:string ;
    rdfs:comment "Describe products of class NOTDEFINED a specialisation of GeographicElement"^^xsd:string ;
    rdfs:seeAlso ifc:IfcGeographicElementEnumType ;
    rdfs:subClassOf p4bldg:GeographicElement .

p4bldg:GeographicElement-TERRAIN a owl:Class ;
    rdfs:label "TERRAIN"^^xsd:string ;
    rdfs:comment "Describe products of class TERRAIN a specialisation of GeographicElement"^^xsd:string ;
    rdfs:seeAlso ifc:IfcGeographicElementEnumType ;
    rdfs:subClassOf p4bldg:GeographicElement .

p4bldg:GeographicElement-USERDEFINED a owl:Class ;
    rdfs:label "USERDEFINED"^^xsd:string ;
    rdfs:comment "Describe products of class USERDEFINED a specialisation of GeographicElement"^^xsd:string ;
    rdfs:seeAlso ifc:IfcGeographicElementEnumType ;
    rdfs:subClassOf p4bldg:GeographicElement .

p4bldg:HeatExchanger-NOTDEFINED a owl:Class ;
    rdfs:label "NOTDEFINED"^^xsd:string ;
    rdfs:comment "Describe products of class NOTDEFINED a specialisation of HeatExchanger"^^xsd:string ;
    rdfs:seeAlso ifc:IfcHeatExchangerEnumType ;
    rdfs:subClassOf p4bldg:HeatExchanger .

p4bldg:HeatExchanger-PLATE a owl:Class ;
    rdfs:label "PLATE"^^xsd:string ;
    rdfs:comment "Describe products of class PLATE a specialisation of HeatExchanger"^^xsd:string ;
    rdfs:seeAlso ifc:IfcHeatExchangerEnumType ;
    rdfs:subClassOf p4bldg:HeatExchanger .

p4bldg:HeatExchanger-SHELLANDTUBE a owl:Class ;
    rdfs:label "SHELLANDTUBE"^^xsd:string ;
    rdfs:comment "Describe products of class SHELLANDTUBE a specialisation of HeatExchanger"^^xsd:string ;
    rdfs:seeAlso ifc:IfcHeatExchangerEnumType ;
    rdfs:subClassOf p4bldg:HeatExchanger .

p4bldg:HeatExchanger-USERDEFINED a owl:Class ;
    rdfs:label "USERDEFINED"^^xsd:string ;
    rdfs:comment "Describe products of class USERDEFINED a specialisation of HeatExchanger"^^xsd:string ;
    rdfs:seeAlso ifc:IfcHeatExchangerEnumType ;
    rdfs:subClassOf p4bldg:HeatExchanger .

p4bldg:Humidifier-ADIABATICAIRWASHER a owl:Class ;
    rdfs:label "ADIABATICAIRWASHER"^^xsd:string ;
    rdfs:comment "Describe products of class ADIABATICAIRWASHER a specialisation of Humidifier"^^xsd:string ;
    rdfs:seeAlso ifc:IfcHumidifierEnumType ;
    rdfs:subClassOf p4bldg:Humidifier .

p4bldg:Humidifier-ADIABATICATOMIZING a owl:Class ;
    rdfs:label "ADIABATICATOMIZING"^^xsd:string ;
    rdfs:comment "Describe products of class ADIABATICATOMIZING a specialisation of Humidifier"^^xsd:string ;
    rdfs:seeAlso ifc:IfcHumidifierEnumType ;
    rdfs:subClassOf p4bldg:Humidifier .

p4bldg:Humidifier-ADIABATICCOMPRESSEDAIRNOZZLE a owl:Class ;
    rdfs:label "ADIABATICCOMPRESSEDAIRNOZZLE"^^xsd:string ;
    rdfs:comment "Describe products of class ADIABATICCOMPRESSEDAIRNOZZLE a specialisation of Humidifier"^^xsd:string ;
    rdfs:seeAlso ifc:IfcHumidifierEnumType ;
    rdfs:subClassOf p4bldg:Humidifier .

p4bldg:Humidifier-ADIABATICPAN a owl:Class ;
    rdfs:label "ADIABATICPAN"^^xsd:string ;
    rdfs:comment "Describe products of class ADIABATICPAN a specialisation of Humidifier"^^xsd:string ;
    rdfs:seeAlso ifc:IfcHumidifierEnumType ;
    rdfs:subClassOf p4bldg:Humidifier .

p4bldg:Humidifier-ADIABATICRIGIDMEDIA a owl:Class ;
    rdfs:label "ADIABATICRIGIDMEDIA"^^xsd:string ;
    rdfs:comment "Describe products of class ADIABATICRIGIDMEDIA a specialisation of Humidifier"^^xsd:string ;
    rdfs:seeAlso ifc:IfcHumidifierEnumType ;
    rdfs:subClassOf p4bldg:Humidifier .

p4bldg:Humidifier-ADIABATICULTRASONIC a owl:Class ;
    rdfs:label "ADIABATICULTRASONIC"^^xsd:string ;
    rdfs:comment "Describe products of class ADIABATICULTRASONIC a specialisation of Humidifier"^^xsd:string ;
    rdfs:seeAlso ifc:IfcHumidifierEnumType ;
    rdfs:subClassOf p4bldg:Humidifier .

p4bldg:Humidifier-ADIABATICWETTEDELEMENT a owl:Class ;
    rdfs:label "ADIABATICWETTEDELEMENT"^^xsd:string ;
    rdfs:comment "Describe products of class ADIABATICWETTEDELEMENT a specialisation of Humidifier"^^xsd:string ;
    rdfs:seeAlso ifc:IfcHumidifierEnumType ;
    rdfs:subClassOf p4bldg:Humidifier .

p4bldg:Humidifier-ASSISTEDBUTANE a owl:Class ;
    rdfs:label "ASSISTEDBUTANE"^^xsd:string ;
    rdfs:comment "Describe products of class ASSISTEDBUTANE a specialisation of Humidifier"^^xsd:string ;
    rdfs:seeAlso ifc:IfcHumidifierEnumType ;
    rdfs:subClassOf p4bldg:Humidifier .

p4bldg:Humidifier-ASSISTEDELECTRIC a owl:Class ;
    rdfs:label "ASSISTEDELECTRIC"^^xsd:string ;
    rdfs:comment "Describe products of class ASSISTEDELECTRIC a specialisation of Humidifier"^^xsd:string ;
    rdfs:seeAlso ifc:IfcHumidifierEnumType ;
    rdfs:subClassOf p4bldg:Humidifier .

p4bldg:Humidifier-ASSISTEDNATURALGAS a owl:Class ;
    rdfs:label "ASSISTEDNATURALGAS"^^xsd:string ;
    rdfs:comment "Describe products of class ASSISTEDNATURALGAS a specialisation of Humidifier"^^xsd:string ;
    rdfs:seeAlso ifc:IfcHumidifierEnumType ;
    rdfs:subClassOf p4bldg:Humidifier .

p4bldg:Humidifier-ASSISTEDPROPANE a owl:Class ;
    rdfs:label "ASSISTEDPROPANE"^^xsd:string ;
    rdfs:comment "Describe products of class ASSISTEDPROPANE a specialisation of Humidifier"^^xsd:string ;
    rdfs:seeAlso ifc:IfcHumidifierEnumType ;
    rdfs:subClassOf p4bldg:Humidifier .

p4bldg:Humidifier-ASSISTEDSTEAM a owl:Class ;
    rdfs:label "ASSISTEDSTEAM"^^xsd:string ;
    rdfs:comment "Describe products of class ASSISTEDSTEAM a specialisation of Humidifier"^^xsd:string ;
    rdfs:seeAlso ifc:IfcHumidifierEnumType ;
    rdfs:subClassOf p4bldg:Humidifier .

p4bldg:Humidifier-NOTDEFINED a owl:Class ;
    rdfs:label "NOTDEFINED"^^xsd:string ;
    rdfs:comment "Describe products of class NOTDEFINED a specialisation of Humidifier"^^xsd:string ;
    rdfs:seeAlso ifc:IfcHumidifierEnumType ;
    rdfs:subClassOf p4bldg:Humidifier .

p4bldg:Humidifier-STEAMINJECTION a owl:Class ;
    rdfs:label "STEAMINJECTION"^^xsd:string ;
    rdfs:comment "Describe products of class STEAMINJECTION a specialisation of Humidifier"^^xsd:string ;
    rdfs:seeAlso ifc:IfcHumidifierEnumType ;
    rdfs:subClassOf p4bldg:Humidifier .

p4bldg:Humidifier-USERDEFINED a owl:Class ;
    rdfs:label "USERDEFINED"^^xsd:string ;
    rdfs:comment "Describe products of class USERDEFINED a specialisation of Humidifier"^^xsd:string ;
    rdfs:seeAlso ifc:IfcHumidifierEnumType ;
    rdfs:subClassOf p4bldg:Humidifier .

p4bldg:Interceptor-CYCLONIC a owl:Class ;
    rdfs:label "CYCLONIC"^^xsd:string ;
    rdfs:comment "Describe products of class CYCLONIC a specialisation of Interceptor"^^xsd:string ;
    rdfs:seeAlso ifc:IfcInterceptorEnumType ;
    rdfs:subClassOf p4bldg:Interceptor .

p4bldg:Interceptor-GREASE a owl:Class ;
    rdfs:label "GREASE"^^xsd:string ;
    rdfs:comment "Describe products of class GREASE a specialisation of Interceptor"^^xsd:string ;
    rdfs:seeAlso ifc:IfcInterceptorEnumType ;
    rdfs:subClassOf p4bldg:Interceptor .

p4bldg:Interceptor-NOTDEFINED a owl:Class ;
    rdfs:label "NOTDEFINED"^^xsd:string ;
    rdfs:comment "Describe products of class NOTDEFINED a specialisation of Interceptor"^^xsd:string ;
    rdfs:seeAlso ifc:IfcInterceptorEnumType ;
    rdfs:subClassOf p4bldg:Interceptor .

p4bldg:Interceptor-OIL a owl:Class ;
    rdfs:label "OIL"^^xsd:string ;
    rdfs:comment "Describe products of class OIL a specialisation of Interceptor"^^xsd:string ;
    rdfs:seeAlso ifc:IfcInterceptorEnumType ;
    rdfs:subClassOf p4bldg:Interceptor .

p4bldg:Interceptor-PETROL a owl:Class ;
    rdfs:label "PETROL"^^xsd:string ;
    rdfs:comment "Describe products of class PETROL a specialisation of Interceptor"^^xsd:string ;
    rdfs:seeAlso ifc:IfcInterceptorEnumType ;
    rdfs:subClassOf p4bldg:Interceptor .

p4bldg:Interceptor-USERDEFINED a owl:Class ;
    rdfs:label "USERDEFINED"^^xsd:string ;
    rdfs:comment "Describe products of class USERDEFINED a specialisation of Interceptor"^^xsd:string ;
    rdfs:seeAlso ifc:IfcInterceptorEnumType ;
    rdfs:subClassOf p4bldg:Interceptor .

p4bldg:JunctionBox-DATA a owl:Class ;
    rdfs:label "DATA"^^xsd:string ;
    rdfs:comment "Describe products of class DATA a specialisation of JunctionBox"^^xsd:string ;
    rdfs:seeAlso ifc:IfcJunctionBoxEnumType ;
    rdfs:subClassOf p4bldg:JunctionBox .

p4bldg:JunctionBox-NOTDEFINED a owl:Class ;
    rdfs:label "NOTDEFINED"^^xsd:string ;
    rdfs:comment "Describe products of class NOTDEFINED a specialisation of JunctionBox"^^xsd:string ;
    rdfs:seeAlso ifc:IfcJunctionBoxEnumType ;
    rdfs:subClassOf p4bldg:JunctionBox .

p4bldg:JunctionBox-POWER a owl:Class ;
    rdfs:label "POWER"^^xsd:string ;
    rdfs:comment "Describe products of class POWER a specialisation of JunctionBox"^^xsd:string ;
    rdfs:seeAlso ifc:IfcJunctionBoxEnumType ;
    rdfs:subClassOf p4bldg:JunctionBox .

p4bldg:JunctionBox-USERDEFINED a owl:Class ;
    rdfs:label "USERDEFINED"^^xsd:string ;
    rdfs:comment "Describe products of class USERDEFINED a specialisation of JunctionBox"^^xsd:string ;
    rdfs:seeAlso ifc:IfcJunctionBoxEnumType ;
    rdfs:subClassOf p4bldg:JunctionBox .

p4bldg:Lamp-COMPACTFLUORESCENT a owl:Class ;
    rdfs:label "COMPACTFLUORESCENT"^^xsd:string ;
    rdfs:comment "Describe products of class COMPACTFLUORESCENT a specialisation of Lamp"^^xsd:string ;
    rdfs:seeAlso ifc:IfcLampEnumType ;
    rdfs:subClassOf p4bldg:Lamp .

p4bldg:Lamp-FLUORESCENT a owl:Class ;
    rdfs:label "FLUORESCENT"^^xsd:string ;
    rdfs:comment "Describe products of class FLUORESCENT a specialisation of Lamp"^^xsd:string ;
    rdfs:seeAlso ifc:IfcLampEnumType ;
    rdfs:subClassOf p4bldg:Lamp .

p4bldg:Lamp-HALOGEN a owl:Class ;
    rdfs:label "HALOGEN"^^xsd:string ;
    rdfs:comment "Describe products of class HALOGEN a specialisation of Lamp"^^xsd:string ;
    rdfs:seeAlso ifc:IfcLampEnumType ;
    rdfs:subClassOf p4bldg:Lamp .

p4bldg:Lamp-HIGHPRESSUREMERCURY a owl:Class ;
    rdfs:label "HIGHPRESSUREMERCURY"^^xsd:string ;
    rdfs:comment "Describe products of class HIGHPRESSUREMERCURY a specialisation of Lamp"^^xsd:string ;
    rdfs:seeAlso ifc:IfcLampEnumType ;
    rdfs:subClassOf p4bldg:Lamp .

p4bldg:Lamp-HIGHPRESSURESODIUM a owl:Class ;
    rdfs:label "HIGHPRESSURESODIUM"^^xsd:string ;
    rdfs:comment "Describe products of class HIGHPRESSURESODIUM a specialisation of Lamp"^^xsd:string ;
    rdfs:seeAlso ifc:IfcLampEnumType ;
    rdfs:subClassOf p4bldg:Lamp .

p4bldg:Lamp-LED a owl:Class ;
    rdfs:label "LED"^^xsd:string ;
    rdfs:comment "Describe products of class LED a specialisation of Lamp"^^xsd:string ;
    rdfs:seeAlso ifc:IfcLampEnumType ;
    rdfs:subClassOf p4bldg:Lamp .

p4bldg:Lamp-METALHALIDE a owl:Class ;
    rdfs:label "METALHALIDE"^^xsd:string ;
    rdfs:comment "Describe products of class METALHALIDE a specialisation of Lamp"^^xsd:string ;
    rdfs:seeAlso ifc:IfcLampEnumType ;
    rdfs:subClassOf p4bldg:Lamp .

p4bldg:Lamp-NOTDEFINED a owl:Class ;
    rdfs:label "NOTDEFINED"^^xsd:string ;
    rdfs:comment "Describe products of class NOTDEFINED a specialisation of Lamp"^^xsd:string ;
    rdfs:seeAlso ifc:IfcLampEnumType ;
    rdfs:subClassOf p4bldg:Lamp .

p4bldg:Lamp-OLED a owl:Class ;
    rdfs:label "OLED"^^xsd:string ;
    rdfs:comment "Describe products of class OLED a specialisation of Lamp"^^xsd:string ;
    rdfs:seeAlso ifc:IfcLampEnumType ;
    rdfs:subClassOf p4bldg:Lamp .

p4bldg:Lamp-TUNGSTENFILAMENT a owl:Class ;
    rdfs:label "TUNGSTENFILAMENT"^^xsd:string ;
    rdfs:comment "Describe products of class TUNGSTENFILAMENT a specialisation of Lamp"^^xsd:string ;
    rdfs:seeAlso ifc:IfcLampEnumType ;
    rdfs:subClassOf p4bldg:Lamp .

p4bldg:Lamp-USERDEFINED a owl:Class ;
    rdfs:label "USERDEFINED"^^xsd:string ;
    rdfs:comment "Describe products of class USERDEFINED a specialisation of Lamp"^^xsd:string ;
    rdfs:seeAlso ifc:IfcLampEnumType ;
    rdfs:subClassOf p4bldg:Lamp .

p4bldg:LightFixture-DIRECTIONSOURCE a owl:Class ;
    rdfs:label "DIRECTIONSOURCE"^^xsd:string ;
    rdfs:comment "Describe products of class DIRECTIONSOURCE a specialisation of LightFixture"^^xsd:string ;
    rdfs:seeAlso ifc:IfcLightFixtureEnumType ;
    rdfs:subClassOf p4bldg:LightFixture .

p4bldg:LightFixture-NOTDEFINED a owl:Class ;
    rdfs:label "NOTDEFINED"^^xsd:string ;
    rdfs:comment "Describe products of class NOTDEFINED a specialisation of LightFixture"^^xsd:string ;
    rdfs:seeAlso ifc:IfcLightFixtureEnumType ;
    rdfs:subClassOf p4bldg:LightFixture .

p4bldg:LightFixture-POINTSOURCE a owl:Class ;
    rdfs:label "POINTSOURCE"^^xsd:string ;
    rdfs:comment "Describe products of class POINTSOURCE a specialisation of LightFixture"^^xsd:string ;
    rdfs:seeAlso ifc:IfcLightFixtureEnumType ;
    rdfs:subClassOf p4bldg:LightFixture .

p4bldg:LightFixture-SECURITYLIGHTING a owl:Class ;
    rdfs:label "SECURITYLIGHTING"^^xsd:string ;
    rdfs:comment "Describe products of class SECURITYLIGHTING a specialisation of LightFixture"^^xsd:string ;
    rdfs:seeAlso ifc:IfcLightFixtureEnumType ;
    rdfs:subClassOf p4bldg:LightFixture .

p4bldg:LightFixture-USERDEFINED a owl:Class ;
    rdfs:label "USERDEFINED"^^xsd:string ;
    rdfs:comment "Describe products of class USERDEFINED a specialisation of LightFixture"^^xsd:string ;
    rdfs:seeAlso ifc:IfcLightFixtureEnumType ;
    rdfs:subClassOf p4bldg:LightFixture .

p4bldg:MechanicalFastener-ANCHORBOLT a owl:Class ;
    rdfs:label "ANCHORBOLT"^^xsd:string ;
    rdfs:comment "Describe products of class ANCHORBOLT a specialisation of MechanicalFastener"^^xsd:string ;
    rdfs:seeAlso ifc:IfcMechanicalFastenerEnumType ;
    rdfs:subClassOf p4bldg:MechanicalFastener .

p4bldg:MechanicalFastener-BOLT a owl:Class ;
    rdfs:label "BOLT"^^xsd:string ;
    rdfs:comment "Describe products of class BOLT a specialisation of MechanicalFastener"^^xsd:string ;
    rdfs:seeAlso ifc:IfcMechanicalFastenerEnumType ;
    rdfs:subClassOf p4bldg:MechanicalFastener .

p4bldg:MechanicalFastener-DOWEL a owl:Class ;
    rdfs:label "DOWEL"^^xsd:string ;
    rdfs:comment "Describe products of class DOWEL a specialisation of MechanicalFastener"^^xsd:string ;
    rdfs:seeAlso ifc:IfcMechanicalFastenerEnumType ;
    rdfs:subClassOf p4bldg:MechanicalFastener .

p4bldg:MechanicalFastener-NAIL a owl:Class ;
    rdfs:label "NAIL"^^xsd:string ;
    rdfs:comment "Describe products of class NAIL a specialisation of MechanicalFastener"^^xsd:string ;
    rdfs:seeAlso ifc:IfcMechanicalFastenerEnumType ;
    rdfs:subClassOf p4bldg:MechanicalFastener .

p4bldg:MechanicalFastener-NAILPLATE a owl:Class ;
    rdfs:label "NAILPLATE"^^xsd:string ;
    rdfs:comment "Describe products of class NAILPLATE a specialisation of MechanicalFastener"^^xsd:string ;
    rdfs:seeAlso ifc:IfcMechanicalFastenerEnumType ;
    rdfs:subClassOf p4bldg:MechanicalFastener .

p4bldg:MechanicalFastener-NOTDEFINED a owl:Class ;
    rdfs:label "NOTDEFINED"^^xsd:string ;
    rdfs:comment "Describe products of class NOTDEFINED a specialisation of MechanicalFastener"^^xsd:string ;
    rdfs:seeAlso ifc:IfcMechanicalFastenerEnumType ;
    rdfs:subClassOf p4bldg:MechanicalFastener .

p4bldg:MechanicalFastener-RIVET a owl:Class ;
    rdfs:label "RIVET"^^xsd:string ;
    rdfs:comment "Describe products of class RIVET a specialisation of MechanicalFastener"^^xsd:string ;
    rdfs:seeAlso ifc:IfcMechanicalFastenerEnumType ;
    rdfs:subClassOf p4bldg:MechanicalFastener .

p4bldg:MechanicalFastener-SCREW a owl:Class ;
    rdfs:label "SCREW"^^xsd:string ;
    rdfs:comment "Describe products of class SCREW a specialisation of MechanicalFastener"^^xsd:string ;
    rdfs:seeAlso ifc:IfcMechanicalFastenerEnumType ;
    rdfs:subClassOf p4bldg:MechanicalFastener .

p4bldg:MechanicalFastener-SHEARCONNECTOR a owl:Class ;
    rdfs:label "SHEARCONNECTOR"^^xsd:string ;
    rdfs:comment "Describe products of class SHEARCONNECTOR a specialisation of MechanicalFastener"^^xsd:string ;
    rdfs:seeAlso ifc:IfcMechanicalFastenerEnumType ;
    rdfs:subClassOf p4bldg:MechanicalFastener .

p4bldg:MechanicalFastener-STAPLE a owl:Class ;
    rdfs:label "STAPLE"^^xsd:string ;
    rdfs:comment "Describe products of class STAPLE a specialisation of MechanicalFastener"^^xsd:string ;
    rdfs:seeAlso ifc:IfcMechanicalFastenerEnumType ;
    rdfs:subClassOf p4bldg:MechanicalFastener .

p4bldg:MechanicalFastener-STUDSHEARCONNECTOR a owl:Class ;
    rdfs:label "STUDSHEARCONNECTOR"^^xsd:string ;
    rdfs:comment "Describe products of class STUDSHEARCONNECTOR a specialisation of MechanicalFastener"^^xsd:string ;
    rdfs:seeAlso ifc:IfcMechanicalFastenerEnumType ;
    rdfs:subClassOf p4bldg:MechanicalFastener .

p4bldg:MechanicalFastener-USERDEFINED a owl:Class ;
    rdfs:label "USERDEFINED"^^xsd:string ;
    rdfs:comment "Describe products of class USERDEFINED a specialisation of MechanicalFastener"^^xsd:string ;
    rdfs:seeAlso ifc:IfcMechanicalFastenerEnumType ;
    rdfs:subClassOf p4bldg:MechanicalFastener .

p4bldg:MedicalDevice-AIRSTATION a owl:Class ;
    rdfs:label "AIRSTATION"^^xsd:string ;
    rdfs:comment "Describe products of class AIRSTATION a specialisation of MedicalDevice"^^xsd:string ;
    rdfs:seeAlso ifc:IfcMedicalDeviceEnumType ;
    rdfs:subClassOf p4bldg:MedicalDevice .

p4bldg:MedicalDevice-FEEDAIRUNIT a owl:Class ;
    rdfs:label "FEEDAIRUNIT"^^xsd:string ;
    rdfs:comment "Describe products of class FEEDAIRUNIT a specialisation of MedicalDevice"^^xsd:string ;
    rdfs:seeAlso ifc:IfcMedicalDeviceEnumType ;
    rdfs:subClassOf p4bldg:MedicalDevice .

p4bldg:MedicalDevice-NOTDEFINED a owl:Class ;
    rdfs:label "NOTDEFINED"^^xsd:string ;
    rdfs:comment "Describe products of class NOTDEFINED a specialisation of MedicalDevice"^^xsd:string ;
    rdfs:seeAlso ifc:IfcMedicalDeviceEnumType ;
    rdfs:subClassOf p4bldg:MedicalDevice .

p4bldg:MedicalDevice-OXYGENGENERATOR a owl:Class ;
    rdfs:label "OXYGENGENERATOR"^^xsd:string ;
    rdfs:comment "Describe products of class OXYGENGENERATOR a specialisation of MedicalDevice"^^xsd:string ;
    rdfs:seeAlso ifc:IfcMedicalDeviceEnumType ;
    rdfs:subClassOf p4bldg:MedicalDevice .

p4bldg:MedicalDevice-OXYGENPLANT a owl:Class ;
    rdfs:label "OXYGENPLANT"^^xsd:string ;
    rdfs:comment "Describe products of class OXYGENPLANT a specialisation of MedicalDevice"^^xsd:string ;
    rdfs:seeAlso ifc:IfcMedicalDeviceEnumType ;
    rdfs:subClassOf p4bldg:MedicalDevice .

p4bldg:MedicalDevice-USERDEFINED a owl:Class ;
    rdfs:label "USERDEFINED"^^xsd:string ;
    rdfs:comment "Describe products of class USERDEFINED a specialisation of MedicalDevice"^^xsd:string ;
    rdfs:seeAlso ifc:IfcMedicalDeviceEnumType ;
    rdfs:subClassOf p4bldg:MedicalDevice .

p4bldg:MedicalDevice-VACUUMSTATION a owl:Class ;
    rdfs:label "VACUUMSTATION"^^xsd:string ;
    rdfs:comment "Describe products of class VACUUMSTATION a specialisation of MedicalDevice"^^xsd:string ;
    rdfs:seeAlso ifc:IfcMedicalDeviceEnumType ;
    rdfs:subClassOf p4bldg:MedicalDevice .

p4bldg:Member-BRACE a owl:Class ;
    rdfs:label "BRACE"^^xsd:string ;
    rdfs:comment "Describe products of class BRACE a specialisation of Member"^^xsd:string ;
    rdfs:seeAlso ifc:IfcMemberEnumType ;
    rdfs:subClassOf p4bldg:Member .

p4bldg:Member-CHORD a owl:Class ;
    rdfs:label "CHORD"^^xsd:string ;
    rdfs:comment "Describe products of class CHORD a specialisation of Member"^^xsd:string ;
    rdfs:seeAlso ifc:IfcMemberEnumType ;
    rdfs:subClassOf p4bldg:Member .

p4bldg:Member-COLLAR a owl:Class ;
    rdfs:label "COLLAR"^^xsd:string ;
    rdfs:comment "Describe products of class COLLAR a specialisation of Member"^^xsd:string ;
    rdfs:seeAlso ifc:IfcMemberEnumType ;
    rdfs:subClassOf p4bldg:Member .

p4bldg:Member-MEMBER a owl:Class ;
    rdfs:label "MEMBER"^^xsd:string ;
    rdfs:comment "Describe products of class MEMBER a specialisation of Member"^^xsd:string ;
    rdfs:seeAlso ifc:IfcMemberEnumType ;
    rdfs:subClassOf p4bldg:Member .

p4bldg:Member-MULLION a owl:Class ;
    rdfs:label "MULLION"^^xsd:string ;
    rdfs:comment "Describe products of class MULLION a specialisation of Member"^^xsd:string ;
    rdfs:seeAlso ifc:IfcMemberEnumType ;
    rdfs:subClassOf p4bldg:Member .

p4bldg:Member-NOTDEFINED a owl:Class ;
    rdfs:label "NOTDEFINED"^^xsd:string ;
    rdfs:comment "Describe products of class NOTDEFINED a specialisation of Member"^^xsd:string ;
    rdfs:seeAlso ifc:IfcMemberEnumType ;
    rdfs:subClassOf p4bldg:Member .

p4bldg:Member-PLATE a owl:Class ;
    rdfs:label "PLATE"^^xsd:string ;
    rdfs:comment "Describe products of class PLATE a specialisation of Member"^^xsd:string ;
    rdfs:seeAlso ifc:IfcMemberEnumType ;
    rdfs:subClassOf p4bldg:Member .

p4bldg:Member-POST a owl:Class ;
    rdfs:label "POST"^^xsd:string ;
    rdfs:comment "Describe products of class POST a specialisation of Member"^^xsd:string ;
    rdfs:seeAlso ifc:IfcMemberEnumType ;
    rdfs:subClassOf p4bldg:Member .

p4bldg:Member-PURLIN a owl:Class ;
    rdfs:label "PURLIN"^^xsd:string ;
    rdfs:comment "Describe products of class PURLIN a specialisation of Member"^^xsd:string ;
    rdfs:seeAlso ifc:IfcMemberEnumType ;
    rdfs:subClassOf p4bldg:Member .

p4bldg:Member-RAFTER a owl:Class ;
    rdfs:label "RAFTER"^^xsd:string ;
    rdfs:comment "Describe products of class RAFTER a specialisation of Member"^^xsd:string ;
    rdfs:seeAlso ifc:IfcMemberEnumType ;
    rdfs:subClassOf p4bldg:Member .

p4bldg:Member-STRINGER a owl:Class ;
    rdfs:label "STRINGER"^^xsd:string ;
    rdfs:comment "Describe products of class STRINGER a specialisation of Member"^^xsd:string ;
    rdfs:seeAlso ifc:IfcMemberEnumType ;
    rdfs:subClassOf p4bldg:Member .

p4bldg:Member-STRUT a owl:Class ;
    rdfs:label "STRUT"^^xsd:string ;
    rdfs:comment "Describe products of class STRUT a specialisation of Member"^^xsd:string ;
    rdfs:seeAlso ifc:IfcMemberEnumType ;
    rdfs:subClassOf p4bldg:Member .

p4bldg:Member-STUD a owl:Class ;
    rdfs:label "STUD"^^xsd:string ;
    rdfs:comment "Describe products of class STUD a specialisation of Member"^^xsd:string ;
    rdfs:seeAlso ifc:IfcMemberEnumType ;
    rdfs:subClassOf p4bldg:Member .

p4bldg:Member-USERDEFINED a owl:Class ;
    rdfs:label "USERDEFINED"^^xsd:string ;
    rdfs:comment "Describe products of class USERDEFINED a specialisation of Member"^^xsd:string ;
    rdfs:seeAlso ifc:IfcMemberEnumType ;
    rdfs:subClassOf p4bldg:Member .

p4bldg:MemberStandardCase a owl:Class ;
    rdfs:label "MemberStandardCase"^^xsd:string ;
    rdfs:comment "Describe products of class MemberStandardCase"^^xsd:string ;
    rdfs:seeAlso ifc:IfcMemberStandardCase ;
    rdfs:subClassOf p4bldg:Member .

p4bldg:MotorConnection-BELTDRIVE a owl:Class ;
    rdfs:label "BELTDRIVE"^^xsd:string ;
    rdfs:comment "Describe products of class BELTDRIVE a specialisation of MotorConnection"^^xsd:string ;
    rdfs:seeAlso ifc:IfcMotorConnectionEnumType ;
    rdfs:subClassOf p4bldg:MotorConnection .

p4bldg:MotorConnection-COUPLING a owl:Class ;
    rdfs:label "COUPLING"^^xsd:string ;
    rdfs:comment "Describe products of class COUPLING a specialisation of MotorConnection"^^xsd:string ;
    rdfs:seeAlso ifc:IfcMotorConnectionEnumType ;
    rdfs:subClassOf p4bldg:MotorConnection .

p4bldg:MotorConnection-DIRECTDRIVE a owl:Class ;
    rdfs:label "DIRECTDRIVE"^^xsd:string ;
    rdfs:comment "Describe products of class DIRECTDRIVE a specialisation of MotorConnection"^^xsd:string ;
    rdfs:seeAlso ifc:IfcMotorConnectionEnumType ;
    rdfs:subClassOf p4bldg:MotorConnection .

p4bldg:MotorConnection-NOTDEFINED a owl:Class ;
    rdfs:label "NOTDEFINED"^^xsd:string ;
    rdfs:comment "Describe products of class NOTDEFINED a specialisation of MotorConnection"^^xsd:string ;
    rdfs:seeAlso ifc:IfcMotorConnectionEnumType ;
    rdfs:subClassOf p4bldg:MotorConnection .

p4bldg:MotorConnection-USERDEFINED a owl:Class ;
    rdfs:label "USERDEFINED"^^xsd:string ;
    rdfs:comment "Describe products of class USERDEFINED a specialisation of MotorConnection"^^xsd:string ;
    rdfs:seeAlso ifc:IfcMotorConnectionEnumType ;
    rdfs:subClassOf p4bldg:MotorConnection .

p4bldg:None a owl:Class .

p4bldg:OpeningElement-NOTDEFINED a owl:Class ;
    rdfs:label "NOTDEFINED"^^xsd:string ;
    rdfs:comment "Describe products of class NOTDEFINED a specialisation of OpeningElement"^^xsd:string ;
    rdfs:seeAlso ifc:IfcOpeningElementEnumType ;
    rdfs:subClassOf p4bldg:OpeningElement .

p4bldg:OpeningElement-OPENING a owl:Class ;
    rdfs:label "OPENING"^^xsd:string ;
    rdfs:comment "Describe products of class OPENING a specialisation of OpeningElement"^^xsd:string ;
    rdfs:seeAlso ifc:IfcOpeningElementEnumType ;
    rdfs:subClassOf p4bldg:OpeningElement .

p4bldg:OpeningElement-RECESS a owl:Class ;
    rdfs:label "RECESS"^^xsd:string ;
    rdfs:comment "Describe products of class RECESS a specialisation of OpeningElement"^^xsd:string ;
    rdfs:seeAlso ifc:IfcOpeningElementEnumType ;
    rdfs:subClassOf p4bldg:OpeningElement .

p4bldg:OpeningElement-USERDEFINED a owl:Class ;
    rdfs:label "USERDEFINED"^^xsd:string ;
    rdfs:comment "Describe products of class USERDEFINED a specialisation of OpeningElement"^^xsd:string ;
    rdfs:seeAlso ifc:IfcOpeningElementEnumType ;
    rdfs:subClassOf p4bldg:OpeningElement .

p4bldg:OpeningStandardCase a owl:Class ;
    rdfs:label "OpeningStandardCase"^^xsd:string ;
    rdfs:comment "Describe products of class OpeningStandardCase"^^xsd:string ;
    rdfs:seeAlso ifc:IfcOpeningStandardCase ;
    rdfs:subClassOf p4bldg:OpeningElement .

p4bldg:Outlet-AUDIOVISUALOUTLET a owl:Class ;
    rdfs:label "AUDIOVISUALOUTLET"^^xsd:string ;
    rdfs:comment "Describe products of class AUDIOVISUALOUTLET a specialisation of Outlet"^^xsd:string ;
    rdfs:seeAlso ifc:IfcOutletEnumType ;
    rdfs:subClassOf p4bldg:Outlet .

p4bldg:Outlet-COMMUNICATIONSOUTLET a owl:Class ;
    rdfs:label "COMMUNICATIONSOUTLET"^^xsd:string ;
    rdfs:comment "Describe products of class COMMUNICATIONSOUTLET a specialisation of Outlet"^^xsd:string ;
    rdfs:seeAlso ifc:IfcOutletEnumType ;
    rdfs:subClassOf p4bldg:Outlet .

p4bldg:Outlet-DATAOUTLET a owl:Class ;
    rdfs:label "DATAOUTLET"^^xsd:string ;
    rdfs:comment "Describe products of class DATAOUTLET a specialisation of Outlet"^^xsd:string ;
    rdfs:seeAlso ifc:IfcOutletEnumType ;
    rdfs:subClassOf p4bldg:Outlet .

p4bldg:Outlet-NOTDEFINED a owl:Class ;
    rdfs:label "NOTDEFINED"^^xsd:string ;
    rdfs:comment "Describe products of class NOTDEFINED a specialisation of Outlet"^^xsd:string ;
    rdfs:seeAlso ifc:IfcOutletEnumType ;
    rdfs:subClassOf p4bldg:Outlet .

p4bldg:Outlet-POWEROUTLET a owl:Class ;
    rdfs:label "POWEROUTLET"^^xsd:string ;
    rdfs:comment "Describe products of class POWEROUTLET a specialisation of Outlet"^^xsd:string ;
    rdfs:seeAlso ifc:IfcOutletEnumType ;
    rdfs:subClassOf p4bldg:Outlet .

p4bldg:Outlet-TELEPHONEOUTLET a owl:Class ;
    rdfs:label "TELEPHONEOUTLET"^^xsd:string ;
    rdfs:comment "Describe products of class TELEPHONEOUTLET a specialisation of Outlet"^^xsd:string ;
    rdfs:seeAlso ifc:IfcOutletEnumType ;
    rdfs:subClassOf p4bldg:Outlet .

p4bldg:Outlet-USERDEFINED a owl:Class ;
    rdfs:label "USERDEFINED"^^xsd:string ;
    rdfs:comment "Describe products of class USERDEFINED a specialisation of Outlet"^^xsd:string ;
    rdfs:seeAlso ifc:IfcOutletEnumType ;
    rdfs:subClassOf p4bldg:Outlet .

p4bldg:Pile-BORED a owl:Class ;
    rdfs:label "BORED"^^xsd:string ;
    rdfs:comment "Describe products of class BORED a specialisation of Pile"^^xsd:string ;
    rdfs:seeAlso ifc:IfcPileEnumType ;
    rdfs:subClassOf p4bldg:Pile .

p4bldg:Pile-COHESION a owl:Class ;
    rdfs:label "COHESION"^^xsd:string ;
    rdfs:comment "Describe products of class COHESION a specialisation of Pile"^^xsd:string ;
    rdfs:seeAlso ifc:IfcPileEnumType ;
    rdfs:subClassOf p4bldg:Pile .

p4bldg:Pile-DRIVEN a owl:Class ;
    rdfs:label "DRIVEN"^^xsd:string ;
    rdfs:comment "Describe products of class DRIVEN a specialisation of Pile"^^xsd:string ;
    rdfs:seeAlso ifc:IfcPileEnumType ;
    rdfs:subClassOf p4bldg:Pile .

p4bldg:Pile-FRICTION a owl:Class ;
    rdfs:label "FRICTION"^^xsd:string ;
    rdfs:comment "Describe products of class FRICTION a specialisation of Pile"^^xsd:string ;
    rdfs:seeAlso ifc:IfcPileEnumType ;
    rdfs:subClassOf p4bldg:Pile .

p4bldg:Pile-JETGROUTING a owl:Class ;
    rdfs:label "JETGROUTING"^^xsd:string ;
    rdfs:comment "Describe products of class JETGROUTING a specialisation of Pile"^^xsd:string ;
    rdfs:seeAlso ifc:IfcPileEnumType ;
    rdfs:subClassOf p4bldg:Pile .

p4bldg:Pile-NOTDEFINED a owl:Class ;
    rdfs:label "NOTDEFINED"^^xsd:string ;
    rdfs:comment "Describe products of class NOTDEFINED a specialisation of Pile"^^xsd:string ;
    rdfs:seeAlso ifc:IfcPileEnumType ;
    rdfs:subClassOf p4bldg:Pile .

p4bldg:Pile-SUPPORT a owl:Class ;
    rdfs:label "SUPPORT"^^xsd:string ;
    rdfs:comment "Describe products of class SUPPORT a specialisation of Pile"^^xsd:string ;
    rdfs:seeAlso ifc:IfcPileEnumType ;
    rdfs:subClassOf p4bldg:Pile .

p4bldg:Pile-USERDEFINED a owl:Class ;
    rdfs:label "USERDEFINED"^^xsd:string ;
    rdfs:comment "Describe products of class USERDEFINED a specialisation of Pile"^^xsd:string ;
    rdfs:seeAlso ifc:IfcPileEnumType ;
    rdfs:subClassOf p4bldg:Pile .

p4bldg:PipeFitting-BEND a owl:Class ;
    rdfs:label "BEND"^^xsd:string ;
    rdfs:comment "Describe products of class BEND a specialisation of PipeFitting"^^xsd:string ;
    rdfs:seeAlso ifc:IfcPipeFittingEnumType ;
    rdfs:subClassOf p4bldg:PipeFitting .

p4bldg:PipeFitting-CONNECTOR a owl:Class ;
    rdfs:label "CONNECTOR"^^xsd:string ;
    rdfs:comment "Describe products of class CONNECTOR a specialisation of PipeFitting"^^xsd:string ;
    rdfs:seeAlso ifc:IfcPipeFittingEnumType ;
    rdfs:subClassOf p4bldg:PipeFitting .

p4bldg:PipeFitting-ENTRY a owl:Class ;
    rdfs:label "ENTRY"^^xsd:string ;
    rdfs:comment "Describe products of class ENTRY a specialisation of PipeFitting"^^xsd:string ;
    rdfs:seeAlso ifc:IfcPipeFittingEnumType ;
    rdfs:subClassOf p4bldg:PipeFitting .

p4bldg:PipeFitting-EXIT a owl:Class ;
    rdfs:label "EXIT"^^xsd:string ;
    rdfs:comment "Describe products of class EXIT a specialisation of PipeFitting"^^xsd:string ;
    rdfs:seeAlso ifc:IfcPipeFittingEnumType ;
    rdfs:subClassOf p4bldg:PipeFitting .

p4bldg:PipeFitting-JUNCTION a owl:Class ;
    rdfs:label "JUNCTION"^^xsd:string ;
    rdfs:comment "Describe products of class JUNCTION a specialisation of PipeFitting"^^xsd:string ;
    rdfs:seeAlso ifc:IfcPipeFittingEnumType ;
    rdfs:subClassOf p4bldg:PipeFitting .

p4bldg:PipeFitting-NOTDEFINED a owl:Class ;
    rdfs:label "NOTDEFINED"^^xsd:string ;
    rdfs:comment "Describe products of class NOTDEFINED a specialisation of PipeFitting"^^xsd:string ;
    rdfs:seeAlso ifc:IfcPipeFittingEnumType ;
    rdfs:subClassOf p4bldg:PipeFitting .

p4bldg:PipeFitting-OBSTRUCTION a owl:Class ;
    rdfs:label "OBSTRUCTION"^^xsd:string ;
    rdfs:comment "Describe products of class OBSTRUCTION a specialisation of PipeFitting"^^xsd:string ;
    rdfs:seeAlso ifc:IfcPipeFittingEnumType ;
    rdfs:subClassOf p4bldg:PipeFitting .

p4bldg:PipeFitting-TRANSITION a owl:Class ;
    rdfs:label "TRANSITION"^^xsd:string ;
    rdfs:comment "Describe products of class TRANSITION a specialisation of PipeFitting"^^xsd:string ;
    rdfs:seeAlso ifc:IfcPipeFittingEnumType ;
    rdfs:subClassOf p4bldg:PipeFitting .

p4bldg:PipeFitting-USERDEFINED a owl:Class ;
    rdfs:label "USERDEFINED"^^xsd:string ;
    rdfs:comment "Describe products of class USERDEFINED a specialisation of PipeFitting"^^xsd:string ;
    rdfs:seeAlso ifc:IfcPipeFittingEnumType ;
    rdfs:subClassOf p4bldg:PipeFitting .

p4bldg:PipeSegment-CULVERT a owl:Class ;
    rdfs:label "CULVERT"^^xsd:string ;
    rdfs:comment "Describe products of class CULVERT a specialisation of PipeSegment"^^xsd:string ;
    rdfs:seeAlso ifc:IfcPipeSegmentEnumType ;
    rdfs:subClassOf p4bldg:PipeSegment .

p4bldg:PipeSegment-FLEXIBLESEGMENT a owl:Class ;
    rdfs:label "FLEXIBLESEGMENT"^^xsd:string ;
    rdfs:comment "Describe products of class FLEXIBLESEGMENT a specialisation of PipeSegment"^^xsd:string ;
    rdfs:seeAlso ifc:IfcPipeSegmentEnumType ;
    rdfs:subClassOf p4bldg:PipeSegment .

p4bldg:PipeSegment-GUTTER a owl:Class ;
    rdfs:label "GUTTER"^^xsd:string ;
    rdfs:comment "Describe products of class GUTTER a specialisation of PipeSegment"^^xsd:string ;
    rdfs:seeAlso ifc:IfcPipeSegmentEnumType ;
    rdfs:subClassOf p4bldg:PipeSegment .

p4bldg:PipeSegment-NOTDEFINED a owl:Class ;
    rdfs:label "NOTDEFINED"^^xsd:string ;
    rdfs:comment "Describe products of class NOTDEFINED a specialisation of PipeSegment"^^xsd:string ;
    rdfs:seeAlso ifc:IfcPipeSegmentEnumType ;
    rdfs:subClassOf p4bldg:PipeSegment .

p4bldg:PipeSegment-RIGIDSEGMENT a owl:Class ;
    rdfs:label "RIGIDSEGMENT"^^xsd:string ;
    rdfs:comment "Describe products of class RIGIDSEGMENT a specialisation of PipeSegment"^^xsd:string ;
    rdfs:seeAlso ifc:IfcPipeSegmentEnumType ;
    rdfs:subClassOf p4bldg:PipeSegment .

p4bldg:PipeSegment-SPOOL a owl:Class ;
    rdfs:label "SPOOL"^^xsd:string ;
    rdfs:comment "Describe products of class SPOOL a specialisation of PipeSegment"^^xsd:string ;
    rdfs:seeAlso ifc:IfcPipeSegmentEnumType ;
    rdfs:subClassOf p4bldg:PipeSegment .

p4bldg:PipeSegment-USERDEFINED a owl:Class ;
    rdfs:label "USERDEFINED"^^xsd:string ;
    rdfs:comment "Describe products of class USERDEFINED a specialisation of PipeSegment"^^xsd:string ;
    rdfs:seeAlso ifc:IfcPipeSegmentEnumType ;
    rdfs:subClassOf p4bldg:PipeSegment .

p4bldg:Plate-CURTAIN_PANEL a owl:Class ;
    rdfs:label "CURTAIN_PANEL"^^xsd:string ;
    rdfs:comment "Describe products of class CURTAIN_PANEL a specialisation of Plate"^^xsd:string ;
    rdfs:seeAlso ifc:IfcPlateEnumType ;
    rdfs:subClassOf p4bldg:Plate .

p4bldg:Plate-NOTDEFINED a owl:Class ;
    rdfs:label "NOTDEFINED"^^xsd:string ;
    rdfs:comment "Describe products of class NOTDEFINED a specialisation of Plate"^^xsd:string ;
    rdfs:seeAlso ifc:IfcPlateEnumType ;
    rdfs:subClassOf p4bldg:Plate .

p4bldg:Plate-SHEET a owl:Class ;
    rdfs:label "SHEET"^^xsd:string ;
    rdfs:comment "Describe products of class SHEET a specialisation of Plate"^^xsd:string ;
    rdfs:seeAlso ifc:IfcPlateEnumType ;
    rdfs:subClassOf p4bldg:Plate .

p4bldg:Plate-USERDEFINED a owl:Class ;
    rdfs:label "USERDEFINED"^^xsd:string ;
    rdfs:comment "Describe products of class USERDEFINED a specialisation of Plate"^^xsd:string ;
    rdfs:seeAlso ifc:IfcPlateEnumType ;
    rdfs:subClassOf p4bldg:Plate .

p4bldg:PlateStandardCase a owl:Class ;
    rdfs:label "PlateStandardCase"^^xsd:string ;
    rdfs:comment "Describe products of class PlateStandardCase"^^xsd:string ;
    rdfs:seeAlso ifc:IfcPlateStandardCase ;
    rdfs:subClassOf p4bldg:Plate .

p4bldg:ProjectionElement-NOTDEFINED a owl:Class ;
    rdfs:label "NOTDEFINED"^^xsd:string ;
    rdfs:comment "Describe products of class NOTDEFINED a specialisation of ProjectionElement"^^xsd:string ;
    rdfs:seeAlso ifc:IfcProjectionElementEnumType ;
    rdfs:subClassOf p4bldg:ProjectionElement .

p4bldg:ProjectionElement-USERDEFINED a owl:Class ;
    rdfs:label "USERDEFINED"^^xsd:string ;
    rdfs:comment "Describe products of class USERDEFINED a specialisation of ProjectionElement"^^xsd:string ;
    rdfs:seeAlso ifc:IfcProjectionElementEnumType ;
    rdfs:subClassOf p4bldg:ProjectionElement .

p4bldg:ProtectiveDevice-CIRCUITBREAKER a owl:Class ;
    rdfs:label "CIRCUITBREAKER"^^xsd:string ;
    rdfs:comment "Describe products of class CIRCUITBREAKER a specialisation of ProtectiveDevice"^^xsd:string ;
    rdfs:seeAlso ifc:IfcProtectiveDeviceEnumType ;
    rdfs:subClassOf p4bldg:ProtectiveDevice .

p4bldg:ProtectiveDevice-EARTHINGSWITCH a owl:Class ;
    rdfs:label "EARTHINGSWITCH"^^xsd:string ;
    rdfs:comment "Describe products of class EARTHINGSWITCH a specialisation of ProtectiveDevice"^^xsd:string ;
    rdfs:seeAlso ifc:IfcProtectiveDeviceEnumType ;
    rdfs:subClassOf p4bldg:ProtectiveDevice .

p4bldg:ProtectiveDevice-EARTHLEAKAGECIRCUITBREAKER a owl:Class ;
    rdfs:label "EARTHLEAKAGECIRCUITBREAKER"^^xsd:string ;
    rdfs:comment "Describe products of class EARTHLEAKAGECIRCUITBREAKER a specialisation of ProtectiveDevice"^^xsd:string ;
    rdfs:seeAlso ifc:IfcProtectiveDeviceEnumType ;
    rdfs:subClassOf p4bldg:ProtectiveDevice .

p4bldg:ProtectiveDevice-FUSEDISCONNECTOR a owl:Class ;
    rdfs:label "FUSEDISCONNECTOR"^^xsd:string ;
    rdfs:comment "Describe products of class FUSEDISCONNECTOR a specialisation of ProtectiveDevice"^^xsd:string ;
    rdfs:seeAlso ifc:IfcProtectiveDeviceEnumType ;
    rdfs:subClassOf p4bldg:ProtectiveDevice .

p4bldg:ProtectiveDevice-NOTDEFINED a owl:Class ;
    rdfs:label "NOTDEFINED"^^xsd:string ;
    rdfs:comment "Describe products of class NOTDEFINED a specialisation of ProtectiveDevice"^^xsd:string ;
    rdfs:seeAlso ifc:IfcProtectiveDeviceEnumType ;
    rdfs:subClassOf p4bldg:ProtectiveDevice .

p4bldg:ProtectiveDevice-RESIDUALCURRENTCIRCUITBREAKER a owl:Class ;
    rdfs:label "RESIDUALCURRENTCIRCUITBREAKER"^^xsd:string ;
    rdfs:comment "Describe products of class RESIDUALCURRENTCIRCUITBREAKER a specialisation of ProtectiveDevice"^^xsd:string ;
    rdfs:seeAlso ifc:IfcProtectiveDeviceEnumType ;
    rdfs:subClassOf p4bldg:ProtectiveDevice .

p4bldg:ProtectiveDevice-RESIDUALCURRENTSWITCH a owl:Class ;
    rdfs:label "RESIDUALCURRENTSWITCH"^^xsd:string ;
    rdfs:comment "Describe products of class RESIDUALCURRENTSWITCH a specialisation of ProtectiveDevice"^^xsd:string ;
    rdfs:seeAlso ifc:IfcProtectiveDeviceEnumType ;
    rdfs:subClassOf p4bldg:ProtectiveDevice .

p4bldg:ProtectiveDevice-USERDEFINED a owl:Class ;
    rdfs:label "USERDEFINED"^^xsd:string ;
    rdfs:comment "Describe products of class USERDEFINED a specialisation of ProtectiveDevice"^^xsd:string ;
    rdfs:seeAlso ifc:IfcProtectiveDeviceEnumType ;
    rdfs:subClassOf p4bldg:ProtectiveDevice .

p4bldg:ProtectiveDevice-VARISTOR a owl:Class ;
    rdfs:label "VARISTOR"^^xsd:string ;
    rdfs:comment "Describe products of class VARISTOR a specialisation of ProtectiveDevice"^^xsd:string ;
    rdfs:seeAlso ifc:IfcProtectiveDeviceEnumType ;
    rdfs:subClassOf p4bldg:ProtectiveDevice .

p4bldg:ProtectiveDeviceTrippingUnit-ELECTROMAGNETIC a owl:Class ;
    rdfs:label "ELECTROMAGNETIC"^^xsd:string ;
    rdfs:comment "Describe products of class ELECTROMAGNETIC a specialisation of ProtectiveDeviceTrippingUnit"^^xsd:string ;
    rdfs:seeAlso ifc:IfcProtectiveDeviceTrippingUnitEnumType ;
    rdfs:subClassOf p4bldg:ProtectiveDeviceTrippingUnit .

p4bldg:ProtectiveDeviceTrippingUnit-ELECTRONIC a owl:Class ;
    rdfs:label "ELECTRONIC"^^xsd:string ;
    rdfs:comment "Describe products of class ELECTRONIC a specialisation of ProtectiveDeviceTrippingUnit"^^xsd:string ;
    rdfs:seeAlso ifc:IfcProtectiveDeviceTrippingUnitEnumType ;
    rdfs:subClassOf p4bldg:ProtectiveDeviceTrippingUnit .

p4bldg:ProtectiveDeviceTrippingUnit-NOTDEFINED a owl:Class ;
    rdfs:label "NOTDEFINED"^^xsd:string ;
    rdfs:comment "Describe products of class NOTDEFINED a specialisation of ProtectiveDeviceTrippingUnit"^^xsd:string ;
    rdfs:seeAlso ifc:IfcProtectiveDeviceTrippingUnitEnumType ;
    rdfs:subClassOf p4bldg:ProtectiveDeviceTrippingUnit .

p4bldg:ProtectiveDeviceTrippingUnit-RESIDUALCURRENT a owl:Class ;
    rdfs:label "RESIDUALCURRENT"^^xsd:string ;
    rdfs:comment "Describe products of class RESIDUALCURRENT a specialisation of ProtectiveDeviceTrippingUnit"^^xsd:string ;
    rdfs:seeAlso ifc:IfcProtectiveDeviceTrippingUnitEnumType ;
    rdfs:subClassOf p4bldg:ProtectiveDeviceTrippingUnit .

p4bldg:ProtectiveDeviceTrippingUnit-THERMAL a owl:Class ;
    rdfs:label "THERMAL"^^xsd:string ;
    rdfs:comment "Describe products of class THERMAL a specialisation of ProtectiveDeviceTrippingUnit"^^xsd:string ;
    rdfs:seeAlso ifc:IfcProtectiveDeviceTrippingUnitEnumType ;
    rdfs:subClassOf p4bldg:ProtectiveDeviceTrippingUnit .

p4bldg:ProtectiveDeviceTrippingUnit-USERDEFINED a owl:Class ;
    rdfs:label "USERDEFINED"^^xsd:string ;
    rdfs:comment "Describe products of class USERDEFINED a specialisation of ProtectiveDeviceTrippingUnit"^^xsd:string ;
    rdfs:seeAlso ifc:IfcProtectiveDeviceTrippingUnitEnumType ;
    rdfs:subClassOf p4bldg:ProtectiveDeviceTrippingUnit .

p4bldg:Pump-CIRCULATOR a owl:Class ;
    rdfs:label "CIRCULATOR"^^xsd:string ;
    rdfs:comment "Describe products of class CIRCULATOR a specialisation of Pump"^^xsd:string ;
    rdfs:seeAlso ifc:IfcPumpEnumType ;
    rdfs:subClassOf p4bldg:Pump .

p4bldg:Pump-ENDSUCTION a owl:Class ;
    rdfs:label "ENDSUCTION"^^xsd:string ;
    rdfs:comment "Describe products of class ENDSUCTION a specialisation of Pump"^^xsd:string ;
    rdfs:seeAlso ifc:IfcPumpEnumType ;
    rdfs:subClassOf p4bldg:Pump .

p4bldg:Pump-NOTDEFINED a owl:Class ;
    rdfs:label "NOTDEFINED"^^xsd:string ;
    rdfs:comment "Describe products of class NOTDEFINED a specialisation of Pump"^^xsd:string ;
    rdfs:seeAlso ifc:IfcPumpEnumType ;
    rdfs:subClassOf p4bldg:Pump .

p4bldg:Pump-SPLITCASE a owl:Class ;
    rdfs:label "SPLITCASE"^^xsd:string ;
    rdfs:comment "Describe products of class SPLITCASE a specialisation of Pump"^^xsd:string ;
    rdfs:seeAlso ifc:IfcPumpEnumType ;
    rdfs:subClassOf p4bldg:Pump .

p4bldg:Pump-SUBMERSIBLEPUMP a owl:Class ;
    rdfs:label "SUBMERSIBLEPUMP"^^xsd:string ;
    rdfs:comment "Describe products of class SUBMERSIBLEPUMP a specialisation of Pump"^^xsd:string ;
    rdfs:seeAlso ifc:IfcPumpEnumType ;
    rdfs:subClassOf p4bldg:Pump .

p4bldg:Pump-SUMPPUMP a owl:Class ;
    rdfs:label "SUMPPUMP"^^xsd:string ;
    rdfs:comment "Describe products of class SUMPPUMP a specialisation of Pump"^^xsd:string ;
    rdfs:seeAlso ifc:IfcPumpEnumType ;
    rdfs:subClassOf p4bldg:Pump .

p4bldg:Pump-USERDEFINED a owl:Class ;
    rdfs:label "USERDEFINED"^^xsd:string ;
    rdfs:comment "Describe products of class USERDEFINED a specialisation of Pump"^^xsd:string ;
    rdfs:seeAlso ifc:IfcPumpEnumType ;
    rdfs:subClassOf p4bldg:Pump .

p4bldg:Pump-VERTICALINLINE a owl:Class ;
    rdfs:label "VERTICALINLINE"^^xsd:string ;
    rdfs:comment "Describe products of class VERTICALINLINE a specialisation of Pump"^^xsd:string ;
    rdfs:seeAlso ifc:IfcPumpEnumType ;
    rdfs:subClassOf p4bldg:Pump .

p4bldg:Pump-VERTICALTURBINE a owl:Class ;
    rdfs:label "VERTICALTURBINE"^^xsd:string ;
    rdfs:comment "Describe products of class VERTICALTURBINE a specialisation of Pump"^^xsd:string ;
    rdfs:seeAlso ifc:IfcPumpEnumType ;
    rdfs:subClassOf p4bldg:Pump .

p4bldg:Railing-BALUSTRADE a owl:Class ;
    rdfs:label "BALUSTRADE"^^xsd:string ;
    rdfs:comment "Describe products of class BALUSTRADE a specialisation of Railing"^^xsd:string ;
    rdfs:seeAlso ifc:IfcRailingEnumType ;
    rdfs:subClassOf p4bldg:Railing .

p4bldg:Railing-GUARDRAIL a owl:Class ;
    rdfs:label "GUARDRAIL"^^xsd:string ;
    rdfs:comment "Describe products of class GUARDRAIL a specialisation of Railing"^^xsd:string ;
    rdfs:seeAlso ifc:IfcRailingEnumType ;
    rdfs:subClassOf p4bldg:Railing .

p4bldg:Railing-HANDRAIL a owl:Class ;
    rdfs:label "HANDRAIL"^^xsd:string ;
    rdfs:comment "Describe products of class HANDRAIL a specialisation of Railing"^^xsd:string ;
    rdfs:seeAlso ifc:IfcRailingEnumType ;
    rdfs:subClassOf p4bldg:Railing .

p4bldg:Railing-NOTDEFINED a owl:Class ;
    rdfs:label "NOTDEFINED"^^xsd:string ;
    rdfs:comment "Describe products of class NOTDEFINED a specialisation of Railing"^^xsd:string ;
    rdfs:seeAlso ifc:IfcRailingEnumType ;
    rdfs:subClassOf p4bldg:Railing .

p4bldg:Railing-USERDEFINED a owl:Class ;
    rdfs:label "USERDEFINED"^^xsd:string ;
    rdfs:comment "Describe products of class USERDEFINED a specialisation of Railing"^^xsd:string ;
    rdfs:seeAlso ifc:IfcRailingEnumType ;
    rdfs:subClassOf p4bldg:Railing .

p4bldg:Ramp-HALF_TURN_RAMP a owl:Class ;
    rdfs:label "HALF_TURN_RAMP"^^xsd:string ;
    rdfs:comment "Describe products of class HALF_TURN_RAMP a specialisation of Ramp"^^xsd:string ;
    rdfs:seeAlso ifc:IfcRampEnumType ;
    rdfs:subClassOf p4bldg:Ramp .

p4bldg:Ramp-NOTDEFINED a owl:Class ;
    rdfs:label "NOTDEFINED"^^xsd:string ;
    rdfs:comment "Describe products of class NOTDEFINED a specialisation of Ramp"^^xsd:string ;
    rdfs:seeAlso ifc:IfcRampEnumType ;
    rdfs:subClassOf p4bldg:Ramp .

p4bldg:Ramp-QUARTER_TURN_RAMP a owl:Class ;
    rdfs:label "QUARTER_TURN_RAMP"^^xsd:string ;
    rdfs:comment "Describe products of class QUARTER_TURN_RAMP a specialisation of Ramp"^^xsd:string ;
    rdfs:seeAlso ifc:IfcRampEnumType ;
    rdfs:subClassOf p4bldg:Ramp .

p4bldg:Ramp-SPIRAL_RAMP a owl:Class ;
    rdfs:label "SPIRAL_RAMP"^^xsd:string ;
    rdfs:comment "Describe products of class SPIRAL_RAMP a specialisation of Ramp"^^xsd:string ;
    rdfs:seeAlso ifc:IfcRampEnumType ;
    rdfs:subClassOf p4bldg:Ramp .

p4bldg:Ramp-STRAIGHT_RUN_RAMP a owl:Class ;
    rdfs:label "STRAIGHT_RUN_RAMP"^^xsd:string ;
    rdfs:comment "Describe products of class STRAIGHT_RUN_RAMP a specialisation of Ramp"^^xsd:string ;
    rdfs:seeAlso ifc:IfcRampEnumType ;
    rdfs:subClassOf p4bldg:Ramp .

p4bldg:Ramp-TWO_QUARTER_TURN_RAMP a owl:Class ;
    rdfs:label "TWO_QUARTER_TURN_RAMP"^^xsd:string ;
    rdfs:comment "Describe products of class TWO_QUARTER_TURN_RAMP a specialisation of Ramp"^^xsd:string ;
    rdfs:seeAlso ifc:IfcRampEnumType ;
    rdfs:subClassOf p4bldg:Ramp .

p4bldg:Ramp-TWO_STRAIGHT_RUN_RAMP a owl:Class ;
    rdfs:label "TWO_STRAIGHT_RUN_RAMP"^^xsd:string ;
    rdfs:comment "Describe products of class TWO_STRAIGHT_RUN_RAMP a specialisation of Ramp"^^xsd:string ;
    rdfs:seeAlso ifc:IfcRampEnumType ;
    rdfs:subClassOf p4bldg:Ramp .

p4bldg:Ramp-USERDEFINED a owl:Class ;
    rdfs:label "USERDEFINED"^^xsd:string ;
    rdfs:comment "Describe products of class USERDEFINED a specialisation of Ramp"^^xsd:string ;
    rdfs:seeAlso ifc:IfcRampEnumType ;
    rdfs:subClassOf p4bldg:Ramp .

p4bldg:RampFlight-NOTDEFINED a owl:Class ;
    rdfs:label "NOTDEFINED"^^xsd:string ;
    rdfs:comment "Describe products of class NOTDEFINED a specialisation of RampFlight"^^xsd:string ;
    rdfs:seeAlso ifc:IfcRampFlightEnumType ;
    rdfs:subClassOf p4bldg:RampFlight .

p4bldg:RampFlight-SPIRAL a owl:Class ;
    rdfs:label "SPIRAL"^^xsd:string ;
    rdfs:comment "Describe products of class SPIRAL a specialisation of RampFlight"^^xsd:string ;
    rdfs:seeAlso ifc:IfcRampFlightEnumType ;
    rdfs:subClassOf p4bldg:RampFlight .

p4bldg:RampFlight-STRAIGHT a owl:Class ;
    rdfs:label "STRAIGHT"^^xsd:string ;
    rdfs:comment "Describe products of class STRAIGHT a specialisation of RampFlight"^^xsd:string ;
    rdfs:seeAlso ifc:IfcRampFlightEnumType ;
    rdfs:subClassOf p4bldg:RampFlight .

p4bldg:RampFlight-USERDEFINED a owl:Class ;
    rdfs:label "USERDEFINED"^^xsd:string ;
    rdfs:comment "Describe products of class USERDEFINED a specialisation of RampFlight"^^xsd:string ;
    rdfs:seeAlso ifc:IfcRampFlightEnumType ;
    rdfs:subClassOf p4bldg:RampFlight .

p4bldg:ReinforcingBar-ANCHORING a owl:Class ;
    rdfs:label "ANCHORING"^^xsd:string ;
    rdfs:comment "Describe products of class ANCHORING a specialisation of ReinforcingBar"^^xsd:string ;
    rdfs:seeAlso ifc:IfcReinforcingBarEnumType ;
    rdfs:subClassOf p4bldg:ReinforcingBar .

p4bldg:ReinforcingBar-EDGE a owl:Class ;
    rdfs:label "EDGE"^^xsd:string ;
    rdfs:comment "Describe products of class EDGE a specialisation of ReinforcingBar"^^xsd:string ;
    rdfs:seeAlso ifc:IfcReinforcingBarEnumType ;
    rdfs:subClassOf p4bldg:ReinforcingBar .

p4bldg:ReinforcingBar-LIGATURE a owl:Class ;
    rdfs:label "LIGATURE"^^xsd:string ;
    rdfs:comment "Describe products of class LIGATURE a specialisation of ReinforcingBar"^^xsd:string ;
    rdfs:seeAlso ifc:IfcReinforcingBarEnumType ;
    rdfs:subClassOf p4bldg:ReinforcingBar .

p4bldg:ReinforcingBar-MAIN a owl:Class ;
    rdfs:label "MAIN"^^xsd:string ;
    rdfs:comment "Describe products of class MAIN a specialisation of ReinforcingBar"^^xsd:string ;
    rdfs:seeAlso ifc:IfcReinforcingBarEnumType ;
    rdfs:subClassOf p4bldg:ReinforcingBar .

p4bldg:ReinforcingBar-NOTDEFINED a owl:Class ;
    rdfs:label "NOTDEFINED"^^xsd:string ;
    rdfs:comment "Describe products of class NOTDEFINED a specialisation of ReinforcingBar"^^xsd:string ;
    rdfs:seeAlso ifc:IfcReinforcingBarEnumType ;
    rdfs:subClassOf p4bldg:ReinforcingBar .

p4bldg:ReinforcingBar-PUNCHING a owl:Class ;
    rdfs:label "PUNCHING"^^xsd:string ;
    rdfs:comment "Describe products of class PUNCHING a specialisation of ReinforcingBar"^^xsd:string ;
    rdfs:seeAlso ifc:IfcReinforcingBarEnumType ;
    rdfs:subClassOf p4bldg:ReinforcingBar .

p4bldg:ReinforcingBar-RING a owl:Class ;
    rdfs:label "RING"^^xsd:string ;
    rdfs:comment "Describe products of class RING a specialisation of ReinforcingBar"^^xsd:string ;
    rdfs:seeAlso ifc:IfcReinforcingBarEnumType ;
    rdfs:subClassOf p4bldg:ReinforcingBar .

p4bldg:ReinforcingBar-SHEAR a owl:Class ;
    rdfs:label "SHEAR"^^xsd:string ;
    rdfs:comment "Describe products of class SHEAR a specialisation of ReinforcingBar"^^xsd:string ;
    rdfs:seeAlso ifc:IfcReinforcingBarEnumType ;
    rdfs:subClassOf p4bldg:ReinforcingBar .

p4bldg:ReinforcingBar-STUD a owl:Class ;
    rdfs:label "STUD"^^xsd:string ;
    rdfs:comment "Describe products of class STUD a specialisation of ReinforcingBar"^^xsd:string ;
    rdfs:seeAlso ifc:IfcReinforcingBarEnumType ;
    rdfs:subClassOf p4bldg:ReinforcingBar .

p4bldg:ReinforcingBar-USERDEFINED a owl:Class ;
    rdfs:label "USERDEFINED"^^xsd:string ;
    rdfs:comment "Describe products of class USERDEFINED a specialisation of ReinforcingBar"^^xsd:string ;
    rdfs:seeAlso ifc:IfcReinforcingBarEnumType ;
    rdfs:subClassOf p4bldg:ReinforcingBar .

p4bldg:ReinforcingMesh-NOTDEFINED a owl:Class ;
    rdfs:label "NOTDEFINED"^^xsd:string ;
    rdfs:comment "Describe products of class NOTDEFINED a specialisation of ReinforcingMesh"^^xsd:string ;
    rdfs:seeAlso ifc:IfcReinforcingMeshEnumType ;
    rdfs:subClassOf p4bldg:ReinforcingMesh .

p4bldg:ReinforcingMesh-USERDEFINED a owl:Class ;
    rdfs:label "USERDEFINED"^^xsd:string ;
    rdfs:comment "Describe products of class USERDEFINED a specialisation of ReinforcingMesh"^^xsd:string ;
    rdfs:seeAlso ifc:IfcReinforcingMeshEnumType ;
    rdfs:subClassOf p4bldg:ReinforcingMesh .

p4bldg:Roof-BARREL_ROOF a owl:Class ;
    rdfs:label "BARREL_ROOF"^^xsd:string ;
    rdfs:comment "Describe products of class BARREL_ROOF a specialisation of Roof"^^xsd:string ;
    rdfs:seeAlso ifc:IfcRoofEnumType ;
    rdfs:subClassOf p4bldg:Roof .

p4bldg:Roof-BUTTERFLY_ROOF a owl:Class ;
    rdfs:label "BUTTERFLY_ROOF"^^xsd:string ;
    rdfs:comment "Describe products of class BUTTERFLY_ROOF a specialisation of Roof"^^xsd:string ;
    rdfs:seeAlso ifc:IfcRoofEnumType ;
    rdfs:subClassOf p4bldg:Roof .

p4bldg:Roof-DOME_ROOF a owl:Class ;
    rdfs:label "DOME_ROOF"^^xsd:string ;
    rdfs:comment "Describe products of class DOME_ROOF a specialisation of Roof"^^xsd:string ;
    rdfs:seeAlso ifc:IfcRoofEnumType ;
    rdfs:subClassOf p4bldg:Roof .

p4bldg:Roof-FLAT_ROOF a owl:Class ;
    rdfs:label "FLAT_ROOF"^^xsd:string ;
    rdfs:comment "Describe products of class FLAT_ROOF a specialisation of Roof"^^xsd:string ;
    rdfs:seeAlso ifc:IfcRoofEnumType ;
    rdfs:subClassOf p4bldg:Roof .

p4bldg:Roof-FREEFORM a owl:Class ;
    rdfs:label "FREEFORM"^^xsd:string ;
    rdfs:comment "Describe products of class FREEFORM a specialisation of Roof"^^xsd:string ;
    rdfs:seeAlso ifc:IfcRoofEnumType ;
    rdfs:subClassOf p4bldg:Roof .

p4bldg:Roof-GABLE_ROOF a owl:Class ;
    rdfs:label "GABLE_ROOF"^^xsd:string ;
    rdfs:comment "Describe products of class GABLE_ROOF a specialisation of Roof"^^xsd:string ;
    rdfs:seeAlso ifc:IfcRoofEnumType ;
    rdfs:subClassOf p4bldg:Roof .

p4bldg:Roof-GAMBREL_ROOF a owl:Class ;
    rdfs:label "GAMBREL_ROOF"^^xsd:string ;
    rdfs:comment "Describe products of class GAMBREL_ROOF a specialisation of Roof"^^xsd:string ;
    rdfs:seeAlso ifc:IfcRoofEnumType ;
    rdfs:subClassOf p4bldg:Roof .

p4bldg:Roof-HIPPED_GABLE_ROOF a owl:Class ;
    rdfs:label "HIPPED_GABLE_ROOF"^^xsd:string ;
    rdfs:comment "Describe products of class HIPPED_GABLE_ROOF a specialisation of Roof"^^xsd:string ;
    rdfs:seeAlso ifc:IfcRoofEnumType ;
    rdfs:subClassOf p4bldg:Roof .

p4bldg:Roof-HIP_ROOF a owl:Class ;
    rdfs:label "HIP_ROOF"^^xsd:string ;
    rdfs:comment "Describe products of class HIP_ROOF a specialisation of Roof"^^xsd:string ;
    rdfs:seeAlso ifc:IfcRoofEnumType ;
    rdfs:subClassOf p4bldg:Roof .

p4bldg:Roof-MANSARD_ROOF a owl:Class ;
    rdfs:label "MANSARD_ROOF"^^xsd:string ;
    rdfs:comment "Describe products of class MANSARD_ROOF a specialisation of Roof"^^xsd:string ;
    rdfs:seeAlso ifc:IfcRoofEnumType ;
    rdfs:subClassOf p4bldg:Roof .

p4bldg:Roof-NOTDEFINED a owl:Class ;
    rdfs:label "NOTDEFINED"^^xsd:string ;
    rdfs:comment "Describe products of class NOTDEFINED a specialisation of Roof"^^xsd:string ;
    rdfs:seeAlso ifc:IfcRoofEnumType ;
    rdfs:subClassOf p4bldg:Roof .

p4bldg:Roof-PAVILION_ROOF a owl:Class ;
    rdfs:label "PAVILION_ROOF"^^xsd:string ;
    rdfs:comment "Describe products of class PAVILION_ROOF a specialisation of Roof"^^xsd:string ;
    rdfs:seeAlso ifc:IfcRoofEnumType ;
    rdfs:subClassOf p4bldg:Roof .

p4bldg:Roof-RAINBOW_ROOF a owl:Class ;
    rdfs:label "RAINBOW_ROOF"^^xsd:string ;
    rdfs:comment "Describe products of class RAINBOW_ROOF a specialisation of Roof"^^xsd:string ;
    rdfs:seeAlso ifc:IfcRoofEnumType ;
    rdfs:subClassOf p4bldg:Roof .

p4bldg:Roof-SHED_ROOF a owl:Class ;
    rdfs:label "SHED_ROOF"^^xsd:string ;
    rdfs:comment "Describe products of class SHED_ROOF a specialisation of Roof"^^xsd:string ;
    rdfs:seeAlso ifc:IfcRoofEnumType ;
    rdfs:subClassOf p4bldg:Roof .

p4bldg:Roof-USERDEFINED a owl:Class ;
    rdfs:label "USERDEFINED"^^xsd:string ;
    rdfs:comment "Describe products of class USERDEFINED a specialisation of Roof"^^xsd:string ;
    rdfs:seeAlso ifc:IfcRoofEnumType ;
    rdfs:subClassOf p4bldg:Roof .

p4bldg:SanitaryTerminal-BATH a owl:Class ;
    rdfs:label "BATH"^^xsd:string ;
    rdfs:comment "Describe products of class BATH a specialisation of SanitaryTerminal"^^xsd:string ;
    rdfs:seeAlso ifc:IfcSanitaryTerminalEnumType ;
    rdfs:subClassOf p4bldg:SanitaryTerminal .

p4bldg:SanitaryTerminal-BIDET a owl:Class ;
    rdfs:label "BIDET"^^xsd:string ;
    rdfs:comment "Describe products of class BIDET a specialisation of SanitaryTerminal"^^xsd:string ;
    rdfs:seeAlso ifc:IfcSanitaryTerminalEnumType ;
    rdfs:subClassOf p4bldg:SanitaryTerminal .

p4bldg:SanitaryTerminal-CISTERN a owl:Class ;
    rdfs:label "CISTERN"^^xsd:string ;
    rdfs:comment "Describe products of class CISTERN a specialisation of SanitaryTerminal"^^xsd:string ;
    rdfs:seeAlso ifc:IfcSanitaryTerminalEnumType ;
    rdfs:subClassOf p4bldg:SanitaryTerminal .

p4bldg:SanitaryTerminal-NOTDEFINED a owl:Class ;
    rdfs:label "NOTDEFINED"^^xsd:string ;
    rdfs:comment "Describe products of class NOTDEFINED a specialisation of SanitaryTerminal"^^xsd:string ;
    rdfs:seeAlso ifc:IfcSanitaryTerminalEnumType ;
    rdfs:subClassOf p4bldg:SanitaryTerminal .

p4bldg:SanitaryTerminal-SANITARYFOUNTAIN a owl:Class ;
    rdfs:label "SANITARYFOUNTAIN"^^xsd:string ;
    rdfs:comment "Describe products of class SANITARYFOUNTAIN a specialisation of SanitaryTerminal"^^xsd:string ;
    rdfs:seeAlso ifc:IfcSanitaryTerminalEnumType ;
    rdfs:subClassOf p4bldg:SanitaryTerminal .

p4bldg:SanitaryTerminal-SHOWER a owl:Class ;
    rdfs:label "SHOWER"^^xsd:string ;
    rdfs:comment "Describe products of class SHOWER a specialisation of SanitaryTerminal"^^xsd:string ;
    rdfs:seeAlso ifc:IfcSanitaryTerminalEnumType ;
    rdfs:subClassOf p4bldg:SanitaryTerminal .

p4bldg:SanitaryTerminal-SINK a owl:Class ;
    rdfs:label "SINK"^^xsd:string ;
    rdfs:comment "Describe products of class SINK a specialisation of SanitaryTerminal"^^xsd:string ;
    rdfs:seeAlso ifc:IfcSanitaryTerminalEnumType ;
    rdfs:subClassOf p4bldg:SanitaryTerminal .

p4bldg:SanitaryTerminal-TOILETPAN a owl:Class ;
    rdfs:label "TOILETPAN"^^xsd:string ;
    rdfs:comment "Describe products of class TOILETPAN a specialisation of SanitaryTerminal"^^xsd:string ;
    rdfs:seeAlso ifc:IfcSanitaryTerminalEnumType ;
    rdfs:subClassOf p4bldg:SanitaryTerminal .

p4bldg:SanitaryTerminal-URINAL a owl:Class ;
    rdfs:label "URINAL"^^xsd:string ;
    rdfs:comment "Describe products of class URINAL a specialisation of SanitaryTerminal"^^xsd:string ;
    rdfs:seeAlso ifc:IfcSanitaryTerminalEnumType ;
    rdfs:subClassOf p4bldg:SanitaryTerminal .

p4bldg:SanitaryTerminal-USERDEFINED a owl:Class ;
    rdfs:label "USERDEFINED"^^xsd:string ;
    rdfs:comment "Describe products of class USERDEFINED a specialisation of SanitaryTerminal"^^xsd:string ;
    rdfs:seeAlso ifc:IfcSanitaryTerminalEnumType ;
    rdfs:subClassOf p4bldg:SanitaryTerminal .

p4bldg:SanitaryTerminal-WASHHANDBASIN a owl:Class ;
    rdfs:label "WASHHANDBASIN"^^xsd:string ;
    rdfs:comment "Describe products of class WASHHANDBASIN a specialisation of SanitaryTerminal"^^xsd:string ;
    rdfs:seeAlso ifc:IfcSanitaryTerminalEnumType ;
    rdfs:subClassOf p4bldg:SanitaryTerminal .

p4bldg:SanitaryTerminal-WCSEAT a owl:Class ;
    rdfs:label "WCSEAT"^^xsd:string ;
    rdfs:comment "Describe products of class WCSEAT a specialisation of SanitaryTerminal"^^xsd:string ;
    rdfs:seeAlso ifc:IfcSanitaryTerminalEnumType ;
    rdfs:subClassOf p4bldg:SanitaryTerminal .

p4bldg:Sensor-CO2SENSOR a owl:Class ;
    rdfs:label "CO2SENSOR"^^xsd:string ;
    rdfs:comment "Describe products of class CO2SENSOR a specialisation of Sensor"^^xsd:string ;
    rdfs:seeAlso ifc:IfcSensorEnumType ;
    rdfs:subClassOf p4bldg:Sensor .

p4bldg:Sensor-CONDUCTANCESENSOR a owl:Class ;
    rdfs:label "CONDUCTANCESENSOR"^^xsd:string ;
    rdfs:comment "Describe products of class CONDUCTANCESENSOR a specialisation of Sensor"^^xsd:string ;
    rdfs:seeAlso ifc:IfcSensorEnumType ;
    rdfs:subClassOf p4bldg:Sensor .

p4bldg:Sensor-CONTACTSENSOR a owl:Class ;
    rdfs:label "CONTACTSENSOR"^^xsd:string ;
    rdfs:comment "Describe products of class CONTACTSENSOR a specialisation of Sensor"^^xsd:string ;
    rdfs:seeAlso ifc:IfcSensorEnumType ;
    rdfs:subClassOf p4bldg:Sensor .

p4bldg:Sensor-COSENSOR a owl:Class ;
    rdfs:label "COSENSOR"^^xsd:string ;
    rdfs:comment "Describe products of class COSENSOR a specialisation of Sensor"^^xsd:string ;
    rdfs:seeAlso ifc:IfcSensorEnumType ;
    rdfs:subClassOf p4bldg:Sensor .

p4bldg:Sensor-FIRESENSOR a owl:Class ;
    rdfs:label "FIRESENSOR"^^xsd:string ;
    rdfs:comment "Describe products of class FIRESENSOR a specialisation of Sensor"^^xsd:string ;
    rdfs:seeAlso ifc:IfcSensorEnumType ;
    rdfs:subClassOf p4bldg:Sensor .

p4bldg:Sensor-FLOWSENSOR a owl:Class ;
    rdfs:label "FLOWSENSOR"^^xsd:string ;
    rdfs:comment "Describe products of class FLOWSENSOR a specialisation of Sensor"^^xsd:string ;
    rdfs:seeAlso ifc:IfcSensorEnumType ;
    rdfs:subClassOf p4bldg:Sensor .

p4bldg:Sensor-FROSTSENSOR a owl:Class ;
    rdfs:label "FROSTSENSOR"^^xsd:string ;
    rdfs:comment "Describe products of class FROSTSENSOR a specialisation of Sensor"^^xsd:string ;
    rdfs:seeAlso ifc:IfcSensorEnumType ;
    rdfs:subClassOf p4bldg:Sensor .

p4bldg:Sensor-GASSENSOR a owl:Class ;
    rdfs:label "GASSENSOR"^^xsd:string ;
    rdfs:comment "Describe products of class GASSENSOR a specialisation of Sensor"^^xsd:string ;
    rdfs:seeAlso ifc:IfcSensorEnumType ;
    rdfs:subClassOf p4bldg:Sensor .

p4bldg:Sensor-HEATSENSOR a owl:Class ;
    rdfs:label "HEATSENSOR"^^xsd:string ;
    rdfs:comment "Describe products of class HEATSENSOR a specialisation of Sensor"^^xsd:string ;
    rdfs:seeAlso ifc:IfcSensorEnumType ;
    rdfs:subClassOf p4bldg:Sensor .

p4bldg:Sensor-HUMIDITYSENSOR a owl:Class ;
    rdfs:label "HUMIDITYSENSOR"^^xsd:string ;
    rdfs:comment "Describe products of class HUMIDITYSENSOR a specialisation of Sensor"^^xsd:string ;
    rdfs:seeAlso ifc:IfcSensorEnumType ;
    rdfs:subClassOf p4bldg:Sensor .

p4bldg:Sensor-IDENTIFIERSENSOR a owl:Class ;
    rdfs:label "IDENTIFIERSENSOR"^^xsd:string ;
    rdfs:comment "Describe products of class IDENTIFIERSENSOR a specialisation of Sensor"^^xsd:string ;
    rdfs:seeAlso ifc:IfcSensorEnumType ;
    rdfs:subClassOf p4bldg:Sensor .

p4bldg:Sensor-IONCONCENTRATIONSENSOR a owl:Class ;
    rdfs:label "IONCONCENTRATIONSENSOR"^^xsd:string ;
    rdfs:comment "Describe products of class IONCONCENTRATIONSENSOR a specialisation of Sensor"^^xsd:string ;
    rdfs:seeAlso ifc:IfcSensorEnumType ;
    rdfs:subClassOf p4bldg:Sensor .

p4bldg:Sensor-LEVELSENSOR a owl:Class ;
    rdfs:label "LEVELSENSOR"^^xsd:string ;
    rdfs:comment "Describe products of class LEVELSENSOR a specialisation of Sensor"^^xsd:string ;
    rdfs:seeAlso ifc:IfcSensorEnumType ;
    rdfs:subClassOf p4bldg:Sensor .

p4bldg:Sensor-LIGHTSENSOR a owl:Class ;
    rdfs:label "LIGHTSENSOR"^^xsd:string ;
    rdfs:comment "Describe products of class LIGHTSENSOR a specialisation of Sensor"^^xsd:string ;
    rdfs:seeAlso ifc:IfcSensorEnumType ;
    rdfs:subClassOf p4bldg:Sensor .

p4bldg:Sensor-MOISTURESENSOR a owl:Class ;
    rdfs:label "MOISTURESENSOR"^^xsd:string ;
    rdfs:comment "Describe products of class MOISTURESENSOR a specialisation of Sensor"^^xsd:string ;
    rdfs:seeAlso ifc:IfcSensorEnumType ;
    rdfs:subClassOf p4bldg:Sensor .

p4bldg:Sensor-MOVEMENTSENSOR a owl:Class ;
    rdfs:label "MOVEMENTSENSOR"^^xsd:string ;
    rdfs:comment "Describe products of class MOVEMENTSENSOR a specialisation of Sensor"^^xsd:string ;
    rdfs:seeAlso ifc:IfcSensorEnumType ;
    rdfs:subClassOf p4bldg:Sensor .

p4bldg:Sensor-NOTDEFINED a owl:Class ;
    rdfs:label "NOTDEFINED"^^xsd:string ;
    rdfs:comment "Describe products of class NOTDEFINED a specialisation of Sensor"^^xsd:string ;
    rdfs:seeAlso ifc:IfcSensorEnumType ;
    rdfs:subClassOf p4bldg:Sensor .

p4bldg:Sensor-PHSENSOR a owl:Class ;
    rdfs:label "PHSENSOR"^^xsd:string ;
    rdfs:comment "Describe products of class PHSENSOR a specialisation of Sensor"^^xsd:string ;
    rdfs:seeAlso ifc:IfcSensorEnumType ;
    rdfs:subClassOf p4bldg:Sensor .

p4bldg:Sensor-PRESSURESENSOR a owl:Class ;
    rdfs:label "PRESSURESENSOR"^^xsd:string ;
    rdfs:comment "Describe products of class PRESSURESENSOR a specialisation of Sensor"^^xsd:string ;
    rdfs:seeAlso ifc:IfcSensorEnumType ;
    rdfs:subClassOf p4bldg:Sensor .

p4bldg:Sensor-RADIATIONSENSOR a owl:Class ;
    rdfs:label "RADIATIONSENSOR"^^xsd:string ;
    rdfs:comment "Describe products of class RADIATIONSENSOR a specialisation of Sensor"^^xsd:string ;
    rdfs:seeAlso ifc:IfcSensorEnumType ;
    rdfs:subClassOf p4bldg:Sensor .

p4bldg:Sensor-RADIOACTIVITYSENSOR a owl:Class ;
    rdfs:label "RADIOACTIVITYSENSOR"^^xsd:string ;
    rdfs:comment "Describe products of class RADIOACTIVITYSENSOR a specialisation of Sensor"^^xsd:string ;
    rdfs:seeAlso ifc:IfcSensorEnumType ;
    rdfs:subClassOf p4bldg:Sensor .

p4bldg:Sensor-SMOKESENSOR a owl:Class ;
    rdfs:label "SMOKESENSOR"^^xsd:string ;
    rdfs:comment "Describe products of class SMOKESENSOR a specialisation of Sensor"^^xsd:string ;
    rdfs:seeAlso ifc:IfcSensorEnumType ;
    rdfs:subClassOf p4bldg:Sensor .

p4bldg:Sensor-SOUNDSENSOR a owl:Class ;
    rdfs:label "SOUNDSENSOR"^^xsd:string ;
    rdfs:comment "Describe products of class SOUNDSENSOR a specialisation of Sensor"^^xsd:string ;
    rdfs:seeAlso ifc:IfcSensorEnumType ;
    rdfs:subClassOf p4bldg:Sensor .

p4bldg:Sensor-TEMPERATURESENSOR a owl:Class ;
    rdfs:label "TEMPERATURESENSOR"^^xsd:string ;
    rdfs:comment "Describe products of class TEMPERATURESENSOR a specialisation of Sensor"^^xsd:string ;
    rdfs:seeAlso ifc:IfcSensorEnumType ;
    rdfs:subClassOf p4bldg:Sensor .

p4bldg:Sensor-USERDEFINED a owl:Class ;
    rdfs:label "USERDEFINED"^^xsd:string ;
    rdfs:comment "Describe products of class USERDEFINED a specialisation of Sensor"^^xsd:string ;
    rdfs:seeAlso ifc:IfcSensorEnumType ;
    rdfs:subClassOf p4bldg:Sensor .

p4bldg:Sensor-WINDSENSOR a owl:Class ;
    rdfs:label "WINDSENSOR"^^xsd:string ;
    rdfs:comment "Describe products of class WINDSENSOR a specialisation of Sensor"^^xsd:string ;
    rdfs:seeAlso ifc:IfcSensorEnumType ;
    rdfs:subClassOf p4bldg:Sensor .

p4bldg:ShadingDevice-AWNING a owl:Class ;
    rdfs:label "AWNING"^^xsd:string ;
    rdfs:comment "Describe products of class AWNING a specialisation of ShadingDevice"^^xsd:string ;
    rdfs:seeAlso ifc:IfcShadingDeviceEnumType ;
    rdfs:subClassOf p4bldg:ShadingDevice .

p4bldg:ShadingDevice-JALOUSIE a owl:Class ;
    rdfs:label "JALOUSIE"^^xsd:string ;
    rdfs:comment "Describe products of class JALOUSIE a specialisation of ShadingDevice"^^xsd:string ;
    rdfs:seeAlso ifc:IfcShadingDeviceEnumType ;
    rdfs:subClassOf p4bldg:ShadingDevice .

p4bldg:ShadingDevice-NOTDEFINED a owl:Class ;
    rdfs:label "NOTDEFINED"^^xsd:string ;
    rdfs:comment "Describe products of class NOTDEFINED a specialisation of ShadingDevice"^^xsd:string ;
    rdfs:seeAlso ifc:IfcShadingDeviceEnumType ;
    rdfs:subClassOf p4bldg:ShadingDevice .

p4bldg:ShadingDevice-SHUTTER a owl:Class ;
    rdfs:label "SHUTTER"^^xsd:string ;
    rdfs:comment "Describe products of class SHUTTER a specialisation of ShadingDevice"^^xsd:string ;
    rdfs:seeAlso ifc:IfcShadingDeviceEnumType ;
    rdfs:subClassOf p4bldg:ShadingDevice .

p4bldg:ShadingDevice-USERDEFINED a owl:Class ;
    rdfs:label "USERDEFINED"^^xsd:string ;
    rdfs:comment "Describe products of class USERDEFINED a specialisation of ShadingDevice"^^xsd:string ;
    rdfs:seeAlso ifc:IfcShadingDeviceEnumType ;
    rdfs:subClassOf p4bldg:ShadingDevice .

p4bldg:Slab-BASESLAB a owl:Class ;
    rdfs:label "BASESLAB"^^xsd:string ;
    rdfs:comment "Describe products of class BASESLAB a specialisation of Slab"^^xsd:string ;
    rdfs:seeAlso ifc:IfcSlabEnumType ;
    rdfs:subClassOf p4bldg:Slab .

p4bldg:Slab-FLOOR a owl:Class ;
    rdfs:label "FLOOR"^^xsd:string ;
    rdfs:comment "Describe products of class FLOOR a specialisation of Slab"^^xsd:string ;
    rdfs:seeAlso ifc:IfcSlabEnumType ;
    rdfs:subClassOf p4bldg:Slab .

p4bldg:Slab-LANDING a owl:Class ;
    rdfs:label "LANDING"^^xsd:string ;
    rdfs:comment "Describe products of class LANDING a specialisation of Slab"^^xsd:string ;
    rdfs:seeAlso ifc:IfcSlabEnumType ;
    rdfs:subClassOf p4bldg:Slab .

p4bldg:Slab-NOTDEFINED a owl:Class ;
    rdfs:label "NOTDEFINED"^^xsd:string ;
    rdfs:comment "Describe products of class NOTDEFINED a specialisation of Slab"^^xsd:string ;
    rdfs:seeAlso ifc:IfcSlabEnumType ;
    rdfs:subClassOf p4bldg:Slab .

p4bldg:Slab-ROOF a owl:Class ;
    rdfs:label "ROOF"^^xsd:string ;
    rdfs:comment "Describe products of class ROOF a specialisation of Slab"^^xsd:string ;
    rdfs:seeAlso ifc:IfcSlabEnumType ;
    rdfs:subClassOf p4bldg:Slab .

p4bldg:Slab-USERDEFINED a owl:Class ;
    rdfs:label "USERDEFINED"^^xsd:string ;
    rdfs:comment "Describe products of class USERDEFINED a specialisation of Slab"^^xsd:string ;
    rdfs:seeAlso ifc:IfcSlabEnumType ;
    rdfs:subClassOf p4bldg:Slab .

p4bldg:SlabElementedCase a owl:Class ;
    rdfs:label "SlabElementedCase"^^xsd:string ;
    rdfs:comment "Describe products of class SlabElementedCase"^^xsd:string ;
    rdfs:seeAlso ifc:IfcSlabElementedCase ;
    rdfs:subClassOf p4bldg:Slab .

p4bldg:SlabStandardCase a owl:Class ;
    rdfs:label "SlabStandardCase"^^xsd:string ;
    rdfs:comment "Describe products of class SlabStandardCase"^^xsd:string ;
    rdfs:seeAlso ifc:IfcSlabStandardCase ;
    rdfs:subClassOf p4bldg:Slab .

p4bldg:SolarDevice-NOTDEFINED a owl:Class ;
    rdfs:label "NOTDEFINED"^^xsd:string ;
    rdfs:comment "Describe products of class NOTDEFINED a specialisation of SolarDevice"^^xsd:string ;
    rdfs:seeAlso ifc:IfcSolarDeviceEnumType ;
    rdfs:subClassOf p4bldg:SolarDevice .

p4bldg:SolarDevice-SOLARCOLLECTOR a owl:Class ;
    rdfs:label "SOLARCOLLECTOR"^^xsd:string ;
    rdfs:comment "Describe products of class SOLARCOLLECTOR a specialisation of SolarDevice"^^xsd:string ;
    rdfs:seeAlso ifc:IfcSolarDeviceEnumType ;
    rdfs:subClassOf p4bldg:SolarDevice .

p4bldg:SolarDevice-SOLARPANEL a owl:Class ;
    rdfs:label "SOLARPANEL"^^xsd:string ;
    rdfs:comment "Describe products of class SOLARPANEL a specialisation of SolarDevice"^^xsd:string ;
    rdfs:seeAlso ifc:IfcSolarDeviceEnumType ;
    rdfs:subClassOf p4bldg:SolarDevice .

p4bldg:SolarDevice-USERDEFINED a owl:Class ;
    rdfs:label "USERDEFINED"^^xsd:string ;
    rdfs:comment "Describe products of class USERDEFINED a specialisation of SolarDevice"^^xsd:string ;
    rdfs:seeAlso ifc:IfcSolarDeviceEnumType ;
    rdfs:subClassOf p4bldg:SolarDevice .

p4bldg:SpaceHeater-CONVECTOR a owl:Class ;
    rdfs:label "CONVECTOR"^^xsd:string ;
    rdfs:comment "Describe products of class CONVECTOR a specialisation of SpaceHeater"^^xsd:string ;
    rdfs:seeAlso ifc:IfcSpaceHeaterEnumType ;
    rdfs:subClassOf p4bldg:SpaceHeater .

p4bldg:SpaceHeater-NOTDEFINED a owl:Class ;
    rdfs:label "NOTDEFINED"^^xsd:string ;
    rdfs:comment "Describe products of class NOTDEFINED a specialisation of SpaceHeater"^^xsd:string ;
    rdfs:seeAlso ifc:IfcSpaceHeaterEnumType ;
    rdfs:subClassOf p4bldg:SpaceHeater .

p4bldg:SpaceHeater-RADIATOR a owl:Class ;
    rdfs:label "RADIATOR"^^xsd:string ;
    rdfs:comment "Describe products of class RADIATOR a specialisation of SpaceHeater"^^xsd:string ;
    rdfs:seeAlso ifc:IfcSpaceHeaterEnumType ;
    rdfs:subClassOf p4bldg:SpaceHeater .

p4bldg:SpaceHeater-USERDEFINED a owl:Class ;
    rdfs:label "USERDEFINED"^^xsd:string ;
    rdfs:comment "Describe products of class USERDEFINED a specialisation of SpaceHeater"^^xsd:string ;
    rdfs:seeAlso ifc:IfcSpaceHeaterEnumType ;
    rdfs:subClassOf p4bldg:SpaceHeater .

p4bldg:StackTerminal-BIRDCAGE a owl:Class ;
    rdfs:label "BIRDCAGE"^^xsd:string ;
    rdfs:comment "Describe products of class BIRDCAGE a specialisation of StackTerminal"^^xsd:string ;
    rdfs:seeAlso ifc:IfcStackTerminalEnumType ;
    rdfs:subClassOf p4bldg:StackTerminal .

p4bldg:StackTerminal-COWL a owl:Class ;
    rdfs:label "COWL"^^xsd:string ;
    rdfs:comment "Describe products of class COWL a specialisation of StackTerminal"^^xsd:string ;
    rdfs:seeAlso ifc:IfcStackTerminalEnumType ;
    rdfs:subClassOf p4bldg:StackTerminal .

p4bldg:StackTerminal-NOTDEFINED a owl:Class ;
    rdfs:label "NOTDEFINED"^^xsd:string ;
    rdfs:comment "Describe products of class NOTDEFINED a specialisation of StackTerminal"^^xsd:string ;
    rdfs:seeAlso ifc:IfcStackTerminalEnumType ;
    rdfs:subClassOf p4bldg:StackTerminal .

p4bldg:StackTerminal-RAINWATERHOPPER a owl:Class ;
    rdfs:label "RAINWATERHOPPER"^^xsd:string ;
    rdfs:comment "Describe products of class RAINWATERHOPPER a specialisation of StackTerminal"^^xsd:string ;
    rdfs:seeAlso ifc:IfcStackTerminalEnumType ;
    rdfs:subClassOf p4bldg:StackTerminal .

p4bldg:StackTerminal-USERDEFINED a owl:Class ;
    rdfs:label "USERDEFINED"^^xsd:string ;
    rdfs:comment "Describe products of class USERDEFINED a specialisation of StackTerminal"^^xsd:string ;
    rdfs:seeAlso ifc:IfcStackTerminalEnumType ;
    rdfs:subClassOf p4bldg:StackTerminal .

p4bldg:Stair-CURVED_RUN_STAIR a owl:Class ;
    rdfs:label "CURVED_RUN_STAIR"^^xsd:string ;
    rdfs:comment "Describe products of class CURVED_RUN_STAIR a specialisation of Stair"^^xsd:string ;
    rdfs:seeAlso ifc:IfcStairEnumType ;
    rdfs:subClassOf p4bldg:Stair .

p4bldg:Stair-DOUBLE_RETURN_STAIR a owl:Class ;
    rdfs:label "DOUBLE_RETURN_STAIR"^^xsd:string ;
    rdfs:comment "Describe products of class DOUBLE_RETURN_STAIR a specialisation of Stair"^^xsd:string ;
    rdfs:seeAlso ifc:IfcStairEnumType ;
    rdfs:subClassOf p4bldg:Stair .

p4bldg:Stair-HALF_TURN_STAIR a owl:Class ;
    rdfs:label "HALF_TURN_STAIR"^^xsd:string ;
    rdfs:comment "Describe products of class HALF_TURN_STAIR a specialisation of Stair"^^xsd:string ;
    rdfs:seeAlso ifc:IfcStairEnumType ;
    rdfs:subClassOf p4bldg:Stair .

p4bldg:Stair-HALF_WINDING_STAIR a owl:Class ;
    rdfs:label "HALF_WINDING_STAIR"^^xsd:string ;
    rdfs:comment "Describe products of class HALF_WINDING_STAIR a specialisation of Stair"^^xsd:string ;
    rdfs:seeAlso ifc:IfcStairEnumType ;
    rdfs:subClassOf p4bldg:Stair .

p4bldg:Stair-NOTDEFINED a owl:Class ;
    rdfs:label "NOTDEFINED"^^xsd:string ;
    rdfs:comment "Describe products of class NOTDEFINED a specialisation of Stair"^^xsd:string ;
    rdfs:seeAlso ifc:IfcStairEnumType ;
    rdfs:subClassOf p4bldg:Stair .

p4bldg:Stair-QUARTER_TURN_STAIR a owl:Class ;
    rdfs:label "QUARTER_TURN_STAIR"^^xsd:string ;
    rdfs:comment "Describe products of class QUARTER_TURN_STAIR a specialisation of Stair"^^xsd:string ;
    rdfs:seeAlso ifc:IfcStairEnumType ;
    rdfs:subClassOf p4bldg:Stair .

p4bldg:Stair-QUARTER_WINDING_STAIR a owl:Class ;
    rdfs:label "QUARTER_WINDING_STAIR"^^xsd:string ;
    rdfs:comment "Describe products of class QUARTER_WINDING_STAIR a specialisation of Stair"^^xsd:string ;
    rdfs:seeAlso ifc:IfcStairEnumType ;
    rdfs:subClassOf p4bldg:Stair .

p4bldg:Stair-SPIRAL_STAIR a owl:Class ;
    rdfs:label "SPIRAL_STAIR"^^xsd:string ;
    rdfs:comment "Describe products of class SPIRAL_STAIR a specialisation of Stair"^^xsd:string ;
    rdfs:seeAlso ifc:IfcStairEnumType ;
    rdfs:subClassOf p4bldg:Stair .

p4bldg:Stair-STRAIGHT_RUN_STAIR a owl:Class ;
    rdfs:label "STRAIGHT_RUN_STAIR"^^xsd:string ;
    rdfs:comment "Describe products of class STRAIGHT_RUN_STAIR a specialisation of Stair"^^xsd:string ;
    rdfs:seeAlso ifc:IfcStairEnumType ;
    rdfs:subClassOf p4bldg:Stair .

p4bldg:Stair-THREE_QUARTER_TURN_STAIR a owl:Class ;
    rdfs:label "THREE_QUARTER_TURN_STAIR"^^xsd:string ;
    rdfs:comment "Describe products of class THREE_QUARTER_TURN_STAIR a specialisation of Stair"^^xsd:string ;
    rdfs:seeAlso ifc:IfcStairEnumType ;
    rdfs:subClassOf p4bldg:Stair .

p4bldg:Stair-THREE_QUARTER_WINDING_STAIR a owl:Class ;
    rdfs:label "THREE_QUARTER_WINDING_STAIR"^^xsd:string ;
    rdfs:comment "Describe products of class THREE_QUARTER_WINDING_STAIR a specialisation of Stair"^^xsd:string ;
    rdfs:seeAlso ifc:IfcStairEnumType ;
    rdfs:subClassOf p4bldg:Stair .

p4bldg:Stair-TWO_CURVED_RUN_STAIR a owl:Class ;
    rdfs:label "TWO_CURVED_RUN_STAIR"^^xsd:string ;
    rdfs:comment "Describe products of class TWO_CURVED_RUN_STAIR a specialisation of Stair"^^xsd:string ;
    rdfs:seeAlso ifc:IfcStairEnumType ;
    rdfs:subClassOf p4bldg:Stair .

p4bldg:Stair-TWO_QUARTER_TURN_STAIR a owl:Class ;
    rdfs:label "TWO_QUARTER_TURN_STAIR"^^xsd:string ;
    rdfs:comment "Describe products of class TWO_QUARTER_TURN_STAIR a specialisation of Stair"^^xsd:string ;
    rdfs:seeAlso ifc:IfcStairEnumType ;
    rdfs:subClassOf p4bldg:Stair .

p4bldg:Stair-TWO_QUARTER_WINDING_STAIR a owl:Class ;
    rdfs:label "TWO_QUARTER_WINDING_STAIR"^^xsd:string ;
    rdfs:comment "Describe products of class TWO_QUARTER_WINDING_STAIR a specialisation of Stair"^^xsd:string ;
    rdfs:seeAlso ifc:IfcStairEnumType ;
    rdfs:subClassOf p4bldg:Stair .

p4bldg:Stair-TWO_STRAIGHT_RUN_STAIR a owl:Class ;
    rdfs:label "TWO_STRAIGHT_RUN_STAIR"^^xsd:string ;
    rdfs:comment "Describe products of class TWO_STRAIGHT_RUN_STAIR a specialisation of Stair"^^xsd:string ;
    rdfs:seeAlso ifc:IfcStairEnumType ;
    rdfs:subClassOf p4bldg:Stair .

p4bldg:Stair-USERDEFINED a owl:Class ;
    rdfs:label "USERDEFINED"^^xsd:string ;
    rdfs:comment "Describe products of class USERDEFINED a specialisation of Stair"^^xsd:string ;
    rdfs:seeAlso ifc:IfcStairEnumType ;
    rdfs:subClassOf p4bldg:Stair .

p4bldg:StairFlight-CURVED a owl:Class ;
    rdfs:label "CURVED"^^xsd:string ;
    rdfs:comment "Describe products of class CURVED a specialisation of StairFlight"^^xsd:string ;
    rdfs:seeAlso ifc:IfcStairFlightEnumType ;
    rdfs:subClassOf p4bldg:StairFlight .

p4bldg:StairFlight-FREEFORM a owl:Class ;
    rdfs:label "FREEFORM"^^xsd:string ;
    rdfs:comment "Describe products of class FREEFORM a specialisation of StairFlight"^^xsd:string ;
    rdfs:seeAlso ifc:IfcStairFlightEnumType ;
    rdfs:subClassOf p4bldg:StairFlight .

p4bldg:StairFlight-NOTDEFINED a owl:Class ;
    rdfs:label "NOTDEFINED"^^xsd:string ;
    rdfs:comment "Describe products of class NOTDEFINED a specialisation of StairFlight"^^xsd:string ;
    rdfs:seeAlso ifc:IfcStairFlightEnumType ;
    rdfs:subClassOf p4bldg:StairFlight .

p4bldg:StairFlight-SPIRAL a owl:Class ;
    rdfs:label "SPIRAL"^^xsd:string ;
    rdfs:comment "Describe products of class SPIRAL a specialisation of StairFlight"^^xsd:string ;
    rdfs:seeAlso ifc:IfcStairFlightEnumType ;
    rdfs:subClassOf p4bldg:StairFlight .

p4bldg:StairFlight-STRAIGHT a owl:Class ;
    rdfs:label "STRAIGHT"^^xsd:string ;
    rdfs:comment "Describe products of class STRAIGHT a specialisation of StairFlight"^^xsd:string ;
    rdfs:seeAlso ifc:IfcStairFlightEnumType ;
    rdfs:subClassOf p4bldg:StairFlight .

p4bldg:StairFlight-USERDEFINED a owl:Class ;
    rdfs:label "USERDEFINED"^^xsd:string ;
    rdfs:comment "Describe products of class USERDEFINED a specialisation of StairFlight"^^xsd:string ;
    rdfs:seeAlso ifc:IfcStairFlightEnumType ;
    rdfs:subClassOf p4bldg:StairFlight .

p4bldg:StairFlight-WINDER a owl:Class ;
    rdfs:label "WINDER"^^xsd:string ;
    rdfs:comment "Describe products of class WINDER a specialisation of StairFlight"^^xsd:string ;
    rdfs:seeAlso ifc:IfcStairFlightEnumType ;
    rdfs:subClassOf p4bldg:StairFlight .

p4bldg:SurfaceFeature-MARK a owl:Class ;
    rdfs:label "MARK"^^xsd:string ;
    rdfs:comment "Describe products of class MARK a specialisation of SurfaceFeature"^^xsd:string ;
    rdfs:seeAlso ifc:IfcSurfaceFeatureEnumType ;
    rdfs:subClassOf p4bldg:SurfaceFeature .

p4bldg:SurfaceFeature-NOTDEFINED a owl:Class ;
    rdfs:label "NOTDEFINED"^^xsd:string ;
    rdfs:comment "Describe products of class NOTDEFINED a specialisation of SurfaceFeature"^^xsd:string ;
    rdfs:seeAlso ifc:IfcSurfaceFeatureEnumType ;
    rdfs:subClassOf p4bldg:SurfaceFeature .

p4bldg:SurfaceFeature-TAG a owl:Class ;
    rdfs:label "TAG"^^xsd:string ;
    rdfs:comment "Describe products of class TAG a specialisation of SurfaceFeature"^^xsd:string ;
    rdfs:seeAlso ifc:IfcSurfaceFeatureEnumType ;
    rdfs:subClassOf p4bldg:SurfaceFeature .

p4bldg:SurfaceFeature-TREATMENT a owl:Class ;
    rdfs:label "TREATMENT"^^xsd:string ;
    rdfs:comment "Describe products of class TREATMENT a specialisation of SurfaceFeature"^^xsd:string ;
    rdfs:seeAlso ifc:IfcSurfaceFeatureEnumType ;
    rdfs:subClassOf p4bldg:SurfaceFeature .

p4bldg:SurfaceFeature-USERDEFINED a owl:Class ;
    rdfs:label "USERDEFINED"^^xsd:string ;
    rdfs:comment "Describe products of class USERDEFINED a specialisation of SurfaceFeature"^^xsd:string ;
    rdfs:seeAlso ifc:IfcSurfaceFeatureEnumType ;
    rdfs:subClassOf p4bldg:SurfaceFeature .

p4bldg:SwitchingDevice-CONTACTOR a owl:Class ;
    rdfs:label "CONTACTOR"^^xsd:string ;
    rdfs:comment "Describe products of class CONTACTOR a specialisation of SwitchingDevice"^^xsd:string ;
    rdfs:seeAlso ifc:IfcSwitchingDeviceEnumType ;
    rdfs:subClassOf p4bldg:SwitchingDevice .

p4bldg:SwitchingDevice-DIMMERSWITCH a owl:Class ;
    rdfs:label "DIMMERSWITCH"^^xsd:string ;
    rdfs:comment "Describe products of class DIMMERSWITCH a specialisation of SwitchingDevice"^^xsd:string ;
    rdfs:seeAlso ifc:IfcSwitchingDeviceEnumType ;
    rdfs:subClassOf p4bldg:SwitchingDevice .

p4bldg:SwitchingDevice-EMERGENCYSTOP a owl:Class ;
    rdfs:label "EMERGENCYSTOP"^^xsd:string ;
    rdfs:comment "Describe products of class EMERGENCYSTOP a specialisation of SwitchingDevice"^^xsd:string ;
    rdfs:seeAlso ifc:IfcSwitchingDeviceEnumType ;
    rdfs:subClassOf p4bldg:SwitchingDevice .

p4bldg:SwitchingDevice-KEYPAD a owl:Class ;
    rdfs:label "KEYPAD"^^xsd:string ;
    rdfs:comment "Describe products of class KEYPAD a specialisation of SwitchingDevice"^^xsd:string ;
    rdfs:seeAlso ifc:IfcSwitchingDeviceEnumType ;
    rdfs:subClassOf p4bldg:SwitchingDevice .

p4bldg:SwitchingDevice-MOMENTARYSWITCH a owl:Class ;
    rdfs:label "MOMENTARYSWITCH"^^xsd:string ;
    rdfs:comment "Describe products of class MOMENTARYSWITCH a specialisation of SwitchingDevice"^^xsd:string ;
    rdfs:seeAlso ifc:IfcSwitchingDeviceEnumType ;
    rdfs:subClassOf p4bldg:SwitchingDevice .

p4bldg:SwitchingDevice-NOTDEFINED a owl:Class ;
    rdfs:label "NOTDEFINED"^^xsd:string ;
    rdfs:comment "Describe products of class NOTDEFINED a specialisation of SwitchingDevice"^^xsd:string ;
    rdfs:seeAlso ifc:IfcSwitchingDeviceEnumType ;
    rdfs:subClassOf p4bldg:SwitchingDevice .

p4bldg:SwitchingDevice-SELECTORSWITCH a owl:Class ;
    rdfs:label "SELECTORSWITCH"^^xsd:string ;
    rdfs:comment "Describe products of class SELECTORSWITCH a specialisation of SwitchingDevice"^^xsd:string ;
    rdfs:seeAlso ifc:IfcSwitchingDeviceEnumType ;
    rdfs:subClassOf p4bldg:SwitchingDevice .

p4bldg:SwitchingDevice-STARTER a owl:Class ;
    rdfs:label "STARTER"^^xsd:string ;
    rdfs:comment "Describe products of class STARTER a specialisation of SwitchingDevice"^^xsd:string ;
    rdfs:seeAlso ifc:IfcSwitchingDeviceEnumType ;
    rdfs:subClassOf p4bldg:SwitchingDevice .

p4bldg:SwitchingDevice-SWITCHDISCONNECTOR a owl:Class ;
    rdfs:label "SWITCHDISCONNECTOR"^^xsd:string ;
    rdfs:comment "Describe products of class SWITCHDISCONNECTOR a specialisation of SwitchingDevice"^^xsd:string ;
    rdfs:seeAlso ifc:IfcSwitchingDeviceEnumType ;
    rdfs:subClassOf p4bldg:SwitchingDevice .

p4bldg:SwitchingDevice-TOGGLESWITCH a owl:Class ;
    rdfs:label "TOGGLESWITCH"^^xsd:string ;
    rdfs:comment "Describe products of class TOGGLESWITCH a specialisation of SwitchingDevice"^^xsd:string ;
    rdfs:seeAlso ifc:IfcSwitchingDeviceEnumType ;
    rdfs:subClassOf p4bldg:SwitchingDevice .

p4bldg:SwitchingDevice-USERDEFINED a owl:Class ;
    rdfs:label "USERDEFINED"^^xsd:string ;
    rdfs:comment "Describe products of class USERDEFINED a specialisation of SwitchingDevice"^^xsd:string ;
    rdfs:seeAlso ifc:IfcSwitchingDeviceEnumType ;
    rdfs:subClassOf p4bldg:SwitchingDevice .

p4bldg:SystemFurnitureElement-NOTDEFINED a owl:Class ;
    rdfs:label "NOTDEFINED"^^xsd:string ;
    rdfs:comment "Describe products of class NOTDEFINED a specialisation of SystemFurnitureElement"^^xsd:string ;
    rdfs:seeAlso ifc:IfcSystemFurnitureElementEnumType ;
    rdfs:subClassOf p4bldg:SystemFurnitureElement .

p4bldg:SystemFurnitureElement-PANEL a owl:Class ;
    rdfs:label "PANEL"^^xsd:string ;
    rdfs:comment "Describe products of class PANEL a specialisation of SystemFurnitureElement"^^xsd:string ;
    rdfs:seeAlso ifc:IfcSystemFurnitureElementEnumType ;
    rdfs:subClassOf p4bldg:SystemFurnitureElement .

p4bldg:SystemFurnitureElement-USERDEFINED a owl:Class ;
    rdfs:label "USERDEFINED"^^xsd:string ;
    rdfs:comment "Describe products of class USERDEFINED a specialisation of SystemFurnitureElement"^^xsd:string ;
    rdfs:seeAlso ifc:IfcSystemFurnitureElementEnumType ;
    rdfs:subClassOf p4bldg:SystemFurnitureElement .

p4bldg:SystemFurnitureElement-WORKSURFACE a owl:Class ;
    rdfs:label "WORKSURFACE"^^xsd:string ;
    rdfs:comment "Describe products of class WORKSURFACE a specialisation of SystemFurnitureElement"^^xsd:string ;
    rdfs:seeAlso ifc:IfcSystemFurnitureElementEnumType ;
    rdfs:subClassOf p4bldg:SystemFurnitureElement .

p4bldg:Tank-BASIN a owl:Class ;
    rdfs:label "BASIN"^^xsd:string ;
    rdfs:comment "Describe products of class BASIN a specialisation of Tank"^^xsd:string ;
    rdfs:seeAlso ifc:IfcTankEnumType ;
    rdfs:subClassOf p4bldg:Tank .

p4bldg:Tank-BREAKPRESSURE a owl:Class ;
    rdfs:label "BREAKPRESSURE"^^xsd:string ;
    rdfs:comment "Describe products of class BREAKPRESSURE a specialisation of Tank"^^xsd:string ;
    rdfs:seeAlso ifc:IfcTankEnumType ;
    rdfs:subClassOf p4bldg:Tank .

p4bldg:Tank-EXPANSION a owl:Class ;
    rdfs:label "EXPANSION"^^xsd:string ;
    rdfs:comment "Describe products of class EXPANSION a specialisation of Tank"^^xsd:string ;
    rdfs:seeAlso ifc:IfcTankEnumType ;
    rdfs:subClassOf p4bldg:Tank .

p4bldg:Tank-FEEDANDEXPANSION a owl:Class ;
    rdfs:label "FEEDANDEXPANSION"^^xsd:string ;
    rdfs:comment "Describe products of class FEEDANDEXPANSION a specialisation of Tank"^^xsd:string ;
    rdfs:seeAlso ifc:IfcTankEnumType ;
    rdfs:subClassOf p4bldg:Tank .

p4bldg:Tank-NOTDEFINED a owl:Class ;
    rdfs:label "NOTDEFINED"^^xsd:string ;
    rdfs:comment "Describe products of class NOTDEFINED a specialisation of Tank"^^xsd:string ;
    rdfs:seeAlso ifc:IfcTankEnumType ;
    rdfs:subClassOf p4bldg:Tank .

p4bldg:Tank-PRESSUREVESSEL a owl:Class ;
    rdfs:label "PRESSUREVESSEL"^^xsd:string ;
    rdfs:comment "Describe products of class PRESSUREVESSEL a specialisation of Tank"^^xsd:string ;
    rdfs:seeAlso ifc:IfcTankEnumType ;
    rdfs:subClassOf p4bldg:Tank .

p4bldg:Tank-STORAGE a owl:Class ;
    rdfs:label "STORAGE"^^xsd:string ;
    rdfs:comment "Describe products of class STORAGE a specialisation of Tank"^^xsd:string ;
    rdfs:seeAlso ifc:IfcTankEnumType ;
    rdfs:subClassOf p4bldg:Tank .

p4bldg:Tank-USERDEFINED a owl:Class ;
    rdfs:label "USERDEFINED"^^xsd:string ;
    rdfs:comment "Describe products of class USERDEFINED a specialisation of Tank"^^xsd:string ;
    rdfs:seeAlso ifc:IfcTankEnumType ;
    rdfs:subClassOf p4bldg:Tank .

p4bldg:Tank-VESSEL a owl:Class ;
    rdfs:label "VESSEL"^^xsd:string ;
    rdfs:comment "Describe products of class VESSEL a specialisation of Tank"^^xsd:string ;
    rdfs:seeAlso ifc:IfcTankEnumType ;
    rdfs:subClassOf p4bldg:Tank .

p4bldg:Tendon-BAR a owl:Class ;
    rdfs:label "BAR"^^xsd:string ;
    rdfs:comment "Describe products of class BAR a specialisation of Tendon"^^xsd:string ;
    rdfs:seeAlso ifc:IfcTendonEnumType ;
    rdfs:subClassOf p4bldg:Tendon .

p4bldg:Tendon-COATED a owl:Class ;
    rdfs:label "COATED"^^xsd:string ;
    rdfs:comment "Describe products of class COATED a specialisation of Tendon"^^xsd:string ;
    rdfs:seeAlso ifc:IfcTendonEnumType ;
    rdfs:subClassOf p4bldg:Tendon .

p4bldg:Tendon-NOTDEFINED a owl:Class ;
    rdfs:label "NOTDEFINED"^^xsd:string ;
    rdfs:comment "Describe products of class NOTDEFINED a specialisation of Tendon"^^xsd:string ;
    rdfs:seeAlso ifc:IfcTendonEnumType ;
    rdfs:subClassOf p4bldg:Tendon .

p4bldg:Tendon-STRAND a owl:Class ;
    rdfs:label "STRAND"^^xsd:string ;
    rdfs:comment "Describe products of class STRAND a specialisation of Tendon"^^xsd:string ;
    rdfs:seeAlso ifc:IfcTendonEnumType ;
    rdfs:subClassOf p4bldg:Tendon .

p4bldg:Tendon-USERDEFINED a owl:Class ;
    rdfs:label "USERDEFINED"^^xsd:string ;
    rdfs:comment "Describe products of class USERDEFINED a specialisation of Tendon"^^xsd:string ;
    rdfs:seeAlso ifc:IfcTendonEnumType ;
    rdfs:subClassOf p4bldg:Tendon .

p4bldg:Tendon-WIRE a owl:Class ;
    rdfs:label "WIRE"^^xsd:string ;
    rdfs:comment "Describe products of class WIRE a specialisation of Tendon"^^xsd:string ;
    rdfs:seeAlso ifc:IfcTendonEnumType ;
    rdfs:subClassOf p4bldg:Tendon .

p4bldg:TendonAnchor-COUPLER a owl:Class ;
    rdfs:label "COUPLER"^^xsd:string ;
    rdfs:comment "Describe products of class COUPLER a specialisation of TendonAnchor"^^xsd:string ;
    rdfs:seeAlso ifc:IfcTendonAnchorEnumType ;
    rdfs:subClassOf p4bldg:TendonAnchor .

p4bldg:TendonAnchor-FIXED_END a owl:Class ;
    rdfs:label "FIXED_END"^^xsd:string ;
    rdfs:comment "Describe products of class FIXED_END a specialisation of TendonAnchor"^^xsd:string ;
    rdfs:seeAlso ifc:IfcTendonAnchorEnumType ;
    rdfs:subClassOf p4bldg:TendonAnchor .

p4bldg:TendonAnchor-NOTDEFINED a owl:Class ;
    rdfs:label "NOTDEFINED"^^xsd:string ;
    rdfs:comment "Describe products of class NOTDEFINED a specialisation of TendonAnchor"^^xsd:string ;
    rdfs:seeAlso ifc:IfcTendonAnchorEnumType ;
    rdfs:subClassOf p4bldg:TendonAnchor .

p4bldg:TendonAnchor-TENSIONING_END a owl:Class ;
    rdfs:label "TENSIONING_END"^^xsd:string ;
    rdfs:comment "Describe products of class TENSIONING_END a specialisation of TendonAnchor"^^xsd:string ;
    rdfs:seeAlso ifc:IfcTendonAnchorEnumType ;
    rdfs:subClassOf p4bldg:TendonAnchor .

p4bldg:TendonAnchor-USERDEFINED a owl:Class ;
    rdfs:label "USERDEFINED"^^xsd:string ;
    rdfs:comment "Describe products of class USERDEFINED a specialisation of TendonAnchor"^^xsd:string ;
    rdfs:seeAlso ifc:IfcTendonAnchorEnumType ;
    rdfs:subClassOf p4bldg:TendonAnchor .

p4bldg:Transformer-CURRENT a owl:Class ;
    rdfs:label "CURRENT"^^xsd:string ;
    rdfs:comment "Describe products of class CURRENT a specialisation of Transformer"^^xsd:string ;
    rdfs:seeAlso ifc:IfcTransformerEnumType ;
    rdfs:subClassOf p4bldg:Transformer .

p4bldg:Transformer-FREQUENCY a owl:Class ;
    rdfs:label "FREQUENCY"^^xsd:string ;
    rdfs:comment "Describe products of class FREQUENCY a specialisation of Transformer"^^xsd:string ;
    rdfs:seeAlso ifc:IfcTransformerEnumType ;
    rdfs:subClassOf p4bldg:Transformer .

p4bldg:Transformer-INVERTER a owl:Class ;
    rdfs:label "INVERTER"^^xsd:string ;
    rdfs:comment "Describe products of class INVERTER a specialisation of Transformer"^^xsd:string ;
    rdfs:seeAlso ifc:IfcTransformerEnumType ;
    rdfs:subClassOf p4bldg:Transformer .

p4bldg:Transformer-NOTDEFINED a owl:Class ;
    rdfs:label "NOTDEFINED"^^xsd:string ;
    rdfs:comment "Describe products of class NOTDEFINED a specialisation of Transformer"^^xsd:string ;
    rdfs:seeAlso ifc:IfcTransformerEnumType ;
    rdfs:subClassOf p4bldg:Transformer .

p4bldg:Transformer-RECTIFIER a owl:Class ;
    rdfs:label "RECTIFIER"^^xsd:string ;
    rdfs:comment "Describe products of class RECTIFIER a specialisation of Transformer"^^xsd:string ;
    rdfs:seeAlso ifc:IfcTransformerEnumType ;
    rdfs:subClassOf p4bldg:Transformer .

p4bldg:Transformer-USERDEFINED a owl:Class ;
    rdfs:label "USERDEFINED"^^xsd:string ;
    rdfs:comment "Describe products of class USERDEFINED a specialisation of Transformer"^^xsd:string ;
    rdfs:seeAlso ifc:IfcTransformerEnumType ;
    rdfs:subClassOf p4bldg:Transformer .

p4bldg:Transformer-VOLTAGE a owl:Class ;
    rdfs:label "VOLTAGE"^^xsd:string ;
    rdfs:comment "Describe products of class VOLTAGE a specialisation of Transformer"^^xsd:string ;
    rdfs:seeAlso ifc:IfcTransformerEnumType ;
    rdfs:subClassOf p4bldg:Transformer .

p4bldg:TransportElement-CRANEWAY a owl:Class ;
    rdfs:label "CRANEWAY"^^xsd:string ;
    rdfs:comment "Describe products of class CRANEWAY a specialisation of TransportElement"^^xsd:string ;
    rdfs:seeAlso ifc:IfcTransportElementEnumType ;
    rdfs:subClassOf p4bldg:TransportElement .

p4bldg:TransportElement-ELEVATOR a owl:Class ;
    rdfs:label "ELEVATOR"^^xsd:string ;
    rdfs:comment "Describe products of class ELEVATOR a specialisation of TransportElement"^^xsd:string ;
    rdfs:seeAlso ifc:IfcTransportElementEnumType ;
    rdfs:subClassOf p4bldg:TransportElement .

p4bldg:TransportElement-ESCALATOR a owl:Class ;
    rdfs:label "ESCALATOR"^^xsd:string ;
    rdfs:comment "Describe products of class ESCALATOR a specialisation of TransportElement"^^xsd:string ;
    rdfs:seeAlso ifc:IfcTransportElementEnumType ;
    rdfs:subClassOf p4bldg:TransportElement .

p4bldg:TransportElement-LIFTINGGEAR a owl:Class ;
    rdfs:label "LIFTINGGEAR"^^xsd:string ;
    rdfs:comment "Describe products of class LIFTINGGEAR a specialisation of TransportElement"^^xsd:string ;
    rdfs:seeAlso ifc:IfcTransportElementEnumType ;
    rdfs:subClassOf p4bldg:TransportElement .

p4bldg:TransportElement-MOVINGWALKWAY a owl:Class ;
    rdfs:label "MOVINGWALKWAY"^^xsd:string ;
    rdfs:comment "Describe products of class MOVINGWALKWAY a specialisation of TransportElement"^^xsd:string ;
    rdfs:seeAlso ifc:IfcTransportElementEnumType ;
    rdfs:subClassOf p4bldg:TransportElement .

p4bldg:TransportElement-NOTDEFINED a owl:Class ;
    rdfs:label "NOTDEFINED"^^xsd:string ;
    rdfs:comment "Describe products of class NOTDEFINED a specialisation of TransportElement"^^xsd:string ;
    rdfs:seeAlso ifc:IfcTransportElementEnumType ;
    rdfs:subClassOf p4bldg:TransportElement .

p4bldg:TransportElement-USERDEFINED a owl:Class ;
    rdfs:label "USERDEFINED"^^xsd:string ;
    rdfs:comment "Describe products of class USERDEFINED a specialisation of TransportElement"^^xsd:string ;
    rdfs:seeAlso ifc:IfcTransportElementEnumType ;
    rdfs:subClassOf p4bldg:TransportElement .

p4bldg:TubeBundle-FINNED a owl:Class ;
    rdfs:label "FINNED"^^xsd:string ;
    rdfs:comment "Describe products of class FINNED a specialisation of TubeBundle"^^xsd:string ;
    rdfs:seeAlso ifc:IfcTubeBundleEnumType ;
    rdfs:subClassOf p4bldg:TubeBundle .

p4bldg:TubeBundle-NOTDEFINED a owl:Class ;
    rdfs:label "NOTDEFINED"^^xsd:string ;
    rdfs:comment "Describe products of class NOTDEFINED a specialisation of TubeBundle"^^xsd:string ;
    rdfs:seeAlso ifc:IfcTubeBundleEnumType ;
    rdfs:subClassOf p4bldg:TubeBundle .

p4bldg:TubeBundle-USERDEFINED a owl:Class ;
    rdfs:label "USERDEFINED"^^xsd:string ;
    rdfs:comment "Describe products of class USERDEFINED a specialisation of TubeBundle"^^xsd:string ;
    rdfs:seeAlso ifc:IfcTubeBundleEnumType ;
    rdfs:subClassOf p4bldg:TubeBundle .

p4bldg:UnitaryControlElement-ALARMPANEL a owl:Class ;
    rdfs:label "ALARMPANEL"^^xsd:string ;
    rdfs:comment "Describe products of class ALARMPANEL a specialisation of UnitaryControlElement"^^xsd:string ;
    rdfs:seeAlso ifc:IfcUnitaryControlElementEnumType ;
    rdfs:subClassOf p4bldg:UnitaryControlElement .

p4bldg:UnitaryControlElement-CONTROLPANEL a owl:Class ;
    rdfs:label "CONTROLPANEL"^^xsd:string ;
    rdfs:comment "Describe products of class CONTROLPANEL a specialisation of UnitaryControlElement"^^xsd:string ;
    rdfs:seeAlso ifc:IfcUnitaryControlElementEnumType ;
    rdfs:subClassOf p4bldg:UnitaryControlElement .

p4bldg:UnitaryControlElement-GASDETECTIONPANEL a owl:Class ;
    rdfs:label "GASDETECTIONPANEL"^^xsd:string ;
    rdfs:comment "Describe products of class GASDETECTIONPANEL a specialisation of UnitaryControlElement"^^xsd:string ;
    rdfs:seeAlso ifc:IfcUnitaryControlElementEnumType ;
    rdfs:subClassOf p4bldg:UnitaryControlElement .

p4bldg:UnitaryControlElement-HUMIDISTAT a owl:Class ;
    rdfs:label "HUMIDISTAT"^^xsd:string ;
    rdfs:comment "Describe products of class HUMIDISTAT a specialisation of UnitaryControlElement"^^xsd:string ;
    rdfs:seeAlso ifc:IfcUnitaryControlElementEnumType ;
    rdfs:subClassOf p4bldg:UnitaryControlElement .

p4bldg:UnitaryControlElement-INDICATORPANEL a owl:Class ;
    rdfs:label "INDICATORPANEL"^^xsd:string ;
    rdfs:comment "Describe products of class INDICATORPANEL a specialisation of UnitaryControlElement"^^xsd:string ;
    rdfs:seeAlso ifc:IfcUnitaryControlElementEnumType ;
    rdfs:subClassOf p4bldg:UnitaryControlElement .

p4bldg:UnitaryControlElement-MIMICPANEL a owl:Class ;
    rdfs:label "MIMICPANEL"^^xsd:string ;
    rdfs:comment "Describe products of class MIMICPANEL a specialisation of UnitaryControlElement"^^xsd:string ;
    rdfs:seeAlso ifc:IfcUnitaryControlElementEnumType ;
    rdfs:subClassOf p4bldg:UnitaryControlElement .

p4bldg:UnitaryControlElement-NOTDEFINED a owl:Class ;
    rdfs:label "NOTDEFINED"^^xsd:string ;
    rdfs:comment "Describe products of class NOTDEFINED a specialisation of UnitaryControlElement"^^xsd:string ;
    rdfs:seeAlso ifc:IfcUnitaryControlElementEnumType ;
    rdfs:subClassOf p4bldg:UnitaryControlElement .

p4bldg:UnitaryControlElement-THERMOSTAT a owl:Class ;
    rdfs:label "THERMOSTAT"^^xsd:string ;
    rdfs:comment "Describe products of class THERMOSTAT a specialisation of UnitaryControlElement"^^xsd:string ;
    rdfs:seeAlso ifc:IfcUnitaryControlElementEnumType ;
    rdfs:subClassOf p4bldg:UnitaryControlElement .

p4bldg:UnitaryControlElement-USERDEFINED a owl:Class ;
    rdfs:label "USERDEFINED"^^xsd:string ;
    rdfs:comment "Describe products of class USERDEFINED a specialisation of UnitaryControlElement"^^xsd:string ;
    rdfs:seeAlso ifc:IfcUnitaryControlElementEnumType ;
    rdfs:subClassOf p4bldg:UnitaryControlElement .

p4bldg:UnitaryControlElement-WEATHERSTATION a owl:Class ;
    rdfs:label "WEATHERSTATION"^^xsd:string ;
    rdfs:comment "Describe products of class WEATHERSTATION a specialisation of UnitaryControlElement"^^xsd:string ;
    rdfs:seeAlso ifc:IfcUnitaryControlElementEnumType ;
    rdfs:subClassOf p4bldg:UnitaryControlElement .

p4bldg:UnitaryEquipment-AIRCONDITIONINGUNIT a owl:Class ;
    rdfs:label "AIRCONDITIONINGUNIT"^^xsd:string ;
    rdfs:comment "Describe products of class AIRCONDITIONINGUNIT a specialisation of UnitaryEquipment"^^xsd:string ;
    rdfs:seeAlso ifc:IfcUnitaryEquipmentEnumType ;
    rdfs:subClassOf p4bldg:UnitaryEquipment .

p4bldg:UnitaryEquipment-AIRHANDLER a owl:Class ;
    rdfs:label "AIRHANDLER"^^xsd:string ;
    rdfs:comment "Describe products of class AIRHANDLER a specialisation of UnitaryEquipment"^^xsd:string ;
    rdfs:seeAlso ifc:IfcUnitaryEquipmentEnumType ;
    rdfs:subClassOf p4bldg:UnitaryEquipment .

p4bldg:UnitaryEquipment-DEHUMIDIFIER a owl:Class ;
    rdfs:label "DEHUMIDIFIER"^^xsd:string ;
    rdfs:comment "Describe products of class DEHUMIDIFIER a specialisation of UnitaryEquipment"^^xsd:string ;
    rdfs:seeAlso ifc:IfcUnitaryEquipmentEnumType ;
    rdfs:subClassOf p4bldg:UnitaryEquipment .

p4bldg:UnitaryEquipment-NOTDEFINED a owl:Class ;
    rdfs:label "NOTDEFINED"^^xsd:string ;
    rdfs:comment "Describe products of class NOTDEFINED a specialisation of UnitaryEquipment"^^xsd:string ;
    rdfs:seeAlso ifc:IfcUnitaryEquipmentEnumType ;
    rdfs:subClassOf p4bldg:UnitaryEquipment .

p4bldg:UnitaryEquipment-ROOFTOPUNIT a owl:Class ;
    rdfs:label "ROOFTOPUNIT"^^xsd:string ;
    rdfs:comment "Describe products of class ROOFTOPUNIT a specialisation of UnitaryEquipment"^^xsd:string ;
    rdfs:seeAlso ifc:IfcUnitaryEquipmentEnumType ;
    rdfs:subClassOf p4bldg:UnitaryEquipment .

p4bldg:UnitaryEquipment-SPLITSYSTEM a owl:Class ;
    rdfs:label "SPLITSYSTEM"^^xsd:string ;
    rdfs:comment "Describe products of class SPLITSYSTEM a specialisation of UnitaryEquipment"^^xsd:string ;
    rdfs:seeAlso ifc:IfcUnitaryEquipmentEnumType ;
    rdfs:subClassOf p4bldg:UnitaryEquipment .

p4bldg:UnitaryEquipment-USERDEFINED a owl:Class ;
    rdfs:label "USERDEFINED"^^xsd:string ;
    rdfs:comment "Describe products of class USERDEFINED a specialisation of UnitaryEquipment"^^xsd:string ;
    rdfs:seeAlso ifc:IfcUnitaryEquipmentEnumType ;
    rdfs:subClassOf p4bldg:UnitaryEquipment .

p4bldg:Valve-AIRRELEASE a owl:Class ;
    rdfs:label "AIRRELEASE"^^xsd:string ;
    rdfs:comment "Describe products of class AIRRELEASE a specialisation of Valve"^^xsd:string ;
    rdfs:seeAlso ifc:IfcValveEnumType ;
    rdfs:subClassOf p4bldg:Valve .

p4bldg:Valve-ANTIVACUUM a owl:Class ;
    rdfs:label "ANTIVACUUM"^^xsd:string ;
    rdfs:comment "Describe products of class ANTIVACUUM a specialisation of Valve"^^xsd:string ;
    rdfs:seeAlso ifc:IfcValveEnumType ;
    rdfs:subClassOf p4bldg:Valve .

p4bldg:Valve-CHANGEOVER a owl:Class ;
    rdfs:label "CHANGEOVER"^^xsd:string ;
    rdfs:comment "Describe products of class CHANGEOVER a specialisation of Valve"^^xsd:string ;
    rdfs:seeAlso ifc:IfcValveEnumType ;
    rdfs:subClassOf p4bldg:Valve .

p4bldg:Valve-CHECK a owl:Class ;
    rdfs:label "CHECK"^^xsd:string ;
    rdfs:comment "Describe products of class CHECK a specialisation of Valve"^^xsd:string ;
    rdfs:seeAlso ifc:IfcValveEnumType ;
    rdfs:subClassOf p4bldg:Valve .

p4bldg:Valve-COMMISSIONING a owl:Class ;
    rdfs:label "COMMISSIONING"^^xsd:string ;
    rdfs:comment "Describe products of class COMMISSIONING a specialisation of Valve"^^xsd:string ;
    rdfs:seeAlso ifc:IfcValveEnumType ;
    rdfs:subClassOf p4bldg:Valve .

p4bldg:Valve-DIVERTING a owl:Class ;
    rdfs:label "DIVERTING"^^xsd:string ;
    rdfs:comment "Describe products of class DIVERTING a specialisation of Valve"^^xsd:string ;
    rdfs:seeAlso ifc:IfcValveEnumType ;
    rdfs:subClassOf p4bldg:Valve .

p4bldg:Valve-DOUBLECHECK a owl:Class ;
    rdfs:label "DOUBLECHECK"^^xsd:string ;
    rdfs:comment "Describe products of class DOUBLECHECK a specialisation of Valve"^^xsd:string ;
    rdfs:seeAlso ifc:IfcValveEnumType ;
    rdfs:subClassOf p4bldg:Valve .

p4bldg:Valve-DOUBLEREGULATING a owl:Class ;
    rdfs:label "DOUBLEREGULATING"^^xsd:string ;
    rdfs:comment "Describe products of class DOUBLEREGULATING a specialisation of Valve"^^xsd:string ;
    rdfs:seeAlso ifc:IfcValveEnumType ;
    rdfs:subClassOf p4bldg:Valve .

p4bldg:Valve-DRAWOFFCOCK a owl:Class ;
    rdfs:label "DRAWOFFCOCK"^^xsd:string ;
    rdfs:comment "Describe products of class DRAWOFFCOCK a specialisation of Valve"^^xsd:string ;
    rdfs:seeAlso ifc:IfcValveEnumType ;
    rdfs:subClassOf p4bldg:Valve .

p4bldg:Valve-FAUCET a owl:Class ;
    rdfs:label "FAUCET"^^xsd:string ;
    rdfs:comment "Describe products of class FAUCET a specialisation of Valve"^^xsd:string ;
    rdfs:seeAlso ifc:IfcValveEnumType ;
    rdfs:subClassOf p4bldg:Valve .

p4bldg:Valve-FLUSHING a owl:Class ;
    rdfs:label "FLUSHING"^^xsd:string ;
    rdfs:comment "Describe products of class FLUSHING a specialisation of Valve"^^xsd:string ;
    rdfs:seeAlso ifc:IfcValveEnumType ;
    rdfs:subClassOf p4bldg:Valve .

p4bldg:Valve-GASCOCK a owl:Class ;
    rdfs:label "GASCOCK"^^xsd:string ;
    rdfs:comment "Describe products of class GASCOCK a specialisation of Valve"^^xsd:string ;
    rdfs:seeAlso ifc:IfcValveEnumType ;
    rdfs:subClassOf p4bldg:Valve .

p4bldg:Valve-GASTAP a owl:Class ;
    rdfs:label "GASTAP"^^xsd:string ;
    rdfs:comment "Describe products of class GASTAP a specialisation of Valve"^^xsd:string ;
    rdfs:seeAlso ifc:IfcValveEnumType ;
    rdfs:subClassOf p4bldg:Valve .

p4bldg:Valve-ISOLATING a owl:Class ;
    rdfs:label "ISOLATING"^^xsd:string ;
    rdfs:comment "Describe products of class ISOLATING a specialisation of Valve"^^xsd:string ;
    rdfs:seeAlso ifc:IfcValveEnumType ;
    rdfs:subClassOf p4bldg:Valve .

p4bldg:Valve-MIXING a owl:Class ;
    rdfs:label "MIXING"^^xsd:string ;
    rdfs:comment "Describe products of class MIXING a specialisation of Valve"^^xsd:string ;
    rdfs:seeAlso ifc:IfcValveEnumType ;
    rdfs:subClassOf p4bldg:Valve .

p4bldg:Valve-NOTDEFINED a owl:Class ;
    rdfs:label "NOTDEFINED"^^xsd:string ;
    rdfs:comment "Describe products of class NOTDEFINED a specialisation of Valve"^^xsd:string ;
    rdfs:seeAlso ifc:IfcValveEnumType ;
    rdfs:subClassOf p4bldg:Valve .

p4bldg:Valve-PRESSUREREDUCING a owl:Class ;
    rdfs:label "PRESSUREREDUCING"^^xsd:string ;
    rdfs:comment "Describe products of class PRESSUREREDUCING a specialisation of Valve"^^xsd:string ;
    rdfs:seeAlso ifc:IfcValveEnumType ;
    rdfs:subClassOf p4bldg:Valve .

p4bldg:Valve-PRESSURERELIEF a owl:Class ;
    rdfs:label "PRESSURERELIEF"^^xsd:string ;
    rdfs:comment "Describe products of class PRESSURERELIEF a specialisation of Valve"^^xsd:string ;
    rdfs:seeAlso ifc:IfcValveEnumType ;
    rdfs:subClassOf p4bldg:Valve .

p4bldg:Valve-REGULATING a owl:Class ;
    rdfs:label "REGULATING"^^xsd:string ;
    rdfs:comment "Describe products of class REGULATING a specialisation of Valve"^^xsd:string ;
    rdfs:seeAlso ifc:IfcValveEnumType ;
    rdfs:subClassOf p4bldg:Valve .

p4bldg:Valve-SAFETYCUTOFF a owl:Class ;
    rdfs:label "SAFETYCUTOFF"^^xsd:string ;
    rdfs:comment "Describe products of class SAFETYCUTOFF a specialisation of Valve"^^xsd:string ;
    rdfs:seeAlso ifc:IfcValveEnumType ;
    rdfs:subClassOf p4bldg:Valve .

p4bldg:Valve-STEAMTRAP a owl:Class ;
    rdfs:label "STEAMTRAP"^^xsd:string ;
    rdfs:comment "Describe products of class STEAMTRAP a specialisation of Valve"^^xsd:string ;
    rdfs:seeAlso ifc:IfcValveEnumType ;
    rdfs:subClassOf p4bldg:Valve .

p4bldg:Valve-STOPCOCK a owl:Class ;
    rdfs:label "STOPCOCK"^^xsd:string ;
    rdfs:comment "Describe products of class STOPCOCK a specialisation of Valve"^^xsd:string ;
    rdfs:seeAlso ifc:IfcValveEnumType ;
    rdfs:subClassOf p4bldg:Valve .

p4bldg:Valve-USERDEFINED a owl:Class ;
    rdfs:label "USERDEFINED"^^xsd:string ;
    rdfs:comment "Describe products of class USERDEFINED a specialisation of Valve"^^xsd:string ;
    rdfs:seeAlso ifc:IfcValveEnumType ;
    rdfs:subClassOf p4bldg:Valve .

p4bldg:VibrationIsolator-COMPRESSION a owl:Class ;
    rdfs:label "COMPRESSION"^^xsd:string ;
    rdfs:comment "Describe products of class COMPRESSION a specialisation of VibrationIsolator"^^xsd:string ;
    rdfs:seeAlso ifc:IfcVibrationIsolatorEnumType ;
    rdfs:subClassOf p4bldg:VibrationIsolator .

p4bldg:VibrationIsolator-NOTDEFINED a owl:Class ;
    rdfs:label "NOTDEFINED"^^xsd:string ;
    rdfs:comment "Describe products of class NOTDEFINED a specialisation of VibrationIsolator"^^xsd:string ;
    rdfs:seeAlso ifc:IfcVibrationIsolatorEnumType ;
    rdfs:subClassOf p4bldg:VibrationIsolator .

p4bldg:VibrationIsolator-SPRING a owl:Class ;
    rdfs:label "SPRING"^^xsd:string ;
    rdfs:comment "Describe products of class SPRING a specialisation of VibrationIsolator"^^xsd:string ;
    rdfs:seeAlso ifc:IfcVibrationIsolatorEnumType ;
    rdfs:subClassOf p4bldg:VibrationIsolator .

p4bldg:VibrationIsolator-USERDEFINED a owl:Class ;
    rdfs:label "USERDEFINED"^^xsd:string ;
    rdfs:comment "Describe products of class USERDEFINED a specialisation of VibrationIsolator"^^xsd:string ;
    rdfs:seeAlso ifc:IfcVibrationIsolatorEnumType ;
    rdfs:subClassOf p4bldg:VibrationIsolator .

p4bldg:VirtualElement a owl:Class ;
    rdfs:label "VirtualElement"^^xsd:string ;
    rdfs:comment "Describe products of class VirtualElement"^^xsd:string ;
    rdfs:seeAlso ifc:IfcVirtualElement ;
    rdfs:subClassOf p4bldg:Element .

p4bldg:VoidingFeature-CHAMFER a owl:Class ;
    rdfs:label "CHAMFER"^^xsd:string ;
    rdfs:comment "Describe products of class CHAMFER a specialisation of VoidingFeature"^^xsd:string ;
    rdfs:seeAlso ifc:IfcVoidingFeatureEnumType ;
    rdfs:subClassOf p4bldg:VoidingFeature .

p4bldg:VoidingFeature-CUTOUT a owl:Class ;
    rdfs:label "CUTOUT"^^xsd:string ;
    rdfs:comment "Describe products of class CUTOUT a specialisation of VoidingFeature"^^xsd:string ;
    rdfs:seeAlso ifc:IfcVoidingFeatureEnumType ;
    rdfs:subClassOf p4bldg:VoidingFeature .

p4bldg:VoidingFeature-EDGE a owl:Class ;
    rdfs:label "EDGE"^^xsd:string ;
    rdfs:comment "Describe products of class EDGE a specialisation of VoidingFeature"^^xsd:string ;
    rdfs:seeAlso ifc:IfcVoidingFeatureEnumType ;
    rdfs:subClassOf p4bldg:VoidingFeature .

p4bldg:VoidingFeature-HOLE a owl:Class ;
    rdfs:label "HOLE"^^xsd:string ;
    rdfs:comment "Describe products of class HOLE a specialisation of VoidingFeature"^^xsd:string ;
    rdfs:seeAlso ifc:IfcVoidingFeatureEnumType ;
    rdfs:subClassOf p4bldg:VoidingFeature .

p4bldg:VoidingFeature-MITER a owl:Class ;
    rdfs:label "MITER"^^xsd:string ;
    rdfs:comment "Describe products of class MITER a specialisation of VoidingFeature"^^xsd:string ;
    rdfs:seeAlso ifc:IfcVoidingFeatureEnumType ;
    rdfs:subClassOf p4bldg:VoidingFeature .

p4bldg:VoidingFeature-NOTCH a owl:Class ;
    rdfs:label "NOTCH"^^xsd:string ;
    rdfs:comment "Describe products of class NOTCH a specialisation of VoidingFeature"^^xsd:string ;
    rdfs:seeAlso ifc:IfcVoidingFeatureEnumType ;
    rdfs:subClassOf p4bldg:VoidingFeature .

p4bldg:VoidingFeature-NOTDEFINED a owl:Class ;
    rdfs:label "NOTDEFINED"^^xsd:string ;
    rdfs:comment "Describe products of class NOTDEFINED a specialisation of VoidingFeature"^^xsd:string ;
    rdfs:seeAlso ifc:IfcVoidingFeatureEnumType ;
    rdfs:subClassOf p4bldg:VoidingFeature .

p4bldg:VoidingFeature-USERDEFINED a owl:Class ;
    rdfs:label "USERDEFINED"^^xsd:string ;
    rdfs:comment "Describe products of class USERDEFINED a specialisation of VoidingFeature"^^xsd:string ;
    rdfs:seeAlso ifc:IfcVoidingFeatureEnumType ;
    rdfs:subClassOf p4bldg:VoidingFeature .

p4bldg:Wall-ELEMENTEDWALL a owl:Class ;
    rdfs:label "ELEMENTEDWALL"^^xsd:string ;
    rdfs:comment "Describe products of class ELEMENTEDWALL a specialisation of Wall"^^xsd:string ;
    rdfs:seeAlso ifc:IfcWallEnumType ;
    rdfs:subClassOf p4bldg:Wall .

p4bldg:Wall-MOVABLE a owl:Class ;
    rdfs:label "MOVABLE"^^xsd:string ;
    rdfs:comment "Describe products of class MOVABLE a specialisation of Wall"^^xsd:string ;
    rdfs:seeAlso ifc:IfcWallEnumType ;
    rdfs:subClassOf p4bldg:Wall .

p4bldg:Wall-NOTDEFINED a owl:Class ;
    rdfs:label "NOTDEFINED"^^xsd:string ;
    rdfs:comment "Describe products of class NOTDEFINED a specialisation of Wall"^^xsd:string ;
    rdfs:seeAlso ifc:IfcWallEnumType ;
    rdfs:subClassOf p4bldg:Wall .

p4bldg:Wall-PARAPET a owl:Class ;
    rdfs:label "PARAPET"^^xsd:string ;
    rdfs:comment "Describe products of class PARAPET a specialisation of Wall"^^xsd:string ;
    rdfs:seeAlso ifc:IfcWallEnumType ;
    rdfs:subClassOf p4bldg:Wall .

p4bldg:Wall-PARTITIONING a owl:Class ;
    rdfs:label "PARTITIONING"^^xsd:string ;
    rdfs:comment "Describe products of class PARTITIONING a specialisation of Wall"^^xsd:string ;
    rdfs:seeAlso ifc:IfcWallEnumType ;
    rdfs:subClassOf p4bldg:Wall .

p4bldg:Wall-PLUMBINGWALL a owl:Class ;
    rdfs:label "PLUMBINGWALL"^^xsd:string ;
    rdfs:comment "Describe products of class PLUMBINGWALL a specialisation of Wall"^^xsd:string ;
    rdfs:seeAlso ifc:IfcWallEnumType ;
    rdfs:subClassOf p4bldg:Wall .

p4bldg:Wall-POLYGONAL a owl:Class ;
    rdfs:label "POLYGONAL"^^xsd:string ;
    rdfs:comment "Describe products of class POLYGONAL a specialisation of Wall"^^xsd:string ;
    rdfs:seeAlso ifc:IfcWallEnumType ;
    rdfs:subClassOf p4bldg:Wall .

p4bldg:Wall-SHEAR a owl:Class ;
    rdfs:label "SHEAR"^^xsd:string ;
    rdfs:comment "Describe products of class SHEAR a specialisation of Wall"^^xsd:string ;
    rdfs:seeAlso ifc:IfcWallEnumType ;
    rdfs:subClassOf p4bldg:Wall .

p4bldg:Wall-SOLIDWALL a owl:Class ;
    rdfs:label "SOLIDWALL"^^xsd:string ;
    rdfs:comment "Describe products of class SOLIDWALL a specialisation of Wall"^^xsd:string ;
    rdfs:seeAlso ifc:IfcWallEnumType ;
    rdfs:subClassOf p4bldg:Wall .

p4bldg:Wall-STANDARD a owl:Class ;
    rdfs:label "STANDARD"^^xsd:string ;
    rdfs:comment "Describe products of class STANDARD a specialisation of Wall"^^xsd:string ;
    rdfs:seeAlso ifc:IfcWallEnumType ;
    rdfs:subClassOf p4bldg:Wall .

p4bldg:Wall-USERDEFINED a owl:Class ;
    rdfs:label "USERDEFINED"^^xsd:string ;
    rdfs:comment "Describe products of class USERDEFINED a specialisation of Wall"^^xsd:string ;
    rdfs:seeAlso ifc:IfcWallEnumType ;
    rdfs:subClassOf p4bldg:Wall .

p4bldg:WallElementedCase a owl:Class ;
    rdfs:label "WallElementedCase"^^xsd:string ;
    rdfs:comment "Describe products of class WallElementedCase"^^xsd:string ;
    rdfs:seeAlso ifc:IfcWallElementedCase ;
    rdfs:subClassOf p4bldg:Wall .

p4bldg:WallStandardCase a owl:Class ;
    rdfs:label "WallStandardCase"^^xsd:string ;
    rdfs:comment "Describe products of class WallStandardCase"^^xsd:string ;
    rdfs:seeAlso ifc:IfcWallStandardCase ;
    rdfs:subClassOf p4bldg:Wall .

p4bldg:WasteTerminal-FLOORTRAP a owl:Class ;
    rdfs:label "FLOORTRAP"^^xsd:string ;
    rdfs:comment "Describe products of class FLOORTRAP a specialisation of WasteTerminal"^^xsd:string ;
    rdfs:seeAlso ifc:IfcWasteTerminalEnumType ;
    rdfs:subClassOf p4bldg:WasteTerminal .

p4bldg:WasteTerminal-FLOORWASTE a owl:Class ;
    rdfs:label "FLOORWASTE"^^xsd:string ;
    rdfs:comment "Describe products of class FLOORWASTE a specialisation of WasteTerminal"^^xsd:string ;
    rdfs:seeAlso ifc:IfcWasteTerminalEnumType ;
    rdfs:subClassOf p4bldg:WasteTerminal .

p4bldg:WasteTerminal-GULLYSUMP a owl:Class ;
    rdfs:label "GULLYSUMP"^^xsd:string ;
    rdfs:comment "Describe products of class GULLYSUMP a specialisation of WasteTerminal"^^xsd:string ;
    rdfs:seeAlso ifc:IfcWasteTerminalEnumType ;
    rdfs:subClassOf p4bldg:WasteTerminal .

p4bldg:WasteTerminal-GULLYTRAP a owl:Class ;
    rdfs:label "GULLYTRAP"^^xsd:string ;
    rdfs:comment "Describe products of class GULLYTRAP a specialisation of WasteTerminal"^^xsd:string ;
    rdfs:seeAlso ifc:IfcWasteTerminalEnumType ;
    rdfs:subClassOf p4bldg:WasteTerminal .

p4bldg:WasteTerminal-NOTDEFINED a owl:Class ;
    rdfs:label "NOTDEFINED"^^xsd:string ;
    rdfs:comment "Describe products of class NOTDEFINED a specialisation of WasteTerminal"^^xsd:string ;
    rdfs:seeAlso ifc:IfcWasteTerminalEnumType ;
    rdfs:subClassOf p4bldg:WasteTerminal .

p4bldg:WasteTerminal-ROOFDRAIN a owl:Class ;
    rdfs:label "ROOFDRAIN"^^xsd:string ;
    rdfs:comment "Describe products of class ROOFDRAIN a specialisation of WasteTerminal"^^xsd:string ;
    rdfs:seeAlso ifc:IfcWasteTerminalEnumType ;
    rdfs:subClassOf p4bldg:WasteTerminal .

p4bldg:WasteTerminal-USERDEFINED a owl:Class ;
    rdfs:label "USERDEFINED"^^xsd:string ;
    rdfs:comment "Describe products of class USERDEFINED a specialisation of WasteTerminal"^^xsd:string ;
    rdfs:seeAlso ifc:IfcWasteTerminalEnumType ;
    rdfs:subClassOf p4bldg:WasteTerminal .

p4bldg:WasteTerminal-WASTEDISPOSALUNIT a owl:Class ;
    rdfs:label "WASTEDISPOSALUNIT"^^xsd:string ;
    rdfs:comment "Describe products of class WASTEDISPOSALUNIT a specialisation of WasteTerminal"^^xsd:string ;
    rdfs:seeAlso ifc:IfcWasteTerminalEnumType ;
    rdfs:subClassOf p4bldg:WasteTerminal .

p4bldg:WasteTerminal-WASTETRAP a owl:Class ;
    rdfs:label "WASTETRAP"^^xsd:string ;
    rdfs:comment "Describe products of class WASTETRAP a specialisation of WasteTerminal"^^xsd:string ;
    rdfs:seeAlso ifc:IfcWasteTerminalEnumType ;
    rdfs:subClassOf p4bldg:WasteTerminal .

p4bldg:Window-LIGHTDOME a owl:Class ;
    rdfs:label "LIGHTDOME"^^xsd:string ;
    rdfs:comment "Describe products of class LIGHTDOME a specialisation of Window"^^xsd:string ;
    rdfs:seeAlso ifc:IfcWindowEnumType ;
    rdfs:subClassOf p4bldg:Window .

p4bldg:Window-NOTDEFINED a owl:Class ;
    rdfs:label "NOTDEFINED"^^xsd:string ;
    rdfs:comment "Describe products of class NOTDEFINED a specialisation of Window"^^xsd:string ;
    rdfs:seeAlso ifc:IfcWindowEnumType ;
    rdfs:subClassOf p4bldg:Window .

p4bldg:Window-SKYLIGHT a owl:Class ;
    rdfs:label "SKYLIGHT"^^xsd:string ;
    rdfs:comment "Describe products of class SKYLIGHT a specialisation of Window"^^xsd:string ;
    rdfs:seeAlso ifc:IfcWindowEnumType ;
    rdfs:subClassOf p4bldg:Window .

p4bldg:Window-USERDEFINED a owl:Class ;
    rdfs:label "USERDEFINED"^^xsd:string ;
    rdfs:comment "Describe products of class USERDEFINED a specialisation of Window"^^xsd:string ;
    rdfs:seeAlso ifc:IfcWindowEnumType ;
    rdfs:subClassOf p4bldg:Window .

p4bldg:Window-WINDOW a owl:Class ;
    rdfs:label "WINDOW"^^xsd:string ;
    rdfs:comment "Describe products of class WINDOW a specialisation of Window"^^xsd:string ;
    rdfs:seeAlso ifc:IfcWindowEnumType ;
    rdfs:subClassOf p4bldg:Window .

p4bldg:WindowStandardCase a owl:Class ;
    rdfs:label "WindowStandardCase"^^xsd:string ;
    rdfs:comment "Describe products of class WindowStandardCase"^^xsd:string ;
    rdfs:seeAlso ifc:IfcWindowStandardCase ;
    rdfs:subClassOf p4bldg:Window .

p4bldg:FeatureElementAddition a owl:Class ;
    rdfs:label "FeatureElementAddition"^^xsd:string ;
    rdfs:comment "Describe products of class FeatureElementAddition"^^xsd:string ;
    rdfs:seeAlso ifc:IfcFeatureElementAddition ;
    rdfs:subClassOf p4bldg:FeatureElement .

<https://www.researchgate.net/profile/Georg_Schneider3> a owl:NamedIndividual .

p4bldg:Burner a owl:Class ;
    rdfs:label "Burner"^^xsd:string ;
    rdfs:comment "Describe products of class Burner"^^xsd:string ;
    rdfs:seeAlso ifc:IfcBurner ;
    rdfs:subClassOf p4bldg:EnergyConversionDevice .

p4bldg:Chimney a owl:Class ;
    rdfs:label "Chimney"^^xsd:string ;
    rdfs:comment "Describe products of class Chimney"^^xsd:string ;
    rdfs:seeAlso ifc:IfcChimney ;
    rdfs:subClassOf p4bldg:BuildingElement .

p4bldg:CurtainWall a owl:Class ;
    rdfs:label "CurtainWall"^^xsd:string ;
    rdfs:comment "Describe products of class CurtainWall"^^xsd:string ;
    rdfs:seeAlso ifc:IfcCurtainWall ;
    rdfs:subClassOf p4bldg:BuildingElement .

p4bldg:DistributionElement a owl:Class ;
    rdfs:label "DistributionElement"^^xsd:string ;
    rdfs:comment "Describe products of class DistributionElement"^^xsd:string ;
    rdfs:seeAlso ifc:IfcDistributionElement ;
    rdfs:subClassOf p4bldg:Element .

p4bldg:FeatureElementSubtraction a owl:Class ;
    rdfs:label "FeatureElementSubtraction"^^xsd:string ;
    rdfs:comment "Describe products of class FeatureElementSubtraction"^^xsd:string ;
    rdfs:seeAlso ifc:IfcFeatureElementSubtraction ;
    rdfs:subClassOf p4bldg:FeatureElement .

p4bldg:FlowStorageDevice a owl:Class ;
    rdfs:label "FlowStorageDevice"^^xsd:string ;
    rdfs:comment "Describe products of class FlowStorageDevice"^^xsd:string ;
    rdfs:seeAlso ifc:IfcFlowStorageDevice ;
    rdfs:subClassOf p4bldg:DistributionFlowElement .

p4bldg:FurnishingElement a owl:Class ;
    rdfs:label "FurnishingElement"^^xsd:string ;
    rdfs:comment "Describe products of class FurnishingElement"^^xsd:string ;
    rdfs:seeAlso ifc:IfcFurnishingElement ;
    rdfs:subClassOf p4bldg:Element .

p4bldg:ProjectionElement a owl:Class ;
    rdfs:label "ProjectionElement"^^xsd:string ;
    rdfs:comment "Describe products of class ProjectionElement"^^xsd:string ;
    rdfs:seeAlso ifc:IfcProjectionElement ;
    rdfs:subClassOf p4bldg:FeatureElementAddition .

p4bldg:ReinforcingMesh a owl:Class ;
    rdfs:label "ReinforcingMesh"^^xsd:string ;
    rdfs:comment "Describe products of class ReinforcingMesh"^^xsd:string ;
    rdfs:seeAlso ifc:IfcReinforcingMesh ;
    rdfs:subClassOf p4bldg:ReinforcingElement .

p4bldg:FeatureElement a owl:Class ;
    rdfs:label "FeatureElement"^^xsd:string ;
    rdfs:comment "Describe products of class FeatureElement"^^xsd:string ;
    rdfs:seeAlso ifc:IfcFeatureElement ;
    rdfs:subClassOf p4bldg:Element .

p4bldg:FlowMovingDevice a owl:Class ;
    rdfs:label "FlowMovingDevice"^^xsd:string ;
    rdfs:comment "Describe products of class FlowMovingDevice"^^xsd:string ;
    rdfs:seeAlso ifc:IfcFlowMovingDevice ;
    rdfs:subClassOf p4bldg:DistributionFlowElement .

p4bldg:FlowTreatmentDevice a owl:Class ;
    rdfs:label "FlowTreatmentDevice"^^xsd:string ;
    rdfs:comment "Describe products of class FlowTreatmentDevice"^^xsd:string ;
    rdfs:seeAlso ifc:IfcFlowTreatmentDevice ;
    rdfs:subClassOf p4bldg:DistributionFlowElement .

p4bldg:GeographicElement a owl:Class ;
    rdfs:label "GeographicElement"^^xsd:string ;
    rdfs:comment "Describe products of class GeographicElement"^^xsd:string ;
    rdfs:seeAlso ifc:IfcGeographicElement ;
    rdfs:subClassOf p4bldg:Element .

p4bldg:TubeBundle a owl:Class ;
    rdfs:label "TubeBundle"^^xsd:string ;
    rdfs:comment "Describe products of class TubeBundle"^^xsd:string ;
    rdfs:seeAlso ifc:IfcTubeBundle ;
    rdfs:subClassOf p4bldg:EnergyConversionDevice .

p4bldg:Boiler a owl:Class ;
    rdfs:label "Boiler"^^xsd:string ;
    rdfs:comment "Describe products of class Boiler"^^xsd:string ;
    rdfs:seeAlso ifc:IfcBoiler ;
    rdfs:subClassOf p4bldg:EnergyConversionDevice .

p4bldg:BuildingElementPart a owl:Class ;
    rdfs:label "BuildingElementPart"^^xsd:string ;
    rdfs:comment "Describe products of class BuildingElementPart"^^xsd:string ;
    rdfs:seeAlso ifc:IfcBuildingElementPart ;
    rdfs:subClassOf p4bldg:ElementComponent .

p4bldg:CooledBeam a owl:Class ;
    rdfs:label "CooledBeam"^^xsd:string ;
    rdfs:comment "Describe products of class CooledBeam"^^xsd:string ;
    rdfs:seeAlso ifc:IfcCooledBeam ;
    rdfs:subClassOf p4bldg:EnergyConversionDevice .

p4bldg:DuctSegment a owl:Class ;
    rdfs:label "DuctSegment"^^xsd:string ;
    rdfs:comment "Describe products of class DuctSegment"^^xsd:string ;
    rdfs:seeAlso ifc:IfcDuctSegment ;
    rdfs:subClassOf p4bldg:FlowSegment .

p4bldg:Engine a owl:Class ;
    rdfs:label "Engine"^^xsd:string ;
    rdfs:comment "Describe products of class Engine"^^xsd:string ;
    rdfs:seeAlso ifc:IfcEngine ;
    rdfs:subClassOf p4bldg:EnergyConversionDevice .

p4bldg:FlowSegment a owl:Class ;
    rdfs:label "FlowSegment"^^xsd:string ;
    rdfs:comment "Describe products of class FlowSegment"^^xsd:string ;
    rdfs:seeAlso ifc:IfcFlowSegment ;
    rdfs:subClassOf p4bldg:DistributionFlowElement .

p4bldg:HeatExchanger a owl:Class ;
    rdfs:label "HeatExchanger"^^xsd:string ;
    rdfs:comment "Describe products of class HeatExchanger"^^xsd:string ;
    rdfs:seeAlso ifc:IfcHeatExchanger ;
    rdfs:subClassOf p4bldg:EnergyConversionDevice .

p4bldg:JunctionBox a owl:Class ;
    rdfs:label "JunctionBox"^^xsd:string ;
    rdfs:comment "Describe products of class JunctionBox"^^xsd:string ;
    rdfs:seeAlso ifc:IfcJunctionBox ;
    rdfs:subClassOf p4bldg:FlowFitting .

p4bldg:RampFlight a owl:Class ;
    rdfs:label "RampFlight"^^xsd:string ;
    rdfs:comment "Describe products of class RampFlight"^^xsd:string ;
    rdfs:seeAlso ifc:IfcRampFlight ;
    rdfs:subClassOf p4bldg:BuildingElement .

p4bldg:ReinforcingElement a owl:Class ;
    rdfs:label "ReinforcingElement"^^xsd:string ;
    rdfs:comment "Describe products of class ReinforcingElement"^^xsd:string ;
    rdfs:seeAlso ifc:IfcReinforcingElement ;
    rdfs:subClassOf p4bldg:ElementComponent .

p4bldg:SolarDevice a owl:Class ;
    rdfs:label "SolarDevice"^^xsd:string ;
    rdfs:comment "Describe products of class SolarDevice"^^xsd:string ;
    rdfs:seeAlso ifc:IfcSolarDevice ;
    rdfs:subClassOf p4bldg:EnergyConversionDevice .

p4bldg:SpaceHeater a owl:Class ;
    rdfs:label "SpaceHeater"^^xsd:string ;
    rdfs:comment "Describe products of class SpaceHeater"^^xsd:string ;
    rdfs:seeAlso ifc:IfcSpaceHeater ;
    rdfs:subClassOf p4bldg:FlowTerminal .

p4bldg:SystemFurnitureElement a owl:Class ;
    rdfs:label "SystemFurnitureElement"^^xsd:string ;
    rdfs:comment "Describe products of class SystemFurnitureElement"^^xsd:string ;
    rdfs:seeAlso ifc:IfcSystemFurnitureElement ;
    rdfs:subClassOf p4bldg:FurnishingElement .

p4bldg:VibrationIsolator a owl:Class ;
    rdfs:label "VibrationIsolator"^^xsd:string ;
    rdfs:comment "Describe products of class VibrationIsolator"^^xsd:string ;
    rdfs:seeAlso ifc:IfcVibrationIsolator ;
    rdfs:subClassOf p4bldg:ElementComponent .

p4bldg:AirTerminalBox a owl:Class ;
    rdfs:label "AirTerminalBox"^^xsd:string ;
    rdfs:comment "Describe products of class AirTerminalBox"^^xsd:string ;
    rdfs:seeAlso ifc:IfcAirTerminalBox ;
    rdfs:subClassOf p4bldg:FlowController .

p4bldg:Chiller a owl:Class ;
    rdfs:label "Chiller"^^xsd:string ;
    rdfs:comment "Describe products of class Chiller"^^xsd:string ;
    rdfs:seeAlso ifc:IfcChiller ;
    rdfs:subClassOf p4bldg:EnergyConversionDevice .

p4bldg:Column a owl:Class ;
    rdfs:label "Column"^^xsd:string ;
    rdfs:comment "Describe products of class Column"^^xsd:string ;
    rdfs:seeAlso ifc:IfcColumn ;
    rdfs:subClassOf p4bldg:BuildingElement .

p4bldg:CoolingTower a owl:Class ;
    rdfs:label "CoolingTower"^^xsd:string ;
    rdfs:comment "Describe products of class CoolingTower"^^xsd:string ;
    rdfs:seeAlso ifc:IfcCoolingTower ;
    rdfs:subClassOf p4bldg:EnergyConversionDevice .

p4bldg:DiscreteAccessory a owl:Class ;
    rdfs:label "DiscreteAccessory"^^xsd:string ;
    rdfs:comment "Describe products of class DiscreteAccessory"^^xsd:string ;
    rdfs:seeAlso ifc:IfcDiscreteAccessory ;
    rdfs:subClassOf p4bldg:ElementComponent .

p4bldg:DuctSilencer a owl:Class ;
    rdfs:label "DuctSilencer"^^xsd:string ;
    rdfs:comment "Describe products of class DuctSilencer"^^xsd:string ;
    rdfs:seeAlso ifc:IfcDuctSilencer ;
    rdfs:subClassOf p4bldg:FlowTreatmentDevice .

p4bldg:ElectricGenerator a owl:Class ;
    rdfs:label "ElectricGenerator"^^xsd:string ;
    rdfs:comment "Describe products of class ElectricGenerator"^^xsd:string ;
    rdfs:seeAlso ifc:IfcElectricGenerator ;
    rdfs:subClassOf p4bldg:EnergyConversionDevice .

p4bldg:ElectricTimeControl a owl:Class ;
    rdfs:label "ElectricTimeControl"^^xsd:string ;
    rdfs:comment "Describe products of class ElectricTimeControl"^^xsd:string ;
    rdfs:seeAlso ifc:IfcElectricTimeControl ;
    rdfs:subClassOf p4bldg:FlowController .

p4bldg:Fastener a owl:Class ;
    rdfs:label "Fastener"^^xsd:string ;
    rdfs:comment "Describe products of class Fastener"^^xsd:string ;
    rdfs:seeAlso ifc:IfcFastener ;
    rdfs:subClassOf p4bldg:ElementComponent .

p4bldg:FlowFitting a owl:Class ;
    rdfs:label "FlowFitting"^^xsd:string ;
    rdfs:comment "Describe products of class FlowFitting"^^xsd:string ;
    rdfs:seeAlso ifc:IfcFlowFitting ;
    rdfs:subClassOf p4bldg:DistributionFlowElement .

p4bldg:LightFixture a owl:Class ;
    rdfs:label "LightFixture"^^xsd:string ;
    rdfs:comment "Describe products of class LightFixture"^^xsd:string ;
    rdfs:seeAlso ifc:IfcLightFixture ;
    rdfs:subClassOf p4bldg:FlowTerminal .

p4bldg:MotorConnection a owl:Class ;
    rdfs:label "MotorConnection"^^xsd:string ;
    rdfs:comment "Describe products of class MotorConnection"^^xsd:string ;
    rdfs:seeAlso ifc:IfcMotorConnection ;
    rdfs:subClassOf p4bldg:EnergyConversionDevice .

p4bldg:OpeningElement a owl:Class ;
    rdfs:label "OpeningElement"^^xsd:string ;
    rdfs:comment "Describe products of class OpeningElement"^^xsd:string ;
    rdfs:seeAlso ifc:IfcOpeningElement ;
    rdfs:subClassOf p4bldg:FeatureElementSubtraction .

p4bldg:Plate a owl:Class ;
    rdfs:label "Plate"^^xsd:string ;
    rdfs:comment "Describe products of class Plate"^^xsd:string ;
    rdfs:seeAlso ifc:IfcPlate ;
    rdfs:subClassOf p4bldg:BuildingElement .

p4bldg:Railing a owl:Class ;
    rdfs:label "Railing"^^xsd:string ;
    rdfs:comment "Describe products of class Railing"^^xsd:string ;
    rdfs:seeAlso ifc:IfcRailing ;
    rdfs:subClassOf p4bldg:BuildingElement .

p4bldg:ShadingDevice a owl:Class ;
    rdfs:label "ShadingDevice"^^xsd:string ;
    rdfs:comment "Describe products of class ShadingDevice"^^xsd:string ;
    rdfs:seeAlso ifc:IfcShadingDevice ;
    rdfs:subClassOf p4bldg:BuildingElement .

p4bldg:StackTerminal a owl:Class ;
    rdfs:label "StackTerminal"^^xsd:string ;
    rdfs:comment "Describe products of class StackTerminal"^^xsd:string ;
    rdfs:seeAlso ifc:IfcStackTerminal ;
    rdfs:subClassOf p4bldg:FlowTerminal .

p4bldg:SurfaceFeature a owl:Class ;
    rdfs:label "SurfaceFeature"^^xsd:string ;
    rdfs:comment "Describe products of class SurfaceFeature"^^xsd:string ;
    rdfs:seeAlso ifc:IfcSurfaceFeature ;
    rdfs:subClassOf p4bldg:FeatureElement .

p4bldg:TendonAnchor a owl:Class ;
    rdfs:label "TendonAnchor"^^xsd:string ;
    rdfs:comment "Describe products of class TendonAnchor"^^xsd:string ;
    rdfs:seeAlso ifc:IfcTendonAnchor ;
    rdfs:subClassOf p4bldg:ReinforcingElement .

p4bldg:AirTerminal a owl:Class ;
    rdfs:label "AirTerminal"^^xsd:string ;
    rdfs:comment "Describe products of class AirTerminal"^^xsd:string ;
    rdfs:seeAlso ifc:IfcAirTerminal ;
    rdfs:subClassOf p4bldg:FlowTerminal .

p4bldg:CableCarrierFitting a owl:Class ;
    rdfs:label "CableCarrierFitting"^^xsd:string ;
    rdfs:comment "Describe products of class CableCarrierFitting"^^xsd:string ;
    rdfs:seeAlso ifc:IfcCableCarrierFitting ;
    rdfs:subClassOf p4bldg:FlowFitting .

p4bldg:CableCarrierSegment a owl:Class ;
    rdfs:label "CableCarrierSegment"^^xsd:string ;
    rdfs:comment "Describe products of class CableCarrierSegment"^^xsd:string ;
    rdfs:seeAlso ifc:IfcCableCarrierSegment ;
    rdfs:subClassOf p4bldg:FlowSegment .

p4bldg:CableSegment a owl:Class ;
    rdfs:label "CableSegment"^^xsd:string ;
    rdfs:comment "Describe products of class CableSegment"^^xsd:string ;
    rdfs:seeAlso ifc:IfcCableSegment ;
    rdfs:subClassOf p4bldg:FlowSegment .

p4bldg:Door a owl:Class ;
    rdfs:label "Door"^^xsd:string ;
    rdfs:comment "Describe products of class Door"^^xsd:string ;
    rdfs:seeAlso ifc:IfcDoor ;
    rdfs:subClassOf p4bldg:BuildingElement .

p4bldg:ElectricDistributionBoard a owl:Class ;
    rdfs:label "ElectricDistributionBoard"^^xsd:string ;
    rdfs:comment "Describe products of class ElectricDistributionBoard"^^xsd:string ;
    rdfs:seeAlso ifc:IfcElectricDistributionBoard ;
    rdfs:subClassOf p4bldg:FlowController .

p4bldg:ElementComponent a owl:Class ;
    rdfs:label "ElementComponent"^^xsd:string ;
    rdfs:comment "Describe products of class ElementComponent"^^xsd:string ;
    rdfs:seeAlso ifc:IfcElementComponent ;
    rdfs:subClassOf p4bldg:Element .

p4bldg:FlowMeter a owl:Class ;
    rdfs:label "FlowMeter"^^xsd:string ;
    rdfs:comment "Describe products of class FlowMeter"^^xsd:string ;
    rdfs:seeAlso ifc:IfcFlowMeter ;
    rdfs:subClassOf p4bldg:FlowController .

p4bldg:Interceptor a owl:Class ;
    rdfs:label "Interceptor"^^xsd:string ;
    rdfs:comment "Describe products of class Interceptor"^^xsd:string ;
    rdfs:seeAlso ifc:IfcInterceptor ;
    rdfs:subClassOf p4bldg:FlowTreatmentDevice .

p4bldg:ProtectiveDeviceTrippingUnit a owl:Class ;
    rdfs:label "ProtectiveDeviceTrippingUnit"^^xsd:string ;
    rdfs:comment "Describe products of class ProtectiveDeviceTrippingUnit"^^xsd:string ;
    rdfs:seeAlso ifc:IfcProtectiveDeviceTrippingUnit ;
    rdfs:subClassOf p4bldg:DistributionControlElement .

p4bldg:Tendon a owl:Class ;
    rdfs:label "Tendon"^^xsd:string ;
    rdfs:comment "Describe products of class Tendon"^^xsd:string ;
    rdfs:seeAlso ifc:IfcTendon ;
    rdfs:subClassOf p4bldg:ReinforcingElement .

p4bldg:Window a owl:Class ;
    rdfs:label "Window"^^xsd:string ;
    rdfs:comment "Describe products of class Window"^^xsd:string ;
    rdfs:seeAlso ifc:IfcWindow ;
    rdfs:subClassOf p4bldg:BuildingElement .

p4bldg:Actuator a owl:Class ;
    rdfs:label "Actuator"^^xsd:string ;
    rdfs:comment "Describe products of class Actuator"^^xsd:string ;
    rdfs:seeAlso ifc:IfcActuator ;
    rdfs:subClassOf p4bldg:DistributionControlElement .

p4bldg:BuildingElementProxy a owl:Class ;
    rdfs:label "BuildingElementProxy"^^xsd:string ;
    rdfs:comment "Describe products of class BuildingElementProxy"^^xsd:string ;
    rdfs:seeAlso ifc:IfcBuildingElementProxy ;
    rdfs:subClassOf p4bldg:BuildingElement .

p4bldg:CableFitting a owl:Class ;
    rdfs:label "CableFitting"^^xsd:string ;
    rdfs:comment "Describe products of class CableFitting"^^xsd:string ;
    rdfs:seeAlso ifc:IfcCableFitting ;
    rdfs:subClassOf p4bldg:FlowFitting .

p4bldg:Controller a owl:Class ;
    rdfs:label "Controller"^^xsd:string ;
    rdfs:comment "Describe products of class Controller"^^xsd:string ;
    rdfs:seeAlso ifc:IfcController ;
    rdfs:subClassOf p4bldg:DistributionControlElement .

p4bldg:DistributionControlElement a owl:Class ;
    rdfs:label "DistributionControlElement"^^xsd:string ;
    rdfs:comment "Describe products of class DistributionControlElement"^^xsd:string ;
    rdfs:seeAlso ifc:IfcDistributionControlElement ;
    rdfs:subClassOf p4bldg:DistributionElement .

p4bldg:ElectricFlowStorageDevice a owl:Class ;
    rdfs:label "ElectricFlowStorageDevice"^^xsd:string ;
    rdfs:comment "Describe products of class ElectricFlowStorageDevice"^^xsd:string ;
    rdfs:seeAlso ifc:IfcElectricFlowStorageDevice ;
    rdfs:subClassOf p4bldg:FlowStorageDevice .

p4bldg:ElectricMotor a owl:Class ;
    rdfs:label "ElectricMotor"^^xsd:string ;
    rdfs:comment "Describe products of class ElectricMotor"^^xsd:string ;
    rdfs:seeAlso ifc:IfcElectricMotor ;
    rdfs:subClassOf p4bldg:EnergyConversionDevice .

p4bldg:FireSuppressionTerminal a owl:Class ;
    rdfs:label "FireSuppressionTerminal"^^xsd:string ;
    rdfs:comment "Describe products of class FireSuppressionTerminal"^^xsd:string ;
    rdfs:seeAlso ifc:IfcFireSuppressionTerminal ;
    rdfs:subClassOf p4bldg:FlowTerminal .

p4bldg:Footing a owl:Class ;
    rdfs:label "Footing"^^xsd:string ;
    rdfs:comment "Describe products of class Footing"^^xsd:string ;
    rdfs:seeAlso ifc:IfcFooting ;
    rdfs:subClassOf p4bldg:BuildingElement .

p4bldg:MedicalDevice a owl:Class ;
    rdfs:label "MedicalDevice"^^xsd:string ;
    rdfs:comment "Describe products of class MedicalDevice"^^xsd:string ;
    rdfs:seeAlso ifc:IfcMedicalDevice ;
    rdfs:subClassOf p4bldg:FlowTerminal .

p4bldg:Outlet a owl:Class ;
    rdfs:label "Outlet"^^xsd:string ;
    rdfs:comment "Describe products of class Outlet"^^xsd:string ;
    rdfs:seeAlso ifc:IfcOutlet ;
    rdfs:subClassOf p4bldg:FlowTerminal .

p4bldg:PipeSegment a owl:Class ;
    rdfs:label "PipeSegment"^^xsd:string ;
    rdfs:comment "Describe products of class PipeSegment"^^xsd:string ;
    rdfs:seeAlso ifc:IfcPipeSegment ;
    rdfs:subClassOf p4bldg:FlowSegment .

p4bldg:StairFlight a owl:Class ;
    rdfs:label "StairFlight"^^xsd:string ;
    rdfs:comment "Describe products of class StairFlight"^^xsd:string ;
    rdfs:seeAlso ifc:IfcStairFlight ;
    rdfs:subClassOf p4bldg:BuildingElement .

p4bldg:Transformer a owl:Class ;
    rdfs:label "Transformer"^^xsd:string ;
    rdfs:comment "Describe products of class Transformer"^^xsd:string ;
    rdfs:seeAlso ifc:IfcTransformer ;
    rdfs:subClassOf p4bldg:EnergyConversionDevice .

p4bldg:TransportElement a owl:Class ;
    rdfs:label "TransportElement"^^xsd:string ;
    rdfs:comment "Describe products of class TransportElement"^^xsd:string ;
    rdfs:seeAlso ifc:IfcTransportElement ;
    rdfs:subClassOf p4bldg:Element .

p4bldg:UnitaryEquipment a owl:Class ;
    rdfs:label "UnitaryEquipment"^^xsd:string ;
    rdfs:comment "Describe products of class UnitaryEquipment"^^xsd:string ;
    rdfs:seeAlso ifc:IfcUnitaryEquipment ;
    rdfs:subClassOf p4bldg:EnergyConversionDevice .

p4bldg:Alarm a owl:Class ;
    rdfs:label "Alarm"^^xsd:string ;
    rdfs:comment "Describe products of class Alarm"^^xsd:string ;
    rdfs:seeAlso ifc:IfcAlarm ;
    rdfs:subClassOf p4bldg:DistributionControlElement .

p4bldg:Evaporator a owl:Class ;
    rdfs:label "Evaporator"^^xsd:string ;
    rdfs:comment "Describe products of class Evaporator"^^xsd:string ;
    rdfs:seeAlso ifc:IfcEvaporator ;
    rdfs:subClassOf p4bldg:EnergyConversionDevice .

p4bldg:Filter a owl:Class ;
    rdfs:label "Filter"^^xsd:string ;
    rdfs:comment "Describe products of class Filter"^^xsd:string ;
    rdfs:seeAlso ifc:IfcFilter ;
    rdfs:subClassOf p4bldg:FlowTreatmentDevice .

p4bldg:FlowController a owl:Class ;
    rdfs:label "FlowController"^^xsd:string ;
    rdfs:comment "Describe products of class FlowController"^^xsd:string ;
    rdfs:seeAlso ifc:IfcFlowController ;
    rdfs:subClassOf p4bldg:DistributionFlowElement .

p4bldg:Pile a owl:Class ;
    rdfs:label "Pile"^^xsd:string ;
    rdfs:comment "Describe products of class Pile"^^xsd:string ;
    rdfs:seeAlso ifc:IfcPile ;
    rdfs:subClassOf p4bldg:BuildingElement .

p4bldg:Ramp a owl:Class ;
    rdfs:label "Ramp"^^xsd:string ;
    rdfs:comment "Describe products of class Ramp"^^xsd:string ;
    rdfs:seeAlso ifc:IfcRamp ;
    rdfs:subClassOf p4bldg:BuildingElement .

p4bldg:Slab a owl:Class ;
    rdfs:label "Slab"^^xsd:string ;
    rdfs:comment "Describe products of class Slab"^^xsd:string ;
    rdfs:seeAlso ifc:IfcSlab ;
    rdfs:subClassOf p4bldg:BuildingElement .

p4bldg:VoidingFeature a owl:Class ;
    rdfs:label "VoidingFeature"^^xsd:string ;
    rdfs:comment "Describe products of class VoidingFeature"^^xsd:string ;
    rdfs:seeAlso ifc:IfcVoidingFeature ;
    rdfs:subClassOf p4bldg:FeatureElementSubtraction .

p4bldg:Beam a owl:Class ;
    rdfs:label "Beam"^^xsd:string ;
    rdfs:comment "Describe products of class Beam"^^xsd:string ;
    rdfs:seeAlso ifc:IfcBeam ;
    rdfs:subClassOf p4bldg:BuildingElement .

p4bldg:Coil a owl:Class ;
    rdfs:label "Coil"^^xsd:string ;
    rdfs:comment "Describe products of class Coil"^^xsd:string ;
    rdfs:seeAlso ifc:IfcCoil ;
    rdfs:subClassOf p4bldg:EnergyConversionDevice .

p4bldg:Condenser a owl:Class ;
    rdfs:label "Condenser"^^xsd:string ;
    rdfs:comment "Describe products of class Condenser"^^xsd:string ;
    rdfs:seeAlso ifc:IfcCondenser ;
    rdfs:subClassOf p4bldg:EnergyConversionDevice .

p4bldg:DistributionFlowElement a owl:Class ;
    rdfs:label "DistributionFlowElement"^^xsd:string ;
    rdfs:comment "Describe products of class DistributionFlowElement"^^xsd:string ;
    rdfs:seeAlso ifc:IfcDistributionFlowElement ;
    rdfs:subClassOf p4bldg:DistributionElement .

p4bldg:DuctFitting a owl:Class ;
    rdfs:label "DuctFitting"^^xsd:string ;
    rdfs:comment "Describe products of class DuctFitting"^^xsd:string ;
    rdfs:seeAlso ifc:IfcDuctFitting ;
    rdfs:subClassOf p4bldg:FlowFitting .

p4bldg:Fan a owl:Class ;
    rdfs:label "Fan"^^xsd:string ;
    rdfs:comment "Describe products of class Fan"^^xsd:string ;
    rdfs:seeAlso ifc:IfcFan ;
    rdfs:subClassOf p4bldg:FlowMovingDevice .

p4bldg:Furniture a owl:Class ;
    rdfs:label "Furniture"^^xsd:string ;
    rdfs:comment "Describe products of class Furniture"^^xsd:string ;
    rdfs:seeAlso ifc:IfcFurniture ;
    rdfs:subClassOf p4bldg:FurnishingElement .

p4bldg:PipeFitting a owl:Class ;
    rdfs:label "PipeFitting"^^xsd:string ;
    rdfs:comment "Describe products of class PipeFitting"^^xsd:string ;
    rdfs:seeAlso ifc:IfcPipeFitting ;
    rdfs:subClassOf p4bldg:FlowFitting .

p4bldg:ProtectiveDevice a owl:Class ;
    rdfs:label "ProtectiveDevice"^^xsd:string ;
    rdfs:comment "Describe products of class ProtectiveDevice"^^xsd:string ;
    rdfs:seeAlso ifc:IfcProtectiveDevice ;
    rdfs:subClassOf p4bldg:FlowController .

p4bldg:Pump a owl:Class ;
    rdfs:label "Pump"^^xsd:string ;
    rdfs:comment "Describe products of class Pump"^^xsd:string ;
    rdfs:seeAlso ifc:IfcPump ;
    rdfs:subClassOf p4bldg:FlowMovingDevice .

p4bldg:Tank a owl:Class ;
    rdfs:label "Tank"^^xsd:string ;
    rdfs:comment "Describe products of class Tank"^^xsd:string ;
    rdfs:seeAlso ifc:IfcTank ;
    rdfs:subClassOf p4bldg:FlowStorageDevice .

p4bldg:WasteTerminal a owl:Class ;
    rdfs:label "WasteTerminal"^^xsd:string ;
    rdfs:comment "Describe products of class WasteTerminal"^^xsd:string ;
    rdfs:seeAlso ifc:IfcWasteTerminal ;
    rdfs:subClassOf p4bldg:FlowTerminal .

p4bldg:DistributionChamberElement a owl:Class ;
    rdfs:label "DistributionChamberElement"^^xsd:string ;
    rdfs:comment "Describe products of class DistributionChamberElement"^^xsd:string ;
    rdfs:seeAlso ifc:IfcDistributionChamberElement ;
    rdfs:subClassOf p4bldg:DistributionFlowElement .

p4bldg:Element a owl:Class ;
    rdfs:label "Element"^^xsd:string ;
    rdfs:comment "Describe products of class Element"^^xsd:string ;
    rdfs:seeAlso ifc:IfcElement ;
    rdfs:subClassOf <https://w3id.org/product#Product> .

p4bldg:FlowInstrument a owl:Class ;
    rdfs:label "FlowInstrument"^^xsd:string ;
    rdfs:comment "Describe products of class FlowInstrument"^^xsd:string ;
    rdfs:seeAlso ifc:IfcFlowInstrument ;
    rdfs:subClassOf p4bldg:DistributionControlElement .

p4bldg:ReinforcingBar a owl:Class ;
    rdfs:label "ReinforcingBar"^^xsd:string ;
    rdfs:comment "Describe products of class ReinforcingBar"^^xsd:string ;
    rdfs:seeAlso ifc:IfcReinforcingBar ;
    rdfs:subClassOf p4bldg:ReinforcingElement .

p4bldg:UnitaryControlElement a owl:Class ;
    rdfs:label "UnitaryControlElement"^^xsd:string ;
    rdfs:comment "Describe products of class UnitaryControlElement"^^xsd:string ;
    rdfs:seeAlso ifc:IfcUnitaryControlElement ;
    rdfs:subClassOf p4bldg:DistributionControlElement .

p4bldg:AirToAirHeatRecovery a owl:Class ;
    rdfs:label "AirToAirHeatRecovery"^^xsd:string ;
    rdfs:comment "Describe products of class AirToAirHeatRecovery"^^xsd:string ;
    rdfs:seeAlso ifc:IfcAirToAirHeatRecovery ;
    rdfs:subClassOf p4bldg:EnergyConversionDevice .

p4bldg:ElementAssembly a owl:Class ;
    rdfs:label "ElementAssembly"^^xsd:string ;
    rdfs:comment "Describe products of class ElementAssembly"^^xsd:string ;
    rdfs:seeAlso ifc:IfcElementAssembly ;
    rdfs:subClassOf p4bldg:Element .

p4bldg:EvaporativeCooler a owl:Class ;
    rdfs:label "EvaporativeCooler"^^xsd:string ;
    rdfs:comment "Describe products of class EvaporativeCooler"^^xsd:string ;
    rdfs:seeAlso ifc:IfcEvaporativeCooler ;
    rdfs:subClassOf p4bldg:EnergyConversionDevice .

p4bldg:Lamp a owl:Class ;
    rdfs:label "Lamp"^^xsd:string ;
    rdfs:comment "Describe products of class Lamp"^^xsd:string ;
    rdfs:seeAlso ifc:IfcLamp ;
    rdfs:subClassOf p4bldg:FlowTerminal .

p4bldg:SwitchingDevice a owl:Class ;
    rdfs:label "SwitchingDevice"^^xsd:string ;
    rdfs:comment "Describe products of class SwitchingDevice"^^xsd:string ;
    rdfs:seeAlso ifc:IfcSwitchingDevice ;
    rdfs:subClassOf p4bldg:FlowController .

p4bldg:Covering a owl:Class ;
    rdfs:label "Covering"^^xsd:string ;
    rdfs:comment "Describe products of class Covering"^^xsd:string ;
    rdfs:seeAlso ifc:IfcCovering ;
    rdfs:subClassOf p4bldg:BuildingElement .

p4bldg:MechanicalFastener a owl:Class ;
    rdfs:label "MechanicalFastener"^^xsd:string ;
    rdfs:comment "Describe products of class MechanicalFastener"^^xsd:string ;
    rdfs:seeAlso ifc:IfcMechanicalFastener ;
    rdfs:subClassOf p4bldg:ElementComponent .

p4bldg:SanitaryTerminal a owl:Class ;
    rdfs:label "SanitaryTerminal"^^xsd:string ;
    rdfs:comment "Describe products of class SanitaryTerminal"^^xsd:string ;
    rdfs:seeAlso ifc:IfcSanitaryTerminal ;
    rdfs:subClassOf p4bldg:FlowTerminal .

p4bldg:AudioVisualAppliance a owl:Class ;
    rdfs:label "AudioVisualAppliance"^^xsd:string ;
    rdfs:comment "Describe products of class AudioVisualAppliance"^^xsd:string ;
    rdfs:seeAlso ifc:IfcAudioVisualAppliance ;
    rdfs:subClassOf p4bldg:FlowTerminal .

p4bldg:Damper a owl:Class ;
    rdfs:label "Damper"^^xsd:string ;
    rdfs:comment "Describe products of class Damper"^^xsd:string ;
    rdfs:seeAlso ifc:IfcDamper ;
    rdfs:subClassOf p4bldg:FlowController .

p4bldg:FlowTerminal a owl:Class ;
    rdfs:label "FlowTerminal"^^xsd:string ;
    rdfs:comment "Describe products of class FlowTerminal"^^xsd:string ;
    rdfs:seeAlso ifc:IfcFlowTerminal ;
    rdfs:subClassOf p4bldg:DistributionFlowElement .

p4bldg:Wall a owl:Class ;
    rdfs:label "Wall"^^xsd:string ;
    rdfs:comment "Describe products of class Wall"^^xsd:string ;
    rdfs:seeAlso ifc:IfcWall ;
    rdfs:subClassOf p4bldg:BuildingElement .

p4bldg:CommunicationsAppliance a owl:Class ;
    rdfs:label "CommunicationsAppliance"^^xsd:string ;
    rdfs:comment "Describe products of class CommunicationsAppliance"^^xsd:string ;
    rdfs:seeAlso ifc:IfcCommunicationsAppliance ;
    rdfs:subClassOf p4bldg:FlowTerminal .

p4bldg:Humidifier a owl:Class ;
    rdfs:label "Humidifier"^^xsd:string ;
    rdfs:comment "Describe products of class Humidifier"^^xsd:string ;
    rdfs:seeAlso ifc:IfcHumidifier ;
    rdfs:subClassOf p4bldg:EnergyConversionDevice .

p4bldg:Member a owl:Class ;
    rdfs:label "Member"^^xsd:string ;
    rdfs:comment "Describe products of class Member"^^xsd:string ;
    rdfs:seeAlso ifc:IfcMember ;
    rdfs:subClassOf p4bldg:BuildingElement .

p4bldg:Roof a owl:Class ;
    rdfs:label "Roof"^^xsd:string ;
    rdfs:comment "Describe products of class Roof"^^xsd:string ;
    rdfs:seeAlso ifc:IfcRoof ;
    rdfs:subClassOf p4bldg:BuildingElement .

p4bldg:Stair a owl:Class ;
    rdfs:label "Stair"^^xsd:string ;
    rdfs:comment "Describe products of class Stair"^^xsd:string ;
    rdfs:seeAlso ifc:IfcStair ;
    rdfs:subClassOf p4bldg:BuildingElement .

p4bldg:Compressor a owl:Class ;
    rdfs:label "Compressor"^^xsd:string ;
    rdfs:comment "Describe products of class Compressor"^^xsd:string ;
    rdfs:seeAlso ifc:IfcCompressor ;
    rdfs:subClassOf p4bldg:FlowMovingDevice .

p4bldg:ElectricAppliance a owl:Class ;
    rdfs:label "ElectricAppliance"^^xsd:string ;
    rdfs:comment "Describe products of class ElectricAppliance"^^xsd:string ;
    rdfs:seeAlso ifc:IfcElectricAppliance ;
    rdfs:subClassOf p4bldg:FlowTerminal .

p4bldg:EnergyConversionDevice a owl:Class ;
    rdfs:label "EnergyConversionDevice"^^xsd:string ;
    rdfs:comment "Describe products of class EnergyConversionDevice"^^xsd:string ;
    rdfs:seeAlso ifc:IfcEnergyConversionDevice ;
    rdfs:subClassOf p4bldg:DistributionFlowElement .

p4bldg:BuildingElement a owl:Class ;
    rdfs:label "BuildingElement"^^xsd:string ;
    rdfs:comment "Describe products of class BuildingElement"^^xsd:string ;
    rdfs:seeAlso ifc:IfcBuildingElement ;
    rdfs:subClassOf p4bldg:Element .

p4bldg:Valve a owl:Class ;
    rdfs:label "Valve"^^xsd:string ;
    rdfs:comment "Describe products of class Valve"^^xsd:string ;
    rdfs:seeAlso ifc:IfcValve ;
    rdfs:subClassOf p4bldg:FlowController .

p4bldg:Sensor a owl:Class ;
    rdfs:label "Sensor"^^xsd:string ;
    rdfs:comment "Describe products of class Sensor"^^xsd:string ;
    rdfs:seeAlso ifc:IfcSensor ;
    rdfs:subClassOf p4bldg:DistributionControlElement .

